VACCS with new

theories/Labelled_Transition_System/Examples_of_LTS/VACCS/VACCS_Instance.v
@@ -42,6 +42,23 @@ Parameter (channel_eq_dec : EqDecision Channel).
 Parameter (channel_is_countable : Countable Channel).
 #[global] Instance channel_countable : Countable Channel. by exact channel_is_countable. Defined.
 
+(* Values and their bound variables *)
+Inductive ChannelData :=
+| cstC : Channel -> ChannelData
+| bvarC : nat -> ChannelData. (* variable as De Bruijn indices *) 
+
+Coercion cstC : Channel >-> ChannelData.
+Coercion bvarC : nat >-> ChannelData.
+
+Lemma ChannelData_dec : forall (x y : ChannelData) , {x = y} + {x <> y}.
+Proof.
+decide equality. 
+* destruct (decide(c = c0)). left. assumption. right. assumption.
+* destruct (decide (n = n0)). left. assumption. right. assumption.
+Qed.
+
+#[global] Instance channeldata_eqdecision : EqDecision ChannelData. by exact ChannelData_dec . Defined.
+
 
 (*************************************** Values ******************************************)
 Parameter (Value : Type).
@@ -60,25 +77,6 @@ Inductive Data :=
 Coercion cst : Value >-> Data.
 Coercion bvar : nat >-> Data.
 
-Inductive TypeOfActions := 
-| act : Channel -> Data -> TypeOfActions.
-
-Notation "c ⋉ v" := (act c v) (at level 50).
-
-Inductive Equation (A : Type) : Type :=
-| Equality : A -> A -> Equation A.
-
-Arguments  Equality {_} _ _.
-
-Notation "x == y" := (Equality x y) (at level 50).
-
-(* Definition Eval_Eq (E : Equation Data) : option bool :=
-match E with
-| cst v0 == cst v1 => if (decide (v0 = v1)) then (Some true)
-                                           else (Some false)
-| _ => None
-end. *)
-
 Lemma Data_dec : forall (x y : Data) , {x = y} + {x <> y}.
 Proof.
 decide equality. 
@@ -87,6 +85,42 @@ decide equality.
 Qed.
 
 #[global] Instance data_eqdecision : EqDecision Data. by exact Data_dec . Defined.
+
+(*********************Labels **********************)
+
+Inductive TypeOfActions := 
+| act : ChannelData -> Data -> TypeOfActions.
+
+Notation "c ⋉ v" := (act c v) (at level 50).
+
+Definition ChannelData_of (a : TypeOfActions) : ChannelData := 
+match a with 
+| c ⋉ v => c
+end.
+
+Definition Data_of (a : TypeOfActions) : Data := 
+match a with 
+| c ⋉ d => d
+end.
+
+Definition ChannelData_of_ext (μ : ExtAct TypeOfActions) : ChannelData := 
+match μ with 
+| ActIn (c ⋉ v) => c
+| ActOut (c ⋉ v) => c
+end.
+
+Definition Data_of_ext (μ : ExtAct TypeOfActions) : Data := 
+match μ with 
+| ActIn (c ⋉ v) => v
+| ActOut (c ⋉ v) => v
+end.
+
+Inductive Equation (A : Type) : Type :=
+| Equality : A -> A -> Equation A.
+
+Arguments  Equality {_} _ _.
+
+Notation "x == y" := (Equality x y) (at level 50).
 
 Definition Eval_Eq (E : Equation Data) : option bool :=
 match E with
@@ -110,7 +144,9 @@ Inductive proc : Type :=
 | pr_if_then_else : Equation Data -> proc -> proc -> proc
 (*The Guards*)
 (*An output is a name of a channel, an ouput value, followed by a process*)
-| pr_output : Channel -> Data -> proc
+| pr_output : ChannelData -> Data -> proc
+(* Restriction of a channel*)
+| pr_restrict : proc -> proc
 | g : gproc -> proc
 
 with gproc : Type :=
@@ -119,7 +155,7 @@ with gproc : Type :=
 (* The Process that does nothing*)
 | gpr_nil : gproc
 (*An input is a name of a channel, an input variable, followed by a process*)
-| gpr_input : Channel ->  proc -> gproc
+| gpr_input : ChannelData ->  proc -> gproc
 (*A tau action : does nothing *)
 | gpr_tau : proc -> gproc
 (* To choose between two processes*)
@@ -140,6 +176,7 @@ Notation "P ‖ Q" := (pr_par P Q) (at level 50).
 Notation "c ! v • 𝟘" := (pr_output c v) (at level 50).
 Notation "c ? x • P" := (gpr_input c P) (at level 50).
 Notation "'t' • P" := (gpr_tau P) (at level 50).
+Notation "'ν' P" := (pr_restrict P) (at level 50).
 Notation "'If' C 'Then' P 'Else' Q" := (pr_if_then_else C P Q)
 (at level 200, right associativity, format
 "'[v   ' 'If'  C '/' '[' 'Then'  P  ']' '/' '[' 'Else'  Q ']' ']'").
@@ -171,6 +208,7 @@ match p with
 | rec x • P =>  rec x • (subst_in_proc k X P)
 | If C Then P Else Q => If (subst_in_Equation k X C) Then (subst_in_proc k X P) Else (subst_in_proc k X Q)
 | c ! v • 𝟘 => c ! (subst_Data k X v) • 𝟘
+| ν P => ν (subst_in_proc k X P)
 | g M => subst_in_gproc k X M
 end
 
@@ -198,6 +236,12 @@ match E with
 | D1 == D2 => (NewVar_in_Data k D1) == (NewVar_in_Data k D2)
 end.
 
+Definition NewVar_in_ext (k : nat) (μ : ExtAct TypeOfActions) : ExtAct TypeOfActions :=
+match μ with
+| ActIn (c ⋉ v) => ActIn (c ⋉ (NewVar_in_Data k v))
+| ActOut (c ⋉ v) => ActOut (c ⋉ (NewVar_in_Data k v))
+end.
+
 Fixpoint NewVar (k : nat) (p : proc) {struct p} : proc :=
 match p with
 | P ‖ Q => (NewVar k P) ‖ (NewVar k Q)
@@ -205,6 +249,7 @@ match p with
 | rec x • P =>  rec x • (NewVar k P)
 | If C Then P Else Q => If (NewVar_in_Equation k C) Then (NewVar k P) Else (NewVar k Q)
 | c ! v • 𝟘 => c ! (NewVar_in_Data k v) • 𝟘
+| ν P => ν (NewVar k P)
 | g M => gNewVar k M
 end
 
@@ -217,6 +262,74 @@ match M with
 | p1 + p2 => (gNewVar k p1) + (gNewVar k p2)
 end.
 
+Definition NewVar_in_ChannelData (k : nat) (Y : ChannelData) : ChannelData := 
+match Y with
+| cstC v => cstC v
+| bvarC i => if (decide(k < (S i))) then bvarC (S i) else bvarC i
+end.
+
+Definition NewVarC_in_ext (k : nat) (μ : ExtAct TypeOfActions) : ExtAct TypeOfActions :=
+match μ with
+| ActIn (c ⋉ v) => ActIn ((NewVar_in_ChannelData k c) ⋉ v)
+| ActOut (c ⋉ v) => ActOut ((NewVar_in_ChannelData k c) ⋉ v)
+end.
+
+Fixpoint NewVarC (k : nat) (p : proc) {struct p} : proc :=
+match p with
+| P ‖ Q => (NewVarC k P) ‖ (NewVarC k Q)
+| pr_var i => pr_var i
+| rec x • P =>  rec x • (NewVarC k P)
+| If C Then P Else Q => If C
+                          Then (NewVarC k P)
+                          Else (NewVarC k Q)
+| c ! v • 𝟘 => (NewVar_in_ChannelData k c) ! v • 𝟘
+| ν P => ν (NewVarC (S k) P)
+| g M => gNewVarC k M
+end
+
+with gNewVarC k M {struct M} : gproc :=
+match M with 
+| ① => ①
+| 𝟘 => 𝟘
+| c ? x • p => (NewVar_in_ChannelData k c) ? x • (NewVarC k p)
+| t • p => t • (NewVarC k p)
+| p1 + p2 => (gNewVarC k p1) + (gNewVarC k p2)
+end.
+
+Definition VarC_add (k : nat) (c : ChannelData) : ChannelData :=
+match c with
+| cstC c => cstC c
+| bvarC i => bvarC (k + i)
+end.
+
+Definition VarC_TypeOfActions_add (k : nat) (a : TypeOfActions) : TypeOfActions :=
+match a with
+| (c ⋉ v) => (VarC_add k c) ⋉ v
+end.
+
+Lemma VarC_TypeOfActions_add_add (k : nat) (i : nat) (a : TypeOfActions) :
+        VarC_TypeOfActions_add k (VarC_TypeOfActions_add i a) = VarC_TypeOfActions_add (k + i) a.
+Proof.
+  revert i a.
+  induction k; destruct a;destruct c; simpl ;eauto.
+  f_equal. replace (k + (i + n))%nat with (k + i + n)%nat by lia. eauto.
+Qed.
+
+Definition VarC_action_add (k : nat) (μ : ExtAct TypeOfActions) : ExtAct TypeOfActions :=
+match μ with
+| ActIn (c ⋉ v) => ActIn ((VarC_add k c) ⋉ v)
+| ActOut (c ⋉ v) => ActOut ((VarC_add k c) ⋉ v)
+end.
+
+Lemma VarC_action_add_add (k : nat) (i : nat) (μ : ExtAct TypeOfActions) :
+        VarC_action_add k (VarC_action_add i μ) = VarC_action_add (k + i) μ.
+Proof.
+  revert k μ.
+  induction k; destruct μ ; destruct a; destruct c; intros; simpl; eauto.
+  + f_equal. f_equal. f_equal. lia.
+  + f_equal. f_equal. f_equal. lia.
+Qed.
+
 (* Substitution for the Recursive Variable *)
 Fixpoint pr_subst (id : nat) (p : proc) (q : proc) : proc :=
   match p with 
@@ -225,6 +338,7 @@ Fixpoint pr_subst (id : nat) (p : proc) (q : proc) : proc :=
   | rec id' • p => if decide (id = id') then p else rec id' • (pr_subst id p q)
   | If C Then P Else Q => If C Then (pr_subst id P q) Else (pr_subst id Q q)
   | c ! v • 𝟘 => c ! v • 𝟘
+  | ν P => ν (pr_subst id P (NewVarC 0 q))
   | g gp => g (gpr_subst id gp q)
 end
 
@@ -254,6 +368,12 @@ Inductive lts : proc-> (ActIO TypeOfActions) -> proc -> Prop :=
     lts (If E Then p Else q) α p'
 | lts_ifZero : forall {p q q' α E}, Eval_Eq E = Some false -> lts q α q' -> 
     lts (If E Then p Else q) α q'
+
+(*The actions for process restriction*)
+| lts_res_ext : forall {p p' μ}, lts p (ActExt (VarC_action_add 1 μ)) p'
+                    -> lts (ν p) (ActExt μ) (ν p')
+| lts_res_tau : forall {p p'}, lts p τ p' -> lts (ν p) τ (ν p')
+
 
 (* Communication of a channel output and input that have the same name*)
 | lts_comL : forall {c v p1 p2 q1 q2},
@@ -289,6 +409,7 @@ Fixpoint size (p : proc) :=
   | If C Then p Else q => S (size p + size q)
   | rec x • p => S (size p)
   | c ! v • 𝟘 => 1
+  | ν P => S (size P)
   | g p => gsize p
   end
 
@@ -302,6 +423,42 @@ with gsize p :=
 end.
 
 Hint Constructors lts:ccs.
+
+Definition VarSwap_in_ChannelData (k0 : nat) (c : ChannelData) : ChannelData := 
+match c with
+| cstC v => cstC v
+| bvarC k => if (decide (k = k0)) then bvarC (S k0)
+                                  else if (decide (k = S k0)) then bvarC k0
+                                                              else bvarC k
+end.
+
+Definition VarSwap_in_ext (k : nat) (μ : ExtAct TypeOfActions) : ExtAct TypeOfActions := 
+match μ with
+| ActIn (c ⋉ v) => ActIn ((VarSwap_in_ChannelData k c) ⋉ v)
+| ActOut (c ⋉ v) => ActOut ((VarSwap_in_ChannelData k c) ⋉ v)
+end.
+
+Fixpoint VarSwap_in_proc (k0 : nat) (p : proc) {struct p} : proc :=
+match p with
+| P ‖ Q => (VarSwap_in_proc k0 P) ‖ (VarSwap_in_proc k0 Q)
+| pr_var i => pr_var i
+| rec x • P =>  rec x • (VarSwap_in_proc k0 P)
+| If C Then P Else Q => If C
+                          Then (VarSwap_in_proc k0 P)
+                          Else (VarSwap_in_proc k0 Q)
+| c ! v • 𝟘 => (VarSwap_in_ChannelData k0 c) ! v • 𝟘
+| ν P => ν (VarSwap_in_proc (S k0) P)
+| g M => gVarSwap_in_proc k0 M
+end
+
+with gVarSwap_in_proc k0 M {struct M} : gproc :=
+match M with 
+| ① => ①
+| 𝟘 => 𝟘
+| c ? x • p => (VarSwap_in_ChannelData k0 c) ? x • (VarSwap_in_proc k0 p)
+| t • p => t • (VarSwap_in_proc k0 p)
+| p1 + p2 => (gVarSwap_in_proc k0 p1) + (gVarSwap_in_proc k0 p2)
+end.
 
 Reserved Notation "p ≡ q" (at level 70).
 
@@ -328,6 +485,20 @@ Inductive cgr_step : proc -> proc -> Prop :=
 | cgr_par_assoc_rev_step : forall p q r,
     p ‖ (q  ‖ r) ≡ (p ‖ q) ‖ r
 
+(* Rules for the Restriction *)
+| cgr_res_nil_step :
+   ν (g 𝟘) ≡ (g 𝟘)
+| cgr_res_nil_rev_step :
+   (g 𝟘) ≡ ν (g 𝟘)
+| cgr_res_swap_step : forall p,
+    ν (ν p) ≡ ν (ν (VarSwap_in_proc 0 p))
+| cgr_res_swap_rev_step : forall p,
+    ν (ν (VarSwap_in_proc 0 p)) ≡ ν (ν p)
+| cgr_res_scope_step : forall p q,
+    ν (p ‖ (NewVarC 0 q)) ≡ (ν p) ‖ q
+| cgr_res_scope_rev_step : forall p q,
+    (ν p) ‖ q ≡ ν (p ‖ (NewVarC 0 q)) 
+
 (* Rules for the Summation *)
 | cgr_choice_nil_step : forall p,
     cgr_step (p + 𝟘) p
@@ -352,6 +523,9 @@ Inductive cgr_step : proc -> proc -> Prop :=
 | cgr_par_step : forall p q r,
     cgr_step p q ->
     p ‖ r ≡ q ‖ r
+| cgr_res_step : forall p q,
+    cgr_step p q ->
+    ν p ≡ ν q
 | cgr_if_left_step : forall C p q q',
     cgr_step q q' ->
     (If C Then p Else q) ≡ (If C Then p Else q')
@@ -367,6 +541,9 @@ Inductive cgr_step : proc -> proc -> Prop :=
 
 
 Hint Constructors cgr_step:cgr_step_structure.
+
+
+
 
 Infix "≡" := cgr_step (at level 70).
 
@@ -454,6 +631,36 @@ Proof.
 constructor.
 apply cgr_par_assoc_rev_step.
 Qed.
+Lemma cgr_res_nil : ν (g 𝟘) ≡* (g 𝟘).
+Proof.
+constructor.
+apply cgr_res_nil_step.
+Qed.
+Lemma cgr_res_nil_rev : (g 𝟘) ≡* ν (g 𝟘).
+Proof.
+constructor.
+apply cgr_res_nil_rev_step.
+Qed.
+Lemma cgr_res_swap : forall p, ν (ν p) ≡* ν (ν (VarSwap_in_proc 0 p)).
+Proof.
+constructor.
+apply cgr_res_swap_step.
+Qed.
+Lemma cgr_res_swap_rev : forall p, ν (ν (VarSwap_in_proc 0 p)) ≡* ν (ν p).
+Proof.
+constructor.
+apply cgr_res_swap_rev_step.
+Qed.
+Lemma cgr_res_scope : forall p q, ν (p ‖ (NewVarC 0 q)) ≡* (ν p) ‖ q.
+Proof.
+constructor.
+apply cgr_res_scope_step.
+Qed.
+Lemma cgr_res_scope_rev : forall p q, (ν p) ‖ q ≡* ν (p ‖ (NewVarC 0 q)).
+Proof.
+constructor.
+apply cgr_res_scope_rev_step.
+Qed.
 Lemma cgr_choice_nil : forall p, p + 𝟘 ≡* p.
 Proof.
 constructor.
@@ -504,6 +711,12 @@ intros. dependent induction H.
 constructor.
 apply cgr_par_step. exact H. eauto with cgr_eq.
 Qed.
+Lemma cgr_res : forall p q, p ≡* q-> ν p ≡* ν q.
+Proof.
+intros. dependent induction H. 
+constructor.
+apply cgr_res_step. exact H. eauto with cgr_eq.
+Qed.
 Lemma cgr_if_left : forall C p q q', q ≡* q' -> (If C Then p Else q) ≡* (If C Then p Else q').
 Proof.
 intros. dependent induction H. 
@@ -552,14 +765,8 @@ Qed.
 cgr_par_nil cgr_par_nil_rev cgr_par_com cgr_par_assoc cgr_par_assoc_rev 
 cgr_choice_nil cgr_choice_nil_rev cgr_choice_com cgr_choice_assoc cgr_choice_assoc_rev
 cgr_recursion cgr_tau cgr_input cgr_if_left cgr_if_right cgr_par cgr_choice
-cgr_full_if cgr_fullchoice cgr_fullpar 
-
-cgr_refl cgr_symm cgr_trans:cgr.
-
-(* Lemma subst_equation E k v x: Eval_Eq E = Some x -> Eval_Eq (subst_in_Equation k v E) = Some x.
-Proof.
-  intros. destruct E. destruct d; destruct d0; simpl in *; eauto; try inversion H.
-Qed. *)
+cgr_full_if cgr_fullchoice cgr_fullpar cgr_res_nil cgr_res_nil_rev cgr_res_swap cgr_res_swap_rev cgr_res
+cgr_res_scope cgr_res_scope_rev cgr_refl cgr_symm cgr_trans:cgr.
 
 Lemma subst_equation E k v x: Eval_Eq E = Some x -> Eval_Eq (subst_in_Equation k v E) = Some x.
 Proof.
@@ -587,6 +794,88 @@ Proof.
   - inversion H; subst.
 Qed.
 
+Lemma subst_and_VarSwap k k0 v p : subst_in_proc k v (VarSwap_in_proc k0 p) = (VarSwap_in_proc k0 (subst_in_proc k v p)).
+Proof. 
+  revert k k0 v.
+  induction p as (p & Hp) using
+    (well_founded_induction (wf_inverse_image _ nat _ size Nat.lt_wf_0)).
+  destruct p; intros; simpl in *.
+  + assert (subst_in_proc k v (VarSwap_in_proc k0 p1) = VarSwap_in_proc k0 (subst_in_proc k v p1)) as eq1.
+    { eapply Hp. simpl. lia. }
+    assert (subst_in_proc k v (VarSwap_in_proc k0 p2) = VarSwap_in_proc k0 (subst_in_proc k v p2)) as eq2.
+    { eapply Hp. simpl. lia. }
+    rewrite eq1, eq2. eauto.
+  + reflexivity.
+  + assert (subst_in_proc k v (VarSwap_in_proc k0 p) = VarSwap_in_proc k0 (subst_in_proc k v p)) as eq.
+    { eapply Hp. simpl. lia. }
+    rewrite eq. eauto.
+  + assert (subst_in_proc k v (VarSwap_in_proc k0 p1) = VarSwap_in_proc k0 (subst_in_proc k v p1)) as eq1.
+    { eapply Hp. simpl. lia. }
+    assert (subst_in_proc k v (VarSwap_in_proc k0 p2) = VarSwap_in_proc k0 (subst_in_proc k v p2)) as eq2.
+    { eapply Hp. simpl. lia. }
+    rewrite eq1, eq2. eauto.
+  + eauto.
+  + assert (subst_in_proc k v (VarSwap_in_proc (S k0) p) = VarSwap_in_proc (S k0) (subst_in_proc k v p)) as eq.
+    { eapply Hp. simpl. lia. }
+    rewrite eq. eauto.
+  + destruct g0; simpl in *.
+    * reflexivity.
+    * reflexivity.
+    * assert ((subst_in_proc (S k) (Succ_bvar v) (VarSwap_in_proc k0 p)) 
+          = (VarSwap_in_proc k0 (subst_in_proc (S k) (Succ_bvar v) p))) as eq.
+      { eapply Hp. simpl. lia. }
+      rewrite eq. eauto.
+   * assert (subst_in_proc k v (VarSwap_in_proc k0 p) = VarSwap_in_proc k0 (subst_in_proc k v p)) as eq.
+     { eapply Hp. simpl. lia. }
+     rewrite eq. eauto.
+   * assert (subst_in_proc k v (VarSwap_in_proc k0 (g g0_1)) = VarSwap_in_proc k0 (subst_in_proc k v (g g0_1))) as eq1.
+     { eapply Hp. simpl. lia. }
+     assert (subst_in_proc k v (VarSwap_in_proc k0 (g g0_2)) = VarSwap_in_proc k0 (subst_in_proc k v (g g0_2))) as eq2.
+     { eapply Hp. simpl. lia. } simpl in *. inversion eq1. inversion eq2.
+     rewrite H0 , H1. eauto.
+Qed.
+
+Lemma subst_and_NewVarC k j v q : subst_in_proc k v (NewVarC j q) = NewVarC j (subst_in_proc k v q).
+Proof.
+  revert k j v.
+  induction q as (q & Hp) using
+    (well_founded_induction (wf_inverse_image _ nat _ size Nat.lt_wf_0)).
+  destruct q; intros; simpl in *.
+  + assert (subst_in_proc k v (NewVarC j q1) = NewVarC j (subst_in_proc k v q1)) as eq1.
+    { eapply Hp. simpl. lia. }
+    assert (subst_in_proc k v (NewVarC j q2) = NewVarC j (subst_in_proc k v q2)) as eq2.
+    { eapply Hp. simpl. lia. }
+    rewrite eq1 , eq2. eauto.
+  + eauto.
+  + assert (subst_in_proc k v (NewVarC j q) = NewVarC j (subst_in_proc k v q)) as eq.
+    { eapply Hp. simpl. lia. }
+    rewrite eq. eauto.
+  + assert (subst_in_proc k v (NewVarC j q1) = NewVarC j (subst_in_proc k v q1)) as eq1.
+    { eapply Hp. simpl. lia. }
+    assert (subst_in_proc k v (NewVarC j q2) = NewVarC j (subst_in_proc k v q2)) as eq2.
+    { eapply Hp. simpl. lia. }
+    rewrite eq1 , eq2. eauto.
+  + eauto.
+  + assert (subst_in_proc k v (NewVarC (S j) q) = NewVarC (S j) (subst_in_proc k v q)) as eq1.
+    { eapply Hp. simpl. eauto. }
+    rewrite eq1. eauto.
+  + destruct g0; simpl in *.
+    * eauto.
+    * eauto.
+    * assert ((subst_in_proc (S k) (Succ_bvar v) (NewVarC j p))
+        = (NewVarC j (subst_in_proc (S k) (Succ_bvar v) p))) as eq.
+      { eapply Hp. simpl. lia. }
+      rewrite eq. eauto.
+    * assert (subst_in_proc k v (NewVarC j p) = NewVarC j (subst_in_proc k v p)) as eq.
+      { eapply Hp. simpl. lia. }
+      rewrite eq. eauto.
+    * assert (subst_in_proc k v (NewVarC j (g g0_1)) = NewVarC j (subst_in_proc k v (g g0_1))) as eq1.
+      { eapply Hp. simpl. lia. }
+      assert (subst_in_proc k v (NewVarC j (g g0_2)) = NewVarC j (subst_in_proc k v (g g0_2))) as eq2.
+      { eapply Hp. simpl. lia. } inversion eq1. inversion eq2. eauto.
+Qed.
+
+
 Lemma Congruence_Respects_Substitution : forall p q v k, p ≡* q -> (subst_in_proc k v p) ≡* (subst_in_proc k v q).
 Proof.
 intros. revert k. revert v. dependent induction H. 
@@ -595,7 +884,92 @@ intros. revert k. revert v. dependent induction H.
   - intros. eapply cgr_if_true_rev; eapply subst_equation in H; eauto.
   - intros. eapply cgr_if_false; eapply subst_equation in H; eauto.
   - intros. eapply cgr_if_false_rev; eapply subst_equation in H; eauto.
+  - intros. rewrite subst_and_VarSwap. eapply cgr_res_swap.
+  - intros. rewrite subst_and_VarSwap. eapply cgr_res_swap_rev.
+  - intros. rewrite subst_and_NewVarC. eapply cgr_res_scope.
+  - intros. rewrite subst_and_NewVarC. eapply cgr_res_scope_rev.
 * eauto with cgr.
+Qed.
+
+Lemma NewVar_and_VarSwap j k0 p : (NewVar j (VarSwap_in_proc k0 p) = VarSwap_in_proc k0 (NewVar j p)).
+Proof.
+  revert j k0.
+  induction p as (p & Hp) using
+    (well_founded_induction (wf_inverse_image _ nat _ size Nat.lt_wf_0)).
+  destruct p; intros; simpl in *.
+  + assert (NewVar j (VarSwap_in_proc k0 p1) = VarSwap_in_proc k0 (NewVar j p1)) as eq1.
+    { eapply Hp. simpl. lia. }
+    assert (NewVar j (VarSwap_in_proc k0 p2) = VarSwap_in_proc k0 (NewVar j p2)) as eq2.
+    { eapply Hp. simpl. lia. }
+    rewrite eq1, eq2. eauto.
+  + reflexivity.
+  + assert (NewVar j (VarSwap_in_proc k0 p) = VarSwap_in_proc k0 (NewVar j p)) as eq.
+    { eapply Hp. simpl. lia. }
+    rewrite eq. eauto.
+  + assert (NewVar j (VarSwap_in_proc k0 p1) = VarSwap_in_proc k0 (NewVar j p1)) as eq1.
+    { eapply Hp. simpl. lia. }
+    assert (NewVar j (VarSwap_in_proc k0 p2) = VarSwap_in_proc k0 (NewVar j p2)) as eq2.
+    { eapply Hp. simpl. lia. }
+    rewrite eq1, eq2. eauto.
+  + eauto.
+  + assert (NewVar j (VarSwap_in_proc (S k0) p) = VarSwap_in_proc (S k0) (NewVar j p)) as eq.
+    { eapply Hp. simpl. lia. }
+    rewrite eq. eauto.
+  + destruct g0; simpl in *.
+    * reflexivity.
+    * reflexivity.
+    * assert (NewVar (S j) (VarSwap_in_proc k0 p) = VarSwap_in_proc k0 (NewVar (S j) p)) as eq.
+      { eapply Hp. simpl. lia. }
+      rewrite eq. eauto.
+   * assert (NewVar j (VarSwap_in_proc k0 p) = VarSwap_in_proc k0 (NewVar j p)) as eq.
+     { eapply Hp. simpl. lia. }
+     rewrite eq. eauto.
+   * assert (NewVar j (VarSwap_in_proc k0 (g g0_1)) = VarSwap_in_proc k0 (NewVar j (g g0_1))) as eq1.
+     { eapply Hp. simpl. lia. }
+     assert (NewVar j (VarSwap_in_proc k0 (g g0_2)) = VarSwap_in_proc k0 (NewVar j (g g0_2))) as eq2.
+     { eapply Hp. simpl. lia. } simpl in *. inversion eq1. inversion eq2.
+     rewrite H0 , H1. eauto.
+Qed.
+
+Lemma NewVar_and_NewVarC j k p : (NewVar k (NewVarC j p) = (NewVarC j (NewVar k p))).
+Proof.
+  revert j k.
+  (* Induction on the size of p*)
+  induction p as (p & Hp) using
+      (well_founded_induction (wf_inverse_image _ nat _ size Nat.lt_wf_0)).
+  intros; destruct p ; simpl in *.
+  + assert (NewVar k (NewVarC j p1) = NewVarC j (NewVar k p1)) as eq1.
+    { eapply Hp; simpl ; lia. }
+    assert (NewVar k (NewVarC j p2) = NewVarC j (NewVar k p2)) as eq2.
+    { eapply Hp; simpl ; lia. }
+    rewrite eq1, eq2. eauto.
+  + eauto.
+  + assert (NewVar k (NewVarC j p) = NewVarC j (NewVar k p)) as eq.
+    { eapply Hp; simpl ; lia. }
+    rewrite eq. eauto.
+  + assert (NewVar k (NewVarC j p1) = NewVarC j (NewVar k p1)) as eq1.
+    { eapply Hp; simpl ; lia. }
+    assert (NewVar k (NewVarC j p2) = NewVarC j (NewVar k p2)) as eq2.
+    { eapply Hp; simpl ; lia. }
+    rewrite eq1, eq2. eauto.
+  + eauto.
+  + assert (NewVar k (NewVarC (S j) p) = NewVarC (S j) (NewVar k p)) as eq.
+    { eapply Hp; simpl ; lia. }
+    rewrite eq. eauto.
+  + destruct g0; simpl in *.
+    * eauto.
+    * eauto.
+    * assert (NewVar (S k) (NewVarC j p) = NewVarC j (NewVar (S k) p)) as eq.
+      { eapply Hp; simpl ; lia. }
+      rewrite eq. eauto.
+    * assert (NewVar k (NewVarC j p) = NewVarC j (NewVar k p)) as eq.
+      { eapply Hp; simpl ; lia. }
+      rewrite eq. eauto.
+    * assert (NewVar k (NewVarC j (g g0_1)) = NewVarC j (NewVar k (g g0_1))) as eq1.
+      { eapply Hp; simpl ; lia. }
+      assert (NewVar k (NewVarC j (g g0_2)) = NewVarC j (NewVar k (g g0_2))) as eq2.
+      { eapply Hp; simpl ; lia. } inversion eq1. inversion eq2.
+      rewrite H0, H1. eauto.
 Qed.
 
 Lemma NewVar_Respects_Congruence : forall p p' j, p ≡* p' -> NewVar j p ≡* NewVar j p'.
@@ -606,8 +980,153 @@ intros.  revert j.  dependent induction H.
 * intros. eapply cgr_if_true_rev; eapply NewVar_equation in H; eauto.
 * intros. eapply cgr_if_false; eapply NewVar_equation in H; eauto.
 * intros. eapply cgr_if_false_rev; eapply NewVar_equation in H; eauto.
-* intros. apply cgr_choice. apply IHcgr_step. 
+* intros. rewrite NewVar_and_VarSwap. eapply cgr_res_swap.
+* intros. rewrite NewVar_and_VarSwap. eapply cgr_res_swap_rev.
+* intros. rewrite NewVar_and_NewVarC. eapply cgr_res_scope.
+* intros. rewrite NewVar_and_NewVarC. eapply cgr_res_scope_rev.
+* intros. apply cgr_choice. apply IHcgr_step.
 - eauto with cgr.
+Qed.
+
+Lemma NewVar_in_ChannelData_and_VarSwap_in_ChannelData j k0 c :
+(NewVar_in_ChannelData (S (S (j + k0))) (VarSwap_in_ChannelData k0 c)
+        = VarSwap_in_ChannelData k0 (NewVar_in_ChannelData (S (S (j + k0))) c)).
+Proof.
+  destruct c.
+  + simpl. reflexivity.
+  + simpl. destruct (decide (n = k0)).
+    - subst. simpl. destruct (decide (j + k0 < k0)).
+      * rewrite decide_True; try lia.
+      * rewrite decide_False; try lia.
+        rewrite decide_False; try lia. simpl.
+        rewrite decide_True; try lia. eauto.
+    - simpl. destruct (decide ((n = S k0)%nat)); subst. 
+      * simpl. destruct (decide ((S (S (j + k0)) < S k0)%nat)); subst.
+        ++ rewrite decide_False; try lia.
+        ++ rewrite decide_False; try lia. simpl.
+           rewrite decide_False; try lia.
+           rewrite decide_True; try lia. eauto.
+      * destruct (decide (S (S (j + k0)) < S n)).
+        ++ simpl. rewrite decide_True; try lia.
+           destruct (decide ((S n = k0))).
+           ** subst. lia.
+           ** rewrite decide_False; try lia. eauto.
+        ++ simpl. rewrite decide_False; try lia.
+           rewrite decide_False; eauto.
+           rewrite decide_False; try lia. eauto.
+Qed.
+
+Lemma NewVarC_and_VarSwap j k0 p : (NewVarC (S (S (j + k0))) (VarSwap_in_proc k0 p) = VarSwap_in_proc k0 (NewVarC (S (S (j + k0))) p)).
+Proof.
+  revert j k0.
+  induction p as (p & Hp) using
+    (well_founded_induction (wf_inverse_image _ nat _ size Nat.lt_wf_0)).
+  destruct p; intros; simpl in *.
+  + assert (NewVarC (S (S (j + k0))) (VarSwap_in_proc k0 p1) = VarSwap_in_proc k0 (NewVarC (S (S (j + k0))) p1)) as eq1.
+    { eapply Hp. simpl. lia. }
+    assert (NewVarC (S (S (j + k0))) (VarSwap_in_proc k0 p2) = VarSwap_in_proc k0 (NewVarC (S (S (j + k0))) p2)) as eq2.
+    { eapply Hp. simpl. lia. }
+    rewrite eq1, eq2. eauto.
+  + reflexivity.
+  + assert (NewVarC (S (S (j + k0))) (VarSwap_in_proc k0 p) = VarSwap_in_proc k0 (NewVarC (S (S (j + k0))) p)) as eq.
+    { eapply Hp. simpl. lia. }
+    rewrite eq. eauto.
+  + assert (NewVarC (S (S (j + k0))) (VarSwap_in_proc k0 p1) = VarSwap_in_proc k0 (NewVarC (S (S (j + k0))) p1)) as eq1.
+    { eapply Hp. simpl. lia. }
+    assert (NewVarC (S (S (j + k0))) (VarSwap_in_proc k0 p2) = VarSwap_in_proc k0 (NewVarC (S (S (j + k0))) p2)) as eq2.
+    { eapply Hp. simpl. lia. }
+    rewrite eq1, eq2. eauto.
+  + rewrite NewVar_in_ChannelData_and_VarSwap_in_ChannelData. eauto.
+  + assert (S (S (S (j + k0))) = S (S (j + (S k0)))) as eq' by lia. rewrite eq'.
+    assert (NewVarC (S (S (j + (S k0)))) (VarSwap_in_proc (S k0) p)
+        = VarSwap_in_proc (S k0) (NewVarC (S (S (j + (S k0)))) p)) as eq.
+    { eapply Hp. simpl. lia. }
+    rewrite eq. eauto.
+  + destruct g0; simpl in *.
+    * reflexivity.
+    * reflexivity.
+    * assert (NewVarC (S (S (j + k0))) (VarSwap_in_proc k0 p) = VarSwap_in_proc k0 (NewVarC (S (S (j + k0))) p)) as eq1.
+      { eapply Hp. simpl. lia. } rewrite eq1.
+      rewrite NewVar_in_ChannelData_and_VarSwap_in_ChannelData. eauto.
+   * assert (NewVarC (S (S (j + k0))) (VarSwap_in_proc k0 p) = VarSwap_in_proc k0 (NewVarC (S (S (j + k0))) p)) as eq.
+     { eapply Hp. simpl. lia. }
+     rewrite eq. eauto.
+   * assert (NewVarC (S (S (j + k0))) (VarSwap_in_proc k0 (g g0_1)) = VarSwap_in_proc k0 (NewVarC (S (S (j + k0))) (g g0_1))) as eq1.
+     { eapply Hp. simpl. lia. }
+     assert (NewVarC (S (S (j + k0))) (VarSwap_in_proc k0 (g g0_2)) = VarSwap_in_proc k0 (NewVarC (S (S (j + k0))) (g g0_2))) as eq2.
+     { eapply Hp. simpl. lia. } simpl in *. inversion eq1. inversion eq2.
+     rewrite H0 , H1. eauto.
+Qed.
+
+Lemma NewVar_in_ChannelData_and_NewVar_in_ChannelData i j c :
+    NewVar_in_ChannelData (i + (S j)) (NewVar_in_ChannelData i c) 
+      = NewVar_in_ChannelData i (NewVar_in_ChannelData ( i + j ) c).
+Proof.
+  destruct c. simpl.
+  + eauto.
+  + simpl. destruct (decide ((i < S n))).
+    - simpl. destruct (decide (i + j < S n)).
+      * rewrite decide_True; try lia. simpl.
+        rewrite decide_True; try lia. eauto.
+      * rewrite decide_False; try lia. simpl.
+        rewrite decide_True; try lia. eauto.
+    - simpl. rewrite decide_False; try lia.
+      rewrite decide_False; try lia. simpl.
+      rewrite decide_False; try lia. eauto.
+Qed.
+
+Lemma NewVarC_and_NewVarC i j p : NewVarC (i + (S j)) (NewVarC i p) = NewVarC i (NewVarC ( i + j ) p).
+Proof.
+  revert i j.
+  induction p as (p & Hp) using
+    (well_founded_induction (wf_inverse_image _ nat _ size Nat.lt_wf_0)).
+  destruct p; intros; simpl in *.
+  + assert ((NewVarC (i + S j) (NewVarC i p1)) = (NewVarC i (NewVarC (i + j) p1))) as eq1.
+    { eapply Hp. simpl. lia. } rewrite eq1.
+    assert ((NewVarC (i + S j) (NewVarC i p2)) = (NewVarC i (NewVarC (i + j) p2))) as eq2.
+    { eapply Hp. simpl. lia. } rewrite eq2. eauto.
+  + eauto.
+  + assert ((NewVarC (i + S j) (NewVarC i p)) = (NewVarC i (NewVarC (i + j) p))) as eq.
+      { eapply Hp. simpl. eauto. } rewrite eq. eauto.
+  + assert ((NewVarC (i + S j) (NewVarC i p1)) = (NewVarC i (NewVarC (i + j) p1))) as eq1.
+    { eapply Hp. simpl. lia. } rewrite eq1.
+    assert ((NewVarC (i + S j) (NewVarC i p2)) = (NewVarC i (NewVarC (i + j) p2))) as eq2.
+    { eapply Hp. simpl. lia. } rewrite eq2. eauto.
+  + rewrite NewVar_in_ChannelData_and_NewVar_in_ChannelData. eauto.
+  + assert (NewVarC (S (i + S j)) (NewVarC (S i) p) = NewVarC (S i) (NewVarC (S (i + j)) p)) as eq.
+    { replace ((S (i + S j))) with ((S i) + S j)%nat; try lia.
+      replace (S (i + j)) with ((S i) + j)%nat; try lia. eapply Hp.
+      simpl. lia. } rewrite eq. eauto.
+  + destruct g0; simpl.
+    * eauto.
+    * eauto.
+    * rewrite NewVar_in_ChannelData_and_NewVar_in_ChannelData.
+      assert ((NewVarC (i + S j) (NewVarC i p)) = (NewVarC i (NewVarC (i + j) p))) as eq.
+      { eapply Hp. simpl. eauto. } rewrite eq. eauto.
+    * assert ((NewVarC (i + S j) (NewVarC i p)) = (NewVarC i (NewVarC (i + j) p))) as eq.
+      { eapply Hp. simpl. eauto. } rewrite eq. eauto.
+    * assert ((NewVarC (i + S j) (NewVarC i (g g0_1))) = (NewVarC i (NewVarC (i + j) (g g0_1)))) as eq1.
+      { eapply Hp. simpl. lia. } inversion eq1.
+      assert ((NewVarC (i + S j) (NewVarC i (g g0_2))) = (NewVarC i (NewVarC (i + j) (g g0_2)))) as eq2.
+      { eapply Hp. simpl. lia. } inversion eq2. eauto.
+Qed.
+
+Lemma NewVarC_Respects_Congruence : forall p p' j, p ≡* p' -> NewVarC j p ≡* NewVarC j p'.
+Proof.
+intros.  revert j.  dependent induction H.
+  - dependent induction H ; simpl ; auto with cgr.
+    * intros. replace j with (j + 0)%nat; eauto.
+      rewrite NewVarC_and_VarSwap. eapply cgr_res_swap.
+    * intros. replace j with (j + 0)%nat; eauto.
+      rewrite NewVarC_and_VarSwap. eapply cgr_res_swap_rev.
+    * intros. assert (NewVarC (0 + (S j)) (NewVarC 0 q) = NewVarC 0 (NewVarC ( 0 + j ) q)) as eq.
+      { rewrite NewVarC_and_NewVarC. eauto. }
+      simpl in *. rewrite eq. eapply cgr_res_scope.
+    * intros. assert (NewVarC (0 + (S j)) (NewVarC 0 q) = NewVarC 0 (NewVarC ( 0 + j ) q)) as eq.
+      { rewrite NewVarC_and_NewVarC. eauto. }
+      simpl in *. rewrite eq. eapply cgr_res_scope_rev.
+    * intros. eapply cgr_fullchoice; eauto. reflexivity.
+  - eauto with cgr.
 Qed.
 
 
@@ -628,6 +1147,7 @@ destruct p; intros; simpl.
     apply Hp. simpl. auto with arith. assumption. 
     apply Hp. simpl. auto with arith. assumption.  
   - eauto with cgr.
+  - eapply cgr_res. apply Hp. simpl. auto with arith. eapply NewVarC_Respects_Congruence. assumption.
   - destruct g0; simpl.
     * reflexivity.
     * reflexivity.
@@ -639,17 +1159,182 @@ destruct p; intros; simpl.
       auto. 
 Qed.
 
+Lemma VarSwap_NewVarC_in_ChannelData k c : NewVar_in_ChannelData k (NewVar_in_ChannelData k c) 
+  = VarSwap_in_ChannelData k (NewVar_in_ChannelData k (NewVar_in_ChannelData k c)).
+Proof.
+  destruct c; simpl.
+  + eauto.
+  + destruct (decide (k < S n)).
+    * simpl. rewrite decide_True; try lia.
+      simpl. rewrite decide_False; try lia.
+      rewrite decide_False; try lia. eauto.
+    * simpl. rewrite decide_False; try lia.
+      simpl. rewrite decide_False; try lia.
+      rewrite decide_False; try lia. eauto.
+Qed.
+
+Lemma VarSwap_NewVarC k q : NewVarC k (NewVarC k q) = VarSwap_in_proc k (NewVarC k (NewVarC k q)).
+Proof.
+  revert k.
+  induction q as (q & Hp) using
+    (well_founded_induction (wf_inverse_image _ nat _ size Nat.lt_wf_0)).
+  destruct q ; intros; simpl in *.
+  + assert (NewVarC k (NewVarC k q1) = VarSwap_in_proc k (NewVarC k (NewVarC k q1))) as eq1.
+    { eapply Hp. simpl. lia. }
+    assert (NewVarC k (NewVarC k q2) = VarSwap_in_proc k (NewVarC k (NewVarC k q2))) as eq2.
+    { eapply Hp. simpl. lia. }
+    rewrite eq1 at 1. rewrite eq2 at 1. eauto.
+  + eauto.
+  + assert (NewVarC k (NewVarC k q) = VarSwap_in_proc k (NewVarC k (NewVarC k q))) as eq.
+    { eapply Hp. simpl. lia. }
+    rewrite eq at 1. eauto.
+  + assert (NewVarC k (NewVarC k q1) = VarSwap_in_proc k (NewVarC k (NewVarC k q1))) as eq1.
+    { eapply Hp. simpl. lia. }
+    assert (NewVarC k (NewVarC k q2) = VarSwap_in_proc k (NewVarC k (NewVarC k q2))) as eq2.
+    { eapply Hp. simpl. lia. }
+    rewrite eq1 at 1. rewrite eq2 at 1. eauto.
+  + rewrite VarSwap_NewVarC_in_ChannelData at 1. eauto.
+  + assert (NewVarC (S k) (NewVarC (S k) q) = VarSwap_in_proc (S k) (NewVarC (S k) (NewVarC (S k) q))) as eq.
+    { eapply Hp. simpl. lia. }
+    rewrite eq at 1. eauto.
+  + destruct g0; simpl in *.
+    * eauto.
+    * eauto.
+    * assert (NewVarC k (NewVarC k p) = VarSwap_in_proc k (NewVarC k (NewVarC k p))) as eq.
+      { eapply Hp. simpl. lia. }
+      rewrite eq at 1. eauto. rewrite VarSwap_NewVarC_in_ChannelData at 1.
+      eauto.
+    * assert (NewVarC k (NewVarC k p) = VarSwap_in_proc k (NewVarC k (NewVarC k p))) as eq.
+      { eapply Hp. simpl. lia. }
+      rewrite eq at 1. eauto.
+    * assert (NewVarC k (NewVarC k (g g0_1)) = VarSwap_in_proc k (NewVarC k (NewVarC k (g g0_1)))) as eq1.
+      { eapply Hp. simpl. lia. }
+      assert (NewVarC k (NewVarC k (g g0_2)) = VarSwap_in_proc k (NewVarC k (NewVarC k (g g0_2)))) as eq2.
+      { eapply Hp. simpl. lia. } inversion eq1. inversion eq2. eauto.
+Qed.
+
+Lemma pr_subst_and_VarSwap n p0 k q : pr_subst n (VarSwap_in_proc k p0) (NewVarC k (NewVarC k q)) 
+      = VarSwap_in_proc k (pr_subst n p0 (NewVarC k (NewVarC k q))).
+Proof.
+  revert n k q.
+  induction p0 as (p0 & Hp) using
+    (well_founded_induction (wf_inverse_image _ nat _ size Nat.lt_wf_0)).
+  intros; destruct p0; simpl in *.
+  + assert (pr_subst n (VarSwap_in_proc k p0_1) (NewVarC k (NewVarC k q))
+       = VarSwap_in_proc k (pr_subst n p0_1 (NewVarC k (NewVarC k q)))) as eq1.
+    { eapply Hp. simpl. lia. }
+    assert (pr_subst n (VarSwap_in_proc k p0_2) (NewVarC k (NewVarC k q))
+       = VarSwap_in_proc k (pr_subst n p0_2 (NewVarC k (NewVarC k q)))) as eq2.
+    { eapply Hp. simpl. lia. }
+    rewrite eq1, eq2. eauto.
+  + destruct (decide (n = n0)); subst.
+    ++ simpl. rewrite VarSwap_NewVarC at 1. eauto.
+    ++ simpl. eauto.
+  + destruct (decide (n = n0)); subst.
+    ++ eauto.
+    ++ simpl. assert (pr_subst n (VarSwap_in_proc k p0) (NewVarC k (NewVarC k q)) 
+          = VarSwap_in_proc k (pr_subst n p0 (NewVarC k (NewVarC k q)))) as eq.
+       { eapply Hp. simpl. lia. }
+       rewrite eq. eauto.
+  + assert (pr_subst n (VarSwap_in_proc k p0_1) (NewVarC k (NewVarC k q))
+      = VarSwap_in_proc k (pr_subst n p0_1 (NewVarC k (NewVarC k q)))) as eq1.
+    { eapply Hp. simpl. lia. }
+    assert (pr_subst n (VarSwap_in_proc k p0_2) (NewVarC k (NewVarC k q))
+      = VarSwap_in_proc k (pr_subst n p0_2 (NewVarC k (NewVarC k q)))) as eq2.
+    { eapply Hp. simpl. lia. }
+    rewrite eq1, eq2. eauto.
+  + eauto.
+  + assert (NewVarC (0 + (S k)) (NewVarC 0 q) = NewVarC 0 (NewVarC ( 0 + k ) q)) as eq.
+    { rewrite NewVarC_and_NewVarC. eauto. }
+    assert (NewVarC (0 + (S k)) (NewVarC 0 (NewVarC k q)) = NewVarC 0 (NewVarC ( 0 + k ) (NewVarC k q))) as eq2.
+    { rewrite NewVarC_and_NewVarC. eauto. } simpl in *. rewrite<- eq2. rewrite<- eq.
+    assert (pr_subst n (VarSwap_in_proc (S k) p0) (NewVarC (S k) (NewVarC (S k) (NewVarC 0 q)))
+      = VarSwap_in_proc (S k) (pr_subst n p0 (NewVarC (S k) (NewVarC (S k) (NewVarC 0 q))))) as eq1.
+    { eapply Hp. simpl. lia. } rewrite eq1. eauto.
+  + destruct g0; simpl.
+    * eauto.
+    * eauto.
+    * rewrite NewVar_and_NewVarC. rewrite NewVar_and_NewVarC.
+      assert ((pr_subst n (VarSwap_in_proc k p) (NewVarC k (NewVarC k (NewVar 0 q))))
+        = (VarSwap_in_proc k (pr_subst n p (NewVarC k (NewVarC k (NewVar 0 q)))))) as eq1.
+      { eapply Hp. simpl. lia. } rewrite eq1. eauto.
+    * assert (pr_subst n (VarSwap_in_proc k p) (NewVarC k (NewVarC k q))
+        = VarSwap_in_proc k (pr_subst n p (NewVarC k (NewVarC k q)))) as eq1.
+      { eapply Hp. simpl. lia. } rewrite eq1. eauto.
+    * assert (pr_subst n (VarSwap_in_proc k (g g0_1)) (NewVarC k (NewVarC k q))
+        = VarSwap_in_proc k (pr_subst n (g g0_1) (NewVarC k (NewVarC k q)))) as eq1.
+      { eapply Hp. simpl. lia. }
+      assert (pr_subst n (VarSwap_in_proc k (g g0_2)) (NewVarC k (NewVarC k q))
+        = VarSwap_in_proc k (pr_subst n (g g0_2) (NewVarC k (NewVarC k q)))) as eq2.
+      { eapply Hp. simpl. lia. } inversion eq1. inversion eq2. eauto.
+Qed.
+
+Lemma pr_subst_and_NewVarC q0 q n k : (pr_subst n (NewVarC k q0) (NewVarC k q) = NewVarC k (pr_subst n q0 q)).
+Proof.
+  revert n k q.
+  induction q0 as (q0 & Hp) using
+    (well_founded_induction (wf_inverse_image _ nat _ size Nat.lt_wf_0)).
+  destruct q0; intros; simpl in *.
+  + assert (pr_subst n (NewVarC k q0_1) (NewVarC k q) = NewVarC k (pr_subst n q0_1 q)) as eq1.
+    { eapply Hp. simpl. lia. }
+    assert (pr_subst n (NewVarC k q0_2) (NewVarC k q) = NewVarC k (pr_subst n q0_2 q)) as eq2.
+    { eapply Hp. simpl. lia. }
+    rewrite eq1 , eq2. eauto.
+  + destruct (decide(n0 = n)).
+    - eauto.
+    - simpl. eauto.
+  + destruct (decide(n0 = n)).
+    - eauto.
+    - simpl. assert (pr_subst n0 (NewVarC k q0) (NewVarC k q) = NewVarC k (pr_subst n0 q0 q)) as eq.
+    { eapply Hp. simpl. lia. }
+    rewrite eq. eauto.
+  + assert (pr_subst n (NewVarC k q0_1) (NewVarC k q) = NewVarC k (pr_subst n q0_1 q)) as eq1.
+    { eapply Hp. simpl. lia. }
+    assert (pr_subst n (NewVarC k q0_2) (NewVarC k q) = NewVarC k (pr_subst n q0_2 q)) as eq2.
+    { eapply Hp. simpl. lia. }
+    rewrite eq1 , eq2. eauto.
+  + eauto.
+  + assert (NewVarC (0 + (S k)) (NewVarC 0 q) = NewVarC 0 (NewVarC ( 0 + k ) q)) as eq1.
+    { rewrite NewVarC_and_NewVarC. eauto. }
+    simpl in *. rewrite<- eq1.
+    assert (pr_subst n (NewVarC (S k) q0) (NewVarC (S k) (NewVarC 0 q))
+      = NewVarC (S k) (pr_subst n q0 (NewVarC 0 q))) as eq2.
+    { eapply Hp. simpl. lia. }
+    rewrite eq2. eauto.
+  + destruct g0; simpl in *.
+    * eauto.
+    * eauto.
+    * simpl. rewrite NewVar_and_NewVarC.
+      assert ((pr_subst n (NewVarC k p) (NewVarC k (NewVar 0 q))) = (NewVarC k (pr_subst n p (NewVar 0 q)))) as eq.
+      { eapply Hp. simpl. lia. }
+      rewrite eq. eauto.
+    * assert (pr_subst n (NewVarC k p) (NewVarC k q) = NewVarC k (pr_subst n p q)) as eq.
+      { eapply Hp. simpl. lia. }
+      rewrite eq. eauto.
+    * assert (pr_subst n (NewVarC k (g g0_1)) (NewVarC k q) = NewVarC k (pr_subst n (g g0_1) q)) as eq1.
+      { eapply Hp. simpl. lia. }
+      assert (pr_subst n (NewVarC k (g g0_2)) (NewVarC k q) = NewVarC k (pr_subst n (g g0_2) q)) as eq2.
+      { eapply Hp. simpl. lia. } inversion eq1. inversion eq2. eauto.
+Qed.
+
+
+
 (* ≡ respects the substitution of his variable*)
 Lemma cgr_step_subst2 : forall p p' q x, p ≡ p' → pr_subst x p q ≡ pr_subst x p' q.
 Proof.
   induction p as (p & Hp) using
     (well_founded_induction (wf_inverse_image _ nat _ size Nat.lt_wf_0)).
   intros p' q n hcgr ; inversion hcgr; try auto; try (exact H); try (now constructor).
+  - simpl. rewrite pr_subst_and_VarSwap. eapply cgr_res_swap_step.
+  - simpl. rewrite pr_subst_and_VarSwap. eapply cgr_res_swap_rev_step.
+  - simpl. rewrite pr_subst_and_NewVarC. eapply cgr_res_scope_step.
+  - simpl. rewrite pr_subst_and_NewVarC. eapply cgr_res_scope_rev_step.
   - simpl. destruct (decide (n = x)). auto. constructor. apply Hp. subst. simpl. auto.  exact H.
   - simpl. constructor. apply Hp. subst. simpl. auto. exact H.
   - simpl. constructor. apply Hp. subst. simpl. auto. exact H. 
   - simpl. constructor. apply Hp. subst. simpl. auto with arith. assumption. 
   - simpl. constructor. apply Hp. subst. simpl. auto with arith. assumption. 
+  - simpl. constructor. apply Hp. subst. simpl. auto with arith. assumption.
   - simpl. constructor. apply Hp. subst. simpl. auto with arith. assumption. 
   - simpl. apply cgr_choice_step. 
     assert (pr_subst n (g p1) q ≡ pr_subst n (g q1) q). apply Hp. subst. simpl. rewrite <-Nat.add_succ_r. 
@@ -696,6 +1381,12 @@ Inductive sts : proc -> proc -> Prop :=
     sts p1 p2 ->
     sts (p1 ‖ q) (p2 ‖ q)
 
+(* Restriction on Channel *)
+| sts_res : forall {p1 p2}, 
+    sts p1 p2 ->
+    sts (ν p1) (ν p2)
+
+
 (*The Congruence respects the Reduction *)
 | sts_cong : forall {p1 p2 q2 q1},
     p1 ≡* p2 -> sts p2 q2 -> q2 ≡* q1 -> sts p1 q1
@@ -703,80 +1394,176 @@ Inductive sts : proc -> proc -> Prop :=
 
 Hint Constructors sts:ccs.
 
+Fixpoint Ѵ (n : nat) (P : proc) : proc :=
+match n with 
+| 0 => P
+| S n => ν (Ѵ  n P)
+end.
+
+Fixpoint NewVarCn (k : nat) (n : nat) (P : proc) : proc :=
+match n with 
+| 0 => P
+| S n => NewVarC k (NewVarCn k n P)
+end.
+
+Fixpoint gNewVarCn (k : nat) (n : nat) (P : gproc) : gproc :=
+match n with 
+| 0 => P
+| S n => gNewVarC k (gNewVarCn k n P)
+end.
+
+Lemma cgr_res_n n P Q : P ≡* Q -> Ѵ  n P ≡* Ѵ  n Q.
+Proof.
+  revert P Q. induction n.
+  - intros; eauto.
+  - intros; simpl. eapply cgr_res. eauto.
+Qed.
+
+Lemma NewVarCn_revert_def n P k: NewVarCn k n (NewVarC k P) = NewVarC k (NewVarCn k n P).
+Proof.
+  revert P. induction n.
+  - reflexivity.
+  - intros; simpl in *. f_equal. eauto.
+Qed.
+
+Lemma VarC_add_zero c : VarC_add 0 c = c.
+Proof.
+  destruct c ; simpl ; eauto.
+Qed.
+
+
+Lemma VarC_add_revert_def k n c : VarC_add (k + n) c = (VarC_add k (VarC_add n c)).
+Proof.
+  revert n c. induction k; intros; simpl.
+  + destruct c; simpl; eauto.
+  + destruct c; simpl; eauto. f_equal. lia.
+Qed.
+
+Lemma cgr_res_scope_n n P Q : (Ѵ  n P) ‖ Q ≡* (Ѵ n (P ‖ NewVarCn 0 n Q)).
+Proof.
+  revert P Q.
+  dependent induction n.
+  - simpl. reflexivity.
+  - intros. simpl. etrans. eapply cgr_res_scope_rev. eapply cgr_res.
+    etrans. eapply IHn. eapply cgr_res_n. eapply cgr_fullpar. reflexivity.
+    rewrite NewVarCn_revert_def. reflexivity.
+Qed.
 
 (* For the (STS-reduction), the reductible terms and reducted terms are pretty all the same, up to ≡* *)
 Lemma ReductionShape : forall P Q, sts P Q ->
-((exists c v P2 G2 S, ((P ≡* ((c ! v • 𝟘) ‖ ((c ? x • P2) + G2)) ‖ S)) /\ (Q ≡*((𝟘 ‖ (P2^v)) ‖ S)))
-\/ (exists P1 G1 S, (P ≡* (((t • P1) + G1) ‖ S)) /\ (Q ≡* (P1 ‖ S)))
-\/ (exists n P1 S, (P ≡* ((rec n • P1) ‖ S)) /\ (Q ≡* (pr_subst n P1 (rec n • P1) ‖ S)))
+((exists c v P2 G2 S n , ((P ≡* Ѵ  n ((c ! v • 𝟘) ‖ ((c ? x • P2) + G2) ‖ S))) /\ (Q ≡* Ѵ  n ((𝟘 ‖ (P2^v)) ‖ S)))
+\/ (exists P1 G1 S n, (P ≡* Ѵ  n (((t • P1) + G1) ‖ S)) /\ (Q ≡* Ѵ  n (P1 ‖ S)))
+\/ (exists n P1 S n', (P ≡* Ѵ  n' ((rec n • P1) ‖ S)) /\ (Q ≡* Ѵ  n' (pr_subst n P1 (rec n • P1) ‖ S)))
 ).
 Proof.
-intros P Q Transition.
-induction Transition.
-  - left. exists c. exists v. exists p2. exists g2. exists (𝟘). split; apply cgr_par_nil_rev.
-  - right. left. exists p. exists g0. exists 𝟘. split; apply cgr_par_nil_rev.
-  - right. right. exists x. exists p. exists 𝟘. split; apply cgr_par_nil_rev.
-  - destruct IHTransition as [IH|[IH|IH]]. 
-    * decompose record IH. left. exists x. exists x0. exists x1. exists x2. exists (x3 ‖ q). split.
-        ** apply transitivity with ((((x ! x0 • 𝟘) ‖ ((x ? l • x1) + x2)) ‖ x3) ‖ q). apply cgr_par. auto. apply cgr_par_assoc.
-        ** apply transitivity with (((𝟘 ‖ x1^x0) ‖ x3) ‖ q). apply cgr_par. auto.  apply cgr_par_assoc. 
-    * decompose record IH. right. left. exists x. exists x0. exists (x1 ‖ q). split.
-        ** apply transitivity with (((t • x + x0) ‖ x1) ‖ q). apply cgr_par. auto. apply cgr_par_assoc.
-        ** apply transitivity with (x ‖ (x1) ‖ q). apply cgr_par. auto. apply cgr_par_assoc.
-    * decompose record IH. right. right. exists x. exists x0. exists (x1 ‖ q). split. 
-        ** apply transitivity with ((rec x • x0 ‖ x1) ‖ q). apply cgr_par. assumption. apply cgr_par_assoc.
-        ** apply transitivity with ((pr_subst x x0 (rec x • x0) ‖ x1) ‖ q). apply cgr_par. assumption. apply cgr_par_assoc.
-  - destruct IHTransition as [IH|[IH|IH]].  
-    * decompose record IH.
-      left. exists x. exists x0. exists x1. exists x2. exists x3.  split. apply cgr_trans with p2. exact H. exact H2.
-      apply cgr_trans with q2. apply cgr_symm. exact H0. exact H3.
-    * decompose record IH.
-      right. left. exists x. exists x0. exists x1. split. apply cgr_trans with p2. exact H. exact H2. apply cgr_trans with q2.
-      apply cgr_symm. apply H0. apply H3.
-    * decompose record IH. 
-      right. right. exists x. exists x0. exists x1. split. apply cgr_trans with p2. exact H. exact H2. apply cgr_trans with q2.
-      apply cgr_symm. apply H0. apply H3.
+  intros P Q Transition. induction Transition.
+  - left. exists c. exists v. exists p2.
+    exists g2. exists 𝟘. exists 0. split.
+    * simpl. etrans. eapply cgr_par_nil_rev. eapply cgr_fullpar; reflexivity.
+    * simpl. etrans. eapply cgr_par_nil_rev. eapply cgr_fullpar; reflexivity.
+  - right. left. exists p. exists g0. exists 𝟘. exists 0. split.
+    * simpl. eapply cgr_par_nil_rev.
+    * simpl. eapply cgr_par_nil_rev.
+  - right. right. exists x. exists p. exists 𝟘. exists 0. split.
+    * simpl. eapply cgr_par_nil_rev.
+    * simpl. eapply cgr_par_nil_rev.
+  - destruct IHTransition as [IH|[IH|IH]];  decompose record IH. 
+    * left. exists x. exists x0. exists x1. exists x2.
+      exists (x3 ‖ NewVarCn 0 x4 q). exists x4. split; simpl.
+      + etrans. apply cgr_par. eauto. etrans. eapply cgr_res_scope_n. eapply cgr_res_n. apply cgr_par_assoc.
+      + etrans. apply cgr_par. eauto. etrans. eapply cgr_res_scope_n. eapply cgr_res_n. apply cgr_par_assoc.
+    * right. left. exists x. exists x0. exists (x1 ‖ NewVarCn 0 x2 q). exists x2. split.
+      + apply transitivity with (Ѵ x2 ((t • x + x0) ‖ x1) ‖ q). apply cgr_par. auto. etrans.
+           eapply cgr_res_scope_n. eapply cgr_res_n. apply cgr_par_assoc.
+      + apply transitivity with (Ѵ x2 (x ‖ x1) ‖ q). apply cgr_par. auto. etrans.
+           eapply cgr_res_scope_n. eapply cgr_res_n. apply cgr_par_assoc.
+    * right. right. exists x. exists x0. exists (x1 ‖ NewVarCn 0 x2 q). exists x2. split. 
+      + apply transitivity with (Ѵ  x2 ((rec x • x0) ‖ x1) ‖ q). apply cgr_par. assumption.
+           etrans. eapply cgr_res_scope_n. eapply cgr_res_n. apply cgr_par_assoc.
+      + apply transitivity with (Ѵ  x2 (pr_subst x x0 (rec x • x0) ‖ x1) ‖ q). apply cgr_par. assumption. 
+           etrans. eapply cgr_res_scope_n. eapply cgr_res_n. apply cgr_par_assoc.
+  - destruct IHTransition as [IH|[IH|IH]]; decompose record IH. 
+    * left. exists x. exists x0. exists x1. exists x2. exists x3. exists (S x4). split.
+      + simpl. eapply cgr_res. eauto.
+      + simpl. eapply cgr_res. eauto.
+    * right. left. exists x. exists x0. exists x1. exists (S x2). split.
+      + simpl. eapply cgr_res. eauto.
+      + simpl. eapply cgr_res. eauto.
+    * right. right. exists x. exists x0. exists x1. exists (S x2). split.
+      + simpl. eapply cgr_res. eauto.
+      + simpl. eapply cgr_res. eauto.
+  - destruct IHTransition as [IH|[IH|IH]]; decompose record IH. 
+    * left. exists x. exists x0. exists x1. exists x2. exists x3. exists x4. split.
+      + apply cgr_trans with p2. exact H. exact H1.
+      + apply cgr_trans with q2. apply cgr_symm. exact H0. exact H3.
+    * right. left. exists x. exists x0. exists x1. exists x2. split.
+      + apply cgr_trans with p2. exact H. exact H1.
+      + apply cgr_trans with q2. apply cgr_symm. apply H0. apply H3.
+    * right. right. exists x. exists x0. exists x1. exists x2. split.
+      + apply cgr_trans with p2. exact H. exact H1.
+      + apply cgr_trans with q2. apply cgr_symm. apply H0. apply H3.
 Qed.
 
 (* For the (LTS-transition), the transitable terms and transitted terms, that performs a INPUT,
 are pretty all the same, up to ≡* *)
 Lemma TransitionShapeForInput : forall P Q c v, (lts P ((c ⋉ v) ?) Q) -> 
-(exists P1 G R, ((P ≡* ((c ? x • P1 + G) ‖ R)) /\ (Q ≡* (P1^v ‖ R)) /\ ((exists L,P = (g L)) -> R = 𝟘))).
+(exists P1 G R n, ((P ≡* Ѵ  n (((VarC_add n c) ? x • P1 + G) ‖ R)) /\ (Q ≡* Ѵ  n (P1^v ‖ R))
+  /\ ((exists L,P = (g L)) -> R = 𝟘 /\ n = 0))).
 Proof.
 intros P Q c v Transition.
  dependent induction Transition.
-- exists P. exists 𝟘. exists 𝟘. split ; try split.
-  * apply cgr_trans with ((c ? x • P) + 𝟘). apply cgr_trans with (c ? x • P). apply cgr_refl. apply cgr_choice_nil_rev. apply cgr_par_nil_rev.
+- exists P. exists 𝟘. exists 𝟘. exists 0. repeat split.
+  * simpl. destruct c.
+    + simpl. apply cgr_trans with ((c ? x • P) + 𝟘). apply cgr_trans with (c ? x • P).
+      apply cgr_refl. apply cgr_choice_nil_rev. apply cgr_par_nil_rev.
+    + simpl. apply cgr_trans with (((bvarC n) ? x • P) + 𝟘). apply cgr_trans with ((bvarC n) ? x • P).
+      apply cgr_refl. apply cgr_choice_nil_rev. apply cgr_par_nil_rev.
   * apply cgr_par_nil_rev.
-  * reflexivity.
-- destruct (IHTransition c v). reflexivity. decompose record H0. exists x. exists x0. exists x1. split; try split.
-  * apply cgr_trans with p. apply cgr_if_true. assumption. assumption.
+- destruct (IHTransition c v). reflexivity. decompose record H0.
+  exists x. exists x0. exists x1. exists x2. split; try split.
+  * apply cgr_trans with p. apply cgr_if_true. assumption. simpl. assumption.
   * assumption.
   * intros. inversion H3. inversion H5.
-- destruct (IHTransition c v). reflexivity. decompose record H0. exists x. exists x0. exists x1. split; try split.
+- destruct (IHTransition c v). reflexivity. decompose record H0.
+  exists x. exists x0. exists x1. exists x2. split; try split.
   * apply cgr_trans with q. apply cgr_if_false. assumption. assumption.
   * assumption.
   * intros. inversion H3. inversion H5.
-- edestruct IHTransition;eauto. decompose record H. exists x. exists x0. exists (x1 ‖ q). split; try split.
-  * apply cgr_trans with ((((c ? l • x) + x0) ‖ x1) ‖ q). apply cgr_par. assumption. apply cgr_par_assoc.
-  * apply cgr_trans with ((x^v ‖ x1) ‖ q). apply cgr_par. assumption. apply cgr_par_assoc.
+- destruct (IHTransition (VarC_add 1 c) v). reflexivity. decompose record H. exists x. exists x0.
+  exists x1. exists (S x2). repeat split.
+  * simpl. eapply cgr_res. rewrite<- VarC_add_revert_def in H1.
+    replace (S x2)%nat with (x2 + 1)%nat by lia. exact H1.
+  * simpl. eapply cgr_res. exact H0.
   * intros. inversion H2. inversion H4.
-- edestruct IHTransition;eauto. decompose record H. exists x. exists x0. exists (x1 ‖ p). split; try split.
-  * apply cgr_trans with ((((c ? l • x) + x0) ‖ x1) ‖ p). apply cgr_trans with (q1 ‖ p). apply cgr_par_com. apply cgr_par. assumption. apply cgr_par_assoc.
-  * apply cgr_trans with ((x^v ‖ x1) ‖ p). apply cgr_trans with (q2 ‖ p). apply cgr_par_com. apply cgr_par. assumption. apply cgr_par_assoc.
   * intros. inversion H2. inversion H4.
-- edestruct IHTransition; eauto. decompose record H. exists x. exists (x0 + p2). exists 𝟘. split ; try split.
-  * apply cgr_trans with ((c ? l • x) + (x0 + p2)). apply cgr_trans with (((c ? l • x) + x0) + p2).
-    apply cgr_choice. assert (x1 = 𝟘). apply H3. exists p1. reflexivity. rewrite H2 in H0. apply transitivity with (((c ? l • x) + x0) ‖ 𝟘).
-    assumption. apply cgr_par_nil. apply cgr_choice_assoc. apply cgr_par_nil_rev.
-  * assert (x1 = 𝟘). apply H3. exists p1. reflexivity. rewrite H2 in H1. assumption.
-  * reflexivity.
-- edestruct IHTransition; eauto. decompose record H. exists x. exists (x0 + p1). exists 𝟘. split; try split.
-  * apply cgr_trans with ((c ? l • x) + (x0 + p1)). apply cgr_trans with (((c ? l • x) + x0) + p1).
-    apply cgr_trans with (p2 + p1). apply cgr_choice_com. apply cgr_choice. assert (x1 = 𝟘). apply H3. exists p2. reflexivity.
-    apply cgr_trans with (((c ? l • x) + x0) ‖ x1). assumption. rewrite H2. apply cgr_par_nil. apply cgr_choice_assoc. apply cgr_par_nil_rev.
-  * assert (x1 = 𝟘). apply H3. exists p2. reflexivity. rewrite <-H2. assumption. 
-  * reflexivity.
+- destruct (IHTransition c v). reflexivity. decompose record H. exists x. exists x0.
+  exists (x1 ‖ NewVarCn 0 x2 q). exists x2. repeat split.
+  * apply cgr_trans with (Ѵ x2 ((((VarC_add x2 c) ? l • x) + x0) ‖ x1) ‖ q). apply cgr_par. assumption.
+    etrans. eapply cgr_res_scope_n. eapply cgr_res_n. apply cgr_par_assoc.
+  * apply cgr_trans with (Ѵ x2 (x^v ‖ x1) ‖ q). apply cgr_par. assumption. etrans.
+    eapply cgr_res_scope_n. eapply cgr_res_n. apply cgr_par_assoc.
+  * intros. inversion H2. inversion H4.
+  * intros. inversion H2. inversion H4.
+- destruct (IHTransition c v). reflexivity. decompose record H. exists x. exists x0. exists (x1 ‖ NewVarCn 0 x2 p). exists x2. repeat split.
+  * apply cgr_trans with (Ѵ x2 ((((VarC_add x2 c) ? l • x) + x0) ‖ x1) ‖ p). apply cgr_trans with (q1 ‖ p).
+    apply cgr_par_com. apply cgr_par. assumption. etrans. eapply cgr_res_scope_n. eapply cgr_res_n. apply cgr_par_assoc.
+  * apply cgr_trans with (Ѵ x2 (x^v ‖ x1) ‖ p). apply cgr_trans with (q2 ‖ p). apply cgr_par_com. apply cgr_par. assumption.
+    etrans. eapply cgr_res_scope_n. eapply cgr_res_n. apply cgr_par_assoc.
+  * intros. inversion H2. inversion H4.
+  * intros. inversion H2. inversion H4.
+- destruct (IHTransition c v). reflexivity. decompose record H. exists x. exists (x0 + p2). exists 𝟘. exists 0. repeat split.
+  * simpl. apply cgr_trans with ((c ? v • x) + (x0 + p2)). apply cgr_trans with (((c ? v • x) + x0) + p2).
+    apply cgr_choice. assert (x1 = 𝟘 ∧ x2 = 0) as (eq1 & eq2). apply H3. exists p1. reflexivity. subst.
+    apply transitivity with (((c ? v • x) + x0) ‖ 𝟘). simpl in *. rewrite VarC_add_zero in H1. eauto.
+    apply cgr_par_nil. apply cgr_choice_assoc. rewrite VarC_add_zero. apply cgr_par_nil_rev.
+  * simpl. assert (x1 = 𝟘 ∧ x2 = 0) as (eq1 & eq2). apply H3. exists p1. reflexivity. subst. simpl in *. assumption.
+- destruct (IHTransition c v). reflexivity. decompose record H. exists x. exists (x0 + p1). exists 𝟘. exists 0. repeat split.
+  * simpl. apply cgr_trans with ((c ? v • x) + (x0 + p1)). apply cgr_trans with (((c ? v • x) + x0) + p1).
+    etrans. eapply cgr_choice_com. apply cgr_choice. assert (x1 = 𝟘 ∧ x2 = 0) as (eq1 & eq2).
+    apply H3. exists p2. reflexivity. subst.
+    apply transitivity with (((c ? v • x) + x0) ‖ 𝟘). simpl in *. rewrite VarC_add_zero in H1. eauto.
+    apply cgr_par_nil. apply cgr_choice_assoc. rewrite VarC_add_zero. apply cgr_par_nil_rev.
+  * simpl. assert (x1 = 𝟘 ∧ x2 = 0) as (eq1 & eq2). apply H3. exists p2. reflexivity. subst. simpl in *. assumption.
 Qed.
 
 
@@ -787,39 +1574,101 @@ Proof. intros. intro l. dependent induction l;eapply IHl; eauto. Defined.
 (* For the (LTS-transition), the transitable terms and transitted terms, that performs a OUPUT,
 are pretty all the same, up to ≡* *)
 Lemma TransitionShapeForOutput : forall P Q c v, (lts P ((c ⋉ v) !) Q) -> 
-(exists R, (P ≡* ((c ! v • 𝟘) ‖ R) /\ (Q ≡* (𝟘 ‖ R)))).
+(exists R n, (P ≡* (Ѵ  n (((VarC_add n c) ! v • 𝟘) ‖ R)) /\ (Q ≡* Ѵ  n (𝟘 ‖ R)))).
 Proof.
 intros P Q c v Transition.
  dependent induction Transition.
-- exists 𝟘. split.
+- exists 𝟘. exists 0. split; simpl; try rewrite VarC_add_zero.
   * apply cgr_par_nil_rev.
   * apply cgr_par_nil_rev.
-- destruct (IHTransition c v). reflexivity. decompose record H0. exists x. split; try split.
+- destruct (IHTransition c v). reflexivity. decompose record H0. exists x. exists x0. split; try split.
   * apply cgr_trans with p. apply cgr_if_true. assumption. assumption.
   * assumption.
-- destruct (IHTransition c v). reflexivity. decompose record H0. exists x. split; try split.
+- destruct (IHTransition c v). reflexivity. decompose record H0. exists x. exists x0. split; try split.
   * apply cgr_trans with q. apply cgr_if_false. assumption. assumption.
   * assumption.
-- edestruct IHTransition;eauto. decompose record H. exists (x ‖ q). split.
-  * apply cgr_trans with (((c ! v • 𝟘) ‖ x) ‖ q). apply cgr_par. assumption. apply cgr_par_assoc.
-  * apply cgr_trans with ((𝟘 ‖ x) ‖ q). apply cgr_par. assumption. apply cgr_par_assoc.
-- edestruct IHTransition; eauto. decompose record H. exists (x ‖ p). split.
-  * apply cgr_trans with (((c ! v • 𝟘) ‖ x) ‖ p). apply cgr_trans with (q1 ‖ p). apply cgr_par_com. apply cgr_par. assumption. apply cgr_par_assoc.
-  * apply cgr_trans with ((𝟘 ‖ x) ‖ p). apply cgr_trans with (q2 ‖ p). apply cgr_par_com. apply cgr_par. assumption. apply cgr_par_assoc.
+- destruct (IHTransition (VarC_add 1 c) v). reflexivity. decompose record H. exists x.
+  exists (S x0). repeat split.
+  * simpl. eapply cgr_res. rewrite<- VarC_add_revert_def in H1.
+    replace (S x0)%nat with (x0 + 1)%nat by lia. exact H1.
+  * simpl. eapply cgr_res. exact H2.
+- edestruct IHTransition;eauto. decompose record H. exists (x ‖ NewVarCn 0 x0 q). exists x0. split.
+  * etrans. apply cgr_par. eassumption. etrans. eapply cgr_res_scope_n. eapply cgr_res_n. apply cgr_par_assoc.
+  * etrans. apply cgr_par. eassumption. etrans. eapply cgr_res_scope_n. eapply cgr_res_n. apply cgr_par_assoc.
+- edestruct IHTransition; eauto. decompose record H. exists (x ‖ NewVarCn 0 x0 p). exists x0. split.
+  * etrans. eapply cgr_par_com. etrans. eapply cgr_par. eassumption. etrans. eapply cgr_res_scope_n.
+    eapply cgr_res_n. apply cgr_par_assoc.
+  * etrans. eapply cgr_par_com. etrans. eapply cgr_par. eassumption. etrans. eapply cgr_res_scope_n.
+    eapply cgr_res_n. apply cgr_par_assoc.
 - edestruct guarded_does_no_output. subst. eauto.
 - edestruct guarded_does_no_output. subst. eauto.
 Qed.
 
+Lemma BigNew_reverse_def_one j p : (Ѵ j (ν p)) = ν (Ѵ j p).
+Proof.
+  revert p.
+  induction j.
+  - intros. simpl. eauto.
+  - intros. simpl. rewrite IHj. eauto.
+Qed.
+
+Lemma BigNew_reverse_def k j p : Ѵ k (Ѵ j p) = Ѵ j (Ѵ k p).
+Proof.
+  revert j p.
+  induction k.
+  - intros; simpl; eauto.
+  - intros; simpl in *. replace ((ν Ѵ k p)) with (Ѵ 1 (Ѵ k p)); eauto.
+    rewrite<- (IHk 1) at 1. simpl. rewrite<- IHk. replace ((ν Ѵ k (Ѵ j p))) with (Ѵ 1 (Ѵ k (Ѵ j p))); eauto.
+    rewrite<- (IHk 1). f_equal. simpl. rewrite BigNew_reverse_def_one. eauto.
+Qed.
+
+Lemma VarC_add_zero_ext μ : VarC_action_add 0 μ = μ.
+Proof.
+  destruct μ; destruct a; destruct c; simpl; eauto.
+Qed.
+
+Lemma NewVarCzero_and_add_Channel c : VarC_add 1 c = NewVar_in_ChannelData 0 c.
+Proof.
+  destruct c; simpl ;eauto.
+Qed.
+
+Lemma NewVarCzero_and_add μ : VarC_action_add 1 μ = NewVarC_in_ext 0 μ.
+Proof.
+  destruct μ; destruct a; simpl; rewrite NewVarCzero_and_add_Channel; eauto.
+Qed.
+
+Lemma NewVarC_and_NewVarC_in_ChannelData k j μ :
+      NewVarC_in_ext j (NewVarC_in_ext (j + k) μ) = NewVarC_in_ext (j + (S k)) (NewVarC_in_ext j μ).
+Proof.
+  destruct μ; destruct a; simpl; rewrite NewVar_in_ChannelData_and_NewVar_in_ChannelData; eauto.
+Qed.
+
+Lemma inversion_res_n_lts k e1 μ e1' : lts (Ѵ k e1) (ActExt μ) e1' -> exists e'1, e1' = (Ѵ k e'1).
+Proof.
+  revert e1 μ e1'.
+  induction k.
+  + simpl; eauto.
+  + intros; simpl in *. inversion H; subst. eapply IHk in H2 as (e'' & eq).
+    subst. exists e''. eauto.
+Qed.
+
+Lemma inversion_res_ext k e1 μ e1' : lts (Ѵ k e1) (ActExt μ) (Ѵ k e1') -> lts e1 (ActExt (VarC_action_add k μ)) e1'.
+Proof.
+  revert e1 μ e1'.
+  induction k.
+  + simpl; eauto. intros. rewrite VarC_add_zero_ext. eauto.
+  + intros; simpl in *. inversion H; subst. eapply IHk in H3.
+    rewrite VarC_action_add_add in H3. replace (S k) with (k+1)%nat by lia.
+    eauto.
+Qed.
+
 
 Lemma TransitionShapeForOutputSimplified : forall P Q c v, (lts P ((c ⋉ v) !) Q) 
-                                        -> (P ≡* ((c ! v • 𝟘) ‖ Q)).
+                                        -> exists n,(P ≡* ((Ѵ  n ((VarC_add n c) ! v • 𝟘))) ‖ Q).
 Proof.
-intros. assert ((exists R, (P ≡* ((c ! v • 𝟘) ‖ R) /\ (Q ≡* (𝟘 ‖ R))))). apply TransitionShapeForOutput. assumption.
-decompose record H0. apply transitivity with (((c ! v • 𝟘) ‖ x) ‖ 𝟘). apply transitivity with ((c ! v • 𝟘) ‖ x).
-assumption. auto with cgr. apply transitivity with ((c ! v • 𝟘) ‖ (x ‖ 𝟘)). auto with cgr. apply cgr_fullpar. auto with cgr.
-eauto with cgr. 
-Qed. 
-
+intros. assert (exists R n, (P ≡* Ѵ  n (((VarC_add n c) ! v • 𝟘) ‖ R)) /\ (Q ≡* Ѵ  n (𝟘 ‖ R))). apply TransitionShapeForOutput. assumption.
+decompose record H0. exists x0. etrans. eassumption. admit.
+Admitted.
 
 (* For the (LTS-transition), the transitable Guards and transitted terms, that performs a Tau ,
 are pretty all the same, up to ≡* *)
@@ -838,6 +1687,7 @@ destruct Hyp. rename H into Transition. dependent induction Transition.
 - inversion H0. inversion H.
 - inversion H0. inversion H.
 - inversion H0. inversion H.
+- inversion H0. inversion H.
 - edestruct IHTransition. reflexivity. exists p1. reflexivity. destruct H. destruct H.  exists x. 
   exists (x0 + p2). split. apply cgr_trans with (((t • x) + x0) + p2).
   apply cgr_choice. assumption.
@@ -852,6 +1702,688 @@ Definition sc_then_lts p α q := exists r, p ≡* r /\ (lts r α q).
 
 (* p performs α to some r and this is equivalent to q*)
 Definition lts_then_sc p α q := exists r, ((lts p α r) /\ r ≡* q).
+
+Lemma Swap_Swap_Chan k c : VarSwap_in_ChannelData k (VarSwap_in_ChannelData k c) = c.
+Proof.
+  destruct c; simpl; eauto.
+  destruct (decide (n = k)).
+  + simpl. rewrite decide_False; try lia. subst.
+    rewrite decide_True; try lia. eauto.
+  + destruct (decide (n = S k)).
+    * subst. simpl. rewrite decide_True; try lia. eauto.
+    * simpl. rewrite decide_False; try lia.
+      rewrite decide_False; try lia. eauto.
+Qed.
+
+Lemma Swap_Swap k p : VarSwap_in_proc k (VarSwap_in_proc k p) = p.
+Proof.
+  revert k.
+  induction p as (p & Hp) using
+    (well_founded_induction (wf_inverse_image _ nat _ size Nat.lt_wf_0)).
+  destruct p; intros ; simpl in *.
+  * assert (VarSwap_in_proc k (VarSwap_in_proc k p1) = p1) as eq1.
+    { eapply Hp. simpl. lia. }
+    assert (VarSwap_in_proc k (VarSwap_in_proc k p2) = p2) as eq2.
+    { eapply Hp. simpl. lia. }
+    rewrite eq1, eq2. eauto.
+  * eauto.
+  * assert (VarSwap_in_proc k (VarSwap_in_proc k p) = p) as eq.
+    { eapply Hp. simpl. lia. }
+    rewrite eq. eauto.
+  * assert (VarSwap_in_proc k (VarSwap_in_proc k p1) = p1) as eq1.
+    { eapply Hp. simpl. lia. }
+    assert (VarSwap_in_proc k (VarSwap_in_proc k p2) = p2) as eq2.
+    { eapply Hp. simpl. lia. }
+    rewrite eq1, eq2. eauto.
+  * rewrite Swap_Swap_Chan. eauto.
+  * assert (VarSwap_in_proc (S k) (VarSwap_in_proc (S k) p) = p) as eq.
+    { eapply Hp. simpl. lia. }
+    rewrite eq. eauto.
+  * destruct g0; simpl in *.
+    + eauto.
+    + eauto.
+    + rewrite Swap_Swap_Chan.
+      assert (VarSwap_in_proc k (VarSwap_in_proc k p) = p) as eq.
+      { eapply Hp. simpl. lia. }
+      rewrite eq. eauto.
+    + assert (VarSwap_in_proc k (VarSwap_in_proc k p) = p) as eq.
+      { eapply Hp. simpl. lia. }
+      rewrite eq. eauto.
+    + assert (VarSwap_in_proc k (VarSwap_in_proc k (g g0_1)) = (g g0_1)) as eq1.
+      { eapply Hp. simpl. lia. }
+      assert (VarSwap_in_proc k (VarSwap_in_proc k (g g0_2)) = (g g0_2)) as eq2.
+      { eapply Hp. simpl. lia. }
+      inversion eq1. inversion eq2. rewrite H0. rewrite H1. rewrite H0. rewrite H1. eauto.
+Qed.
+
+Lemma VarSwap_swap_proc p p' μ k : lts (VarSwap_in_proc k p) (ActExt (VarC_action_add (S (S k)) μ)) p' -> 
+lts p (ActExt (VarC_action_add (S (S k)) μ)) (VarSwap_in_proc k p').
+Proof.
+  revert p' μ k.
+  induction p as (p & Hp) using
+    (well_founded_induction (wf_inverse_image _ nat _ size Nat.lt_wf_0)).
+  destruct p; intros; simpl in *.
+  + dependent destruction H.
+    * simpl. rewrite Swap_Swap. eapply lts_parL. eapply Hp. simpl. lia. eauto.
+    * simpl. rewrite Swap_Swap. eapply lts_parR. eapply Hp. simpl. lia. eauto.
+  + inversion H.
+  + inversion H.
+  + dependent destruction H.
+    * simpl. eapply lts_ifOne; eauto. eapply Hp. simpl. lia. eauto.
+    * simpl. eapply lts_ifZero; eauto. eapply Hp. simpl. lia. eauto.
+  + destruct c.
+      - simpl in *. inversion H; subst. simpl. constructor.
+      - simpl in *. destruct (decide (n = k)).
+        ++ subst. inversion H; subst. destruct μ. 
+           ++++ destruct a. simpl in *. inversion H3.
+           ++++ destruct a. simpl in *. inversion H3. subst. destruct c.
+                +++++ simpl in *. inversion H1.
+                +++++ simpl in *. destruct n. 
+                      ++++++ inversion H1. lia.
+                      ++++++ inversion H1. lia.
+        ++ destruct (decide (n = S k)).
+           ++++ subst. inversion H; subst. destruct μ.
+                +++++ destruct a. simpl in *. inversion H3.
+                +++++ destruct a. simpl in *. inversion H3. subst. destruct c.
+                      ++++++ inversion H1.
+                      ++++++ inversion H1. lia.
+           ++++ inversion H; subst. simpl. eapply lts_output.
+  + dependent destruction H. rewrite VarC_action_add_add in H. simpl in H.
+    eapply Hp in H; simpl ; try lia. replace (S (S (S k)))%nat with (1 + (S (S k)))%nat in H by lia.
+    rewrite<- VarC_action_add_add in H. eapply lts_res_ext in H. eauto. 
+  + destruct g0.
+    * inversion H.
+    * inversion H.
+    * simpl in *. destruct c.
+      - simpl in *. inversion H; subst. rewrite<- subst_and_VarSwap. rewrite Swap_Swap. eapply lts_input.
+      - simpl in *. destruct (decide (n = k)).
+        ++ subst. inversion H; subst. destruct μ. 
+           ++++ destruct a. simpl in *. inversion H3. subst. destruct c.
+                +++++ simpl in *. inversion H1.
+                +++++ simpl in *. destruct n. 
+                      ++++++ inversion H3. lia.
+                      ++++++ inversion H1. lia.
+           ++++ destruct a. simpl in *. inversion H3.
+        ++ destruct (decide (n = S k)).
+           ++++ subst. inversion H; subst. destruct μ. 
+                +++++ destruct a. simpl in *. inversion H3. subst. destruct c.
+                      ++++++ inversion H3.
+                      ++++++ inversion H1. lia.
+                +++++ destruct a. simpl in *. inversion H3.
+           ++++ inversion H; subst. rewrite<- subst_and_VarSwap. rewrite Swap_Swap. eapply lts_input.
+    * inversion H.
+    * dependent destruction H.
+      - simpl. eapply lts_choiceL. eapply Hp. simpl. lia. eauto.
+      - simpl. eapply lts_choiceR. eapply Hp. simpl. lia. eauto.
+Qed.
+
+Lemma VarC_action_add_Swap k μ : 
+      (VarC_action_add 1 (VarSwap_in_ext k μ) = VarSwap_in_ext (S k) (VarC_action_add 1 μ)).
+Proof.
+  destruct μ; destruct a; destruct c; simpl in *.
+  + eauto.
+  + destruct (decide (n = k)).
+    - subst. rewrite decide_True; eauto.
+    - destruct (decide (n = S k)); subst.
+      ++ rewrite decide_False; eauto.
+         rewrite decide_True; eauto.
+      ++ rewrite decide_False; eauto.
+         rewrite decide_False; eauto.
+  + eauto.
+  + destruct (decide (n = k)).
+    - subst. rewrite decide_True; eauto.
+    - destruct (decide (n = S k)); subst.
+      ++ rewrite decide_False; eauto.
+         rewrite decide_True; eauto.
+      ++ rewrite decide_False; eauto.
+         rewrite decide_False; eauto.
+Qed.
+
+Lemma VarSwap_swap2_proc p p' μ k : lts (VarSwap_in_proc k p) (ActExt μ) p' -> 
+lts p (ActExt (VarSwap_in_ext k μ)) (VarSwap_in_proc k p').
+Proof.
+  revert p' μ k.
+  induction p as (p & Hp) using
+    (well_founded_induction (wf_inverse_image _ nat _ size Nat.lt_wf_0)).
+  destruct p; intros; simpl in *.
+  + dependent destruction H.
+    * simpl. rewrite Swap_Swap. eapply lts_parL. eapply Hp. simpl. lia. eauto.
+    * simpl. rewrite Swap_Swap. eapply lts_parR. eapply Hp. simpl. lia. eauto.
+  + inversion H.
+  + inversion H.
+  + dependent destruction H.
+    * simpl. eapply lts_ifOne; eauto. eapply Hp. simpl. lia. eauto.
+    * simpl. eapply lts_ifZero; eauto. eapply Hp. simpl. lia. eauto.
+  + destruct c.
+      - simpl in *. inversion H; subst. eapply lts_output.
+      - simpl in *. destruct (decide (n = k)).
+        ++ subst. inversion H; subst. simpl. rewrite decide_False; try lia. rewrite decide_True; try lia.
+           constructor.
+        ++ destruct (decide (n = S k)).
+           ++++ subst. inversion H; subst. simpl in *. rewrite decide_True; try lia.
+                eapply lts_output.
+           ++++ inversion H; subst. simpl in *.
+                rewrite decide_False; try lia. rewrite decide_False; try lia. eapply lts_output.
+  + dependent destruction H. simpl in *. eapply Hp in H; try lia.
+    eapply lts_res_ext. rewrite VarC_action_add_Swap. eauto.
+  + destruct g0.
+    * inversion H.
+    * inversion H.
+    * simpl in *. destruct c.
+      - simpl in *. inversion H; subst. rewrite<- subst_and_VarSwap. rewrite Swap_Swap. eapply lts_input.
+      - simpl in *. destruct (decide (n = k)).
+        ++ subst. inversion H; subst. rewrite<- subst_and_VarSwap. rewrite Swap_Swap.
+           simpl in *. rewrite decide_False; try lia. rewrite decide_True; try lia. eapply lts_input.
+        ++ destruct (decide (n = S k)).
+           ++++ subst. inversion H; subst. simpl in *. rewrite decide_True; try lia.
+                rewrite<- subst_and_VarSwap. rewrite Swap_Swap. eapply lts_input.
+           ++++ inversion H; subst. rewrite<- subst_and_VarSwap. rewrite Swap_Swap. simpl in *.
+                rewrite decide_False; try lia. rewrite decide_False; try lia. eapply lts_input.
+    * inversion H.
+    * dependent destruction H.
+      - simpl. eapply lts_choiceL. eapply Hp. simpl. lia. eauto.
+      - simpl. eapply lts_choiceR. eapply Hp. simpl. lia. eauto.
+Qed.
+
+Lemma NewVarC_preserves_transition k p μ q :
+  lts p (ActExt μ) q -> lts (NewVarC k p) (ActExt (NewVarC_in_ext k μ)) (NewVarC k q).
+Proof.
+  revert k μ q. induction p as (p & Hp) using
+    (well_founded_induction (wf_inverse_image _ nat _ size Nat.lt_wf_0)).
+  destruct p; simpl in *; intros.
+  + inversion H; subst; simpl in *.
+    - eapply lts_parL. eapply Hp; eauto. simpl. lia.
+    - eapply lts_parR. eapply Hp; eauto. simpl. lia.
+  + inversion H.
+  + inversion H.
+  + inversion H; subst; simpl in *.
+    * eapply lts_ifOne; eauto. eapply Hp; eauto. simpl. lia.
+    * eapply lts_ifZero; eauto. eapply Hp; eauto. simpl. lia.
+  + inversion H; subst. simpl. eapply lts_output.
+  + inversion H; subst; simpl in *.
+    eapply lts_res_ext. rewrite NewVarCzero_and_add.
+    assert (k = (0 + k))%nat as eq by lia. rewrite eq at 2.
+    rewrite NewVarC_and_NewVarC_in_ChannelData. simpl. eapply Hp. lia. eauto.
+  + destruct g0; simpl in *.
+    * inversion H.
+    * inversion H.
+    * inversion H; subst. simpl. rewrite<- subst_and_NewVarC. eapply lts_input.
+    * inversion H.
+    * inversion H; subst; simpl in *.
+      - eapply lts_choiceL. eapply Hp in H4; simpl; try lia. eauto.
+      - eapply lts_choiceR. eapply Hp in H4; simpl; try lia. eauto.
+Qed.
+
+Lemma NewVarCn_preserves_transition k q μ q2 :
+  lts q (ActExt μ) q2 -> lts (NewVarCn 0 k q) (ActExt (VarC_action_add k μ)) (NewVarCn 0 k q2).
+Proof.
+  revert μ q2 q. induction k.
+  + intros. simpl; rewrite VarC_add_zero_ext. eauto.
+  + intros; simpl in *. replace (S k)%nat with (1 + k)%nat; try lia.
+    rewrite<- VarC_action_add_add. rewrite NewVarCzero_and_add. eapply NewVarC_preserves_transition.
+    eapply IHk. eauto.
+Qed.
+
+Lemma NewVarC_preserves_reduction k p q :
+  lts p τ q -> lts (NewVarC k p) τ (NewVarC k q).
+Proof.
+  revert k q. induction p as (p & Hp) using
+    (well_founded_induction (wf_inverse_image _ nat _ size Nat.lt_wf_0)).
+  destruct p; simpl in *; intros.
+  + inversion H; subst; simpl in *.
+    - eapply NewVarC_preserves_transition in H2.
+      eapply NewVarC_preserves_transition in H3.
+      eapply lts_comL; eauto.
+    - eapply NewVarC_preserves_transition in H2.
+      eapply NewVarC_preserves_transition in H3.
+      eapply lts_comR; eauto.
+    - eapply lts_parL. eapply Hp; eauto. simpl. lia.
+    - eapply lts_parR. eapply Hp; eauto. simpl. lia.
+  + inversion H.
+  + inversion H; subst. rewrite<- pr_subst_and_NewVarC. constructor.
+  + inversion H; subst; simpl in *.
+    * eapply lts_ifOne; eauto. eapply Hp; eauto. simpl. lia.
+    * eapply lts_ifZero; eauto. eapply Hp; eauto. simpl. lia.
+  + inversion H.
+  + inversion H; subst; simpl in *.
+    eapply lts_res_tau. eapply Hp. lia. eauto.
+  + destruct g0; simpl in *.
+    * inversion H.
+    * inversion H.
+    * inversion H.
+    * inversion H; subst. constructor.
+    * inversion H; subst; simpl in *.
+      - eapply lts_choiceL. eapply Hp in H4; simpl; try lia. eauto.
+      - eapply lts_choiceR. eapply Hp in H4; simpl; try lia. eauto.
+Qed.
+
+Lemma NewVarCn_preserves_reduction q q2 k :
+  lts q τ q2 -> lts (NewVarCn 0 k q) τ (NewVarCn 0 k q2).
+Proof.
+  revert q q2. induction k.
+  + intros. simpl;eauto.
+  + intros; simpl in *. eapply NewVarC_preserves_reduction.
+    eapply IHk. eauto.
+Qed.
+
+Lemma VarSwap_com_VarC_in_ChannelData k j c : (NewVar_in_ChannelData j (VarSwap_in_ChannelData (j + k) c) 
+          = VarSwap_in_ChannelData (j + S k) (NewVar_in_ChannelData j c)).
+Proof.
+  destruct c; simpl.
+  + eauto.
+  + destruct (decide (n = (j + k)%nat)); subst.
+    - rewrite decide_True; try lia. simpl.
+      rewrite decide_True; try lia.
+      rewrite decide_True; try lia. eauto.
+    - destruct (decide (n = S (j + k))); subst.
+      * simpl. rewrite decide_True; try lia.
+        rewrite decide_True; try lia. simpl.
+        rewrite decide_False; try lia.
+        rewrite decide_True; try lia. eauto.
+      * simpl. destruct (decide (j < S n)); subst.
+        ++ simpl. rewrite decide_False; try lia.
+           rewrite decide_False; try lia. eauto.
+        ++ simpl. rewrite decide_False; try lia.
+           rewrite decide_False; try lia. eauto.
+Qed.
+
+Lemma VarSwap_com_VarC k j p : (NewVarC j (VarSwap_in_proc (j + k) p) = VarSwap_in_proc (j + S k) (NewVarC j p)).
+Proof.
+  revert k j.
+  induction p as (p & Hp) using
+    (well_founded_induction (wf_inverse_image _ nat _ size Nat.lt_wf_0)).
+  destruct p; intros; simpl in *.
+  + assert (NewVarC j (VarSwap_in_proc (j + k) p1) = VarSwap_in_proc (j + S k) (NewVarC j p1)) as eq1.
+    { eapply Hp. simpl. lia. }
+    assert (NewVarC j (VarSwap_in_proc (j + k) p2) = VarSwap_in_proc (j + S k) (NewVarC j p2)) as eq2.
+    { eapply Hp. simpl. lia. }
+    rewrite eq1, eq2. eauto.
+  + eauto.
+  + f_equal. eapply Hp. lia.
+  + assert (NewVarC j (VarSwap_in_proc (j + k) p1) = VarSwap_in_proc (j + S k) (NewVarC j p1)) as eq1.
+    { eapply Hp. simpl. lia. }
+    assert (NewVarC j (VarSwap_in_proc (j + k) p2) = VarSwap_in_proc (j + S k) (NewVarC j p2)) as eq2.
+    { eapply Hp. simpl. lia. }
+    rewrite eq1, eq2. eauto.
+  + rewrite VarSwap_com_VarC_in_ChannelData. eauto.
+  + f_equal. replace (S (j + k))%nat with ((S j) + k)%nat by lia.
+    replace (S (j + S k))%nat with ((S j) + S k)%nat by lia.
+    eapply Hp. lia.
+  + destruct g0; simpl in *.
+    - eauto.
+    - eauto.
+    - rewrite VarSwap_com_VarC_in_ChannelData.
+      assert (NewVarC j (VarSwap_in_proc (j + k) p) = VarSwap_in_proc (j + S k) (NewVarC j p)) as eq.
+      { eapply Hp. simpl. lia. }
+      rewrite eq. eauto.
+    - assert (NewVarC j (VarSwap_in_proc (j + k) p) = VarSwap_in_proc (j + S k) (NewVarC j p)) as eq.
+      { eapply Hp. simpl. lia. }
+      rewrite eq. eauto.
+    - assert (NewVarC j (VarSwap_in_proc (j + k) (g g0_1)) = VarSwap_in_proc (j + S k) (NewVarC j (g g0_1))) as eq1.
+      { eapply Hp. simpl. lia. }
+      assert (NewVarC j (VarSwap_in_proc (j + k) (g g0_2)) = VarSwap_in_proc (j + S k) (NewVarC j (g g0_2))) as eq2.
+      { eapply Hp. simpl. lia. } inversion eq1. inversion eq2. eauto.
+Qed.
+
+Lemma pr_subst_and_VarSwap2  (n : nat) (p : proc) (k : nat) (q : proc) : 
+    pr_subst n (VarSwap_in_proc k p) (VarSwap_in_proc k q) =
+    VarSwap_in_proc k (pr_subst n p q).
+Proof.
+  revert n k q.
+  induction p as (p & Hp) using
+    (well_founded_induction (wf_inverse_image _ nat _ size Nat.lt_wf_0)).
+  destruct p; intros; simpl in *.
+  + assert (pr_subst n (VarSwap_in_proc k p1) (VarSwap_in_proc k q) = VarSwap_in_proc k (pr_subst n p1 q)) as eq1.
+    { eapply Hp. simpl. lia. }
+    assert (pr_subst n (VarSwap_in_proc k p2) (VarSwap_in_proc k q) = VarSwap_in_proc k (pr_subst n p2 q)) as eq2.
+    { eapply Hp. simpl. lia. }
+    rewrite eq1, eq2. eauto.
+  + destruct (decide (n0 = n)); simpl ; eauto.
+  + destruct (decide (n0 = n)); simpl.
+    - eauto.
+    - assert (pr_subst n0 (VarSwap_in_proc k p) (VarSwap_in_proc k q) = VarSwap_in_proc k (pr_subst n0 p q)) as eq.
+      { eapply Hp. simpl. lia. }
+      rewrite eq. eauto.
+  + assert (pr_subst n (VarSwap_in_proc k p1) (VarSwap_in_proc k q) = VarSwap_in_proc k (pr_subst n p1 q)) as eq1.
+    { eapply Hp. simpl. lia. }
+    assert (pr_subst n (VarSwap_in_proc k p2) (VarSwap_in_proc k q) = VarSwap_in_proc k (pr_subst n p2 q)) as eq2.
+    { eapply Hp. simpl. lia. }
+    rewrite eq1, eq2. eauto.
+  + eauto.
+  + f_equal. replace k with (0 + k)%nat by lia. rewrite VarSwap_com_VarC.
+    simpl in *. eapply Hp. eauto.
+  + destruct g0; simpl in *.
+    * eauto.
+    * eauto.
+    * rewrite NewVar_and_VarSwap.
+      assert (pr_subst n (VarSwap_in_proc k p) (VarSwap_in_proc k (NewVar 0 q))
+          = VarSwap_in_proc k (pr_subst n p (NewVar 0 q))) as eq.
+      { eapply Hp. simpl. lia. }
+      rewrite eq. eauto.
+    * assert (pr_subst n (VarSwap_in_proc k p) (VarSwap_in_proc k q)
+          = VarSwap_in_proc k (pr_subst n p q)) as eq.
+      { eapply Hp. simpl. lia. }
+      rewrite eq. eauto.
+    * assert (pr_subst n (VarSwap_in_proc k (g g0_1)) (VarSwap_in_proc k q) 
+                  = VarSwap_in_proc k (pr_subst n (g g0_1) q)) as eq1.
+      { eapply Hp. simpl. lia. }
+      assert (pr_subst n (VarSwap_in_proc k (g g0_2)) (VarSwap_in_proc k q) 
+                  = VarSwap_in_proc k (pr_subst n (g g0_2) q)) as eq2.
+      { eapply Hp. simpl. lia. } inversion eq1. inversion eq2. eauto.
+Qed.
+
+Lemma VarSwap_swap_tau_proc p p' k : lts (VarSwap_in_proc k p) τ p' -> 
+lts p τ (VarSwap_in_proc k p').
+Proof.
+  revert k p'.
+  induction p as (p & Hp) using
+    (well_founded_induction (wf_inverse_image _ nat _ size Nat.lt_wf_0)).
+  destruct p; intros; simpl in *.
+  * dependent destruction H; simpl in *.
+    - eapply VarSwap_swap2_proc in H, H0. simpl in *. eapply lts_comL; eauto.
+    - eapply VarSwap_swap2_proc in H, H0. simpl in *. eapply lts_comR; eauto.
+    - rewrite Swap_Swap. eapply lts_parL. eapply Hp; simpl; eauto. lia.
+    - rewrite Swap_Swap. eapply lts_parR. eapply Hp; simpl; eauto. lia.
+  * inversion H.
+  * dependent destruction H; simpl in *. rewrite<- pr_subst_and_VarSwap2.
+    simpl in *. rewrite Swap_Swap. constructor.
+  * dependent destruction H; simpl in *.
+    - eapply lts_ifOne; eauto. eapply Hp; simpl; eauto. lia.
+    - eapply lts_ifZero; eauto. eapply Hp; simpl; eauto. lia.
+  * inversion H.
+  * dependent destruction H; simpl in *.
+    eapply lts_res_tau. eapply Hp; simpl; eauto.
+  * destruct g0; simpl in *.
+    - inversion H.
+    - inversion H.
+    - inversion H.
+    - dependent destruction H; simpl in *. rewrite Swap_Swap. eapply lts_tau.
+    - dependent destruction H; simpl in *.
+      + eapply lts_choiceL. eapply Hp; simpl; eauto. lia.
+      + eapply lts_choiceR. eapply Hp; simpl; eauto. lia.
+Qed.
+
+Lemma NewVarC_in_ChannelData_inv c c' k : NewVar_in_ChannelData k c = NewVar_in_ChannelData k c' -> c = c'.
+Proof.
+  destruct c; destruct c'; simpl; eauto; intro Hyp.
+  + destruct (decide (k < S n)); inversion Hyp.
+  + destruct (decide (k < S n)); inversion Hyp.
+  + destruct (decide (k < S n)); destruct (decide (k < S n0)).
+    - inversion Hyp. eauto.
+    - inversion Hyp. lia.
+    - inversion Hyp. lia.
+    - eauto.
+Qed.
+
+Lemma NewVarC_in_ext_inv μ μ' k : NewVarC_in_ext k μ = NewVarC_in_ext k μ' -> μ = μ'.
+Proof.
+  destruct μ; destruct μ'; destruct a; destruct a0; simpl in *; intro Hyp; inversion Hyp; subst;
+  eapply NewVarC_in_ChannelData_inv in H0 ; subst; eauto.
+Qed.
+
+Lemma NewVarC_in_ext_rev_Input c v μ' k : ActIn (c ⋉ v) = NewVarC_in_ext k μ' 
+    -> exists c' v', μ' = ActIn (c' ⋉ v') /\ v = v' /\ NewVar_in_ChannelData k c' = c.
+Proof.
+  destruct μ'; destruct c; destruct a; simpl in * ; intro Hyp; try (inversion Hyp); subst.
+  + exists c0. exists d. split ;eauto.
+  + exists c. exists d. split ;eauto.
+Qed.
+
+Lemma NewVarC_in_ext_rev_Output c v μ' k : ActOut (c ⋉ v) = NewVarC_in_ext k μ' 
+    -> exists c' v', μ' = ActOut (c' ⋉ v') /\ v = v' /\ NewVar_in_ChannelData k c' = c.
+Proof.
+  destruct μ'; destruct c; destruct a; simpl in * ; intro Hyp; try (inversion Hyp); subst.
+  + exists c0. exists d. split ;eauto.
+  + exists c. exists d. split ;eauto.
+Qed.
+
+Lemma NewVarC_inv p p' k : NewVarC k p = NewVarC k p' -> p = p'.
+Proof.
+  revert p' k.
+  induction p as (p & Hp) using
+    (well_founded_induction (wf_inverse_image _ nat _ size Nat.lt_wf_0)); destruct p; 
+    destruct p'; simpl in *; eauto; intros k Hyp ; try (inversion Hyp).
+  + eapply Hp in H0; subst; try lia.
+    eapply Hp in H1; subst; try lia. eauto.
+  + subst. f_equal. eauto.
+  + subst. eapply Hp in H1; subst; try lia.
+    eapply Hp in H2; subst; try lia. eauto.
+  + eapply NewVarC_in_ChannelData_inv in H0. subst. reflexivity.
+  + f_equal. eapply Hp in H0; eauto ; try lia.
+  + destruct g0; destruct g1; simpl in *; eauto; try (inversion Hyp).
+    - eapply Hp in H2; subst; eauto. eapply NewVarC_in_ChannelData_inv in H1. subst; eauto.
+    - eapply Hp in H1; subst; eauto.
+    - assert (NewVarC k (g g0_1) = NewVarC k (g g1_1)); simpl; eauto. inversion H1; eauto.
+      assert (NewVarC k (g g0_2) = NewVarC k (g g1_2)); simpl; eauto. inversion H2; eauto.
+      eapply Hp in H; simpl ; try lia. eapply Hp in H3; simpl ; try lia. inversion H. inversion H3. subst. eauto.
+Qed.
+
+Lemma inversion_k_NewVarC k μ μ' : NewVarC_in_ext 0 μ = NewVarC_in_ext (S k) μ' 
+  -> NewVarC_in_ext 0 μ = μ' \/ (exists μ'0, μ = NewVarC_in_ext k μ'0).
+Proof.
+  intro Hyp.
+  destruct μ; destruct a; destruct μ'; destruct a; destruct c; destruct c0; simpl in *; subst; try (inversion Hyp).
+    + subst. right. exists (ActIn (c0 ⋉ d0)). simpl; eauto.
+    + destruct (decide ((S k < S n))); inversion H0.
+    + destruct (decide ((S k < S n0))).
+      - subst. inversion H0. subst. right. inversion l.
+        ++ subst. exists (ActIn (k ⋉ d0)). simpl; eauto. rewrite decide_True; try lia. eauto.
+        ++ subst. assert (0 < n0); try lia. assert (0 < n0); try lia. eapply Nat.succ_pred_pos in H. exists (ActIn (Nat.pred n0 ⋉ d0)).
+           simpl. rewrite decide_True; try lia. f_equal. f_equal. eapply Nat.succ_pred_pos in H2. eauto.
+      - subst. inversion H0. subst. left; eauto.
+    + subst. left. eauto.
+    + destruct (decide ((S k < S n))); inversion H0.
+    + destruct (decide ((S k < S n0))).
+      - subst. inversion H0. subst. right. inversion l.
+        ++ subst. exists (ActOut (k ⋉ d0)). simpl; eauto. rewrite decide_True; try lia. eauto.
+        ++ subst. assert (0 < n0); try lia. assert (0 < n0); try lia. eapply Nat.succ_pred_pos in H. exists (ActOut (Nat.pred n0 ⋉ d0)).
+           simpl. rewrite decide_True; try lia. f_equal. f_equal. eapply Nat.succ_pred_pos in H2. eauto.
+      - subst. inversion H0. subst. left; eauto.
+Qed.
+
+Lemma NewVarC_ext_proc p μ p' k : lts (NewVarC k p) (ActExt μ)  p' -> 
+exists μ' p'', μ = NewVarC_in_ext k μ' /\ p' = (NewVarC k p'').
+Proof.
+  revert μ p' k.
+  induction p as (p & Hp) using
+    (well_founded_induction (wf_inverse_image _ nat _ size Nat.lt_wf_0)).
+  destruct p; intros; simpl in *.
+  * dependent destruction H; simpl in *.
+    - eapply Hp in H as (μ' & p'' & eq' & eq'') ; simpl; subst ; try lia.
+      exists μ'. exists (p'' ‖  p2). split; eauto.
+    - eapply Hp in H as (μ' & p'' & eq' & eq'') ; simpl; subst ; try lia.
+      exists μ'. exists (p1 ‖  p''). split; eauto.
+  * inversion H.
+  * inversion H.
+  * dependent destruction H; simpl in *.
+    - eapply Hp in H0 as (μ' & p'' & eq' & eq'') ; simpl; subst ; try lia.
+      exists μ'. exists p''. split; eauto.
+    - eapply Hp in H0 as (μ' & p'' & eq' & eq'') ; simpl; subst ; try lia.
+      exists μ'. exists p''. split; eauto.
+  * inversion H; subst. exists (ActOut (c ⋉ d)). exists 𝟘.
+    split; eauto.
+  * dependent destruction H; simpl in *.
+    eapply Hp in H as (μ' & p'' & eq' & eq'') ; simpl; subst ; try lia.
+    rewrite NewVarCzero_and_add in eq'.
+    assert (NewVarC_in_ext 0 μ = NewVarC_in_ext (S k) μ'); eauto.
+    eapply inversion_k_NewVarC in eq'. destruct eq' as [case1 | (μ'0 & case2)]; subst.
+    + replace (S k) with (0 + S k)%nat in H by lia.
+      rewrite<- NewVarC_and_NewVarC_in_ChannelData in H. simpl in *.
+      exists μ. exists (ν p''). split. eapply NewVarC_in_ext_inv in H. eauto.
+      simpl. eauto.
+    + exists μ'0. exists (ν p''). split; eauto.
+  * destruct g0; simpl in *.
+    - inversion H.
+    - inversion H.
+    - inversion H; subst. exists (ActIn (c ⋉ v)). exists (p ^ v).
+      split ;eauto. rewrite subst_and_NewVarC. eauto.
+    - inversion H.
+    - dependent destruction H; simpl in *.
+      + assert (lts (NewVarC k (g g0_1)) (ActExt μ) q) as Hyp; eauto.
+        eapply Hp in Hyp as (μ' & p'' & eq' & eq'') ; simpl; subst ; try lia.
+        exists μ'. exists p''. split; eauto.
+      + assert (lts (NewVarC k (g g0_2)) (ActExt μ) q) as Hyp; eauto.
+        eapply Hp in Hyp as (μ' & p'' & eq' & eq'') ; simpl; subst ; try lia.
+        exists μ'. exists p''. split; eauto.
+Qed.
+
+Lemma NewVarC_tau_proc p p' k : lts (NewVarC k p) τ p' ->
+ exists p'', p' = NewVarC k p''.
+Proof.
+  revert k p'.
+  induction p as (p & Hp) using
+    (well_founded_induction (wf_inverse_image _ nat _ size Nat.lt_wf_0)).
+  destruct p; intros; simpl in *.
+  * dependent destruction H; simpl in *.
+    - assert (lts (NewVarC k p1) ((c ⋉ v) !) p3); eauto. assert (lts (NewVarC k p2) ((c ⋉ v) ?) q2); eauto.
+      eapply NewVarC_ext_proc in H as (μ' & p'' & eq' & eq'') ; simpl; subst ; try lia.
+      eapply NewVarC_ext_proc in H0 as (μ'' & p''' & eq'' & eq''') ; simpl; subst ; try lia.
+      exists (p'' ‖  p'''). split; eauto.
+    - assert (lts (NewVarC k p2) ((c ⋉ v) !) p3); eauto. assert (lts (NewVarC k p1) ((c ⋉ v) ?) q2); eauto.
+      eapply NewVarC_ext_proc in H as (μ' & p'' & eq' & eq'') ; simpl; subst ; try lia.
+      eapply NewVarC_ext_proc in H0 as (μ'' & p''' & eq'' & eq''') ; simpl; subst ; try lia.
+      exists (p''' ‖  p''). split; eauto.
+    - eapply Hp in H as (p'' & eq'') ; simpl; subst ; try lia.
+      exists (p'' ‖  p2). split; eauto.
+    - eapply Hp in H as (p'' & eq'') ; simpl; subst ; try lia.
+      exists (p1 ‖  p''). split; eauto.
+  * inversion H.
+  * inversion H ; subst. exists (pr_subst n p (rec n • p)).
+    rewrite<- pr_subst_and_NewVarC. simpl; eauto.
+  * dependent destruction H; simpl in *.
+    - eapply Hp in H0 as (p'' & eq'') ; simpl; subst ; try lia.
+      exists p''. split; eauto.
+    - eapply Hp in H0 as (p'' & eq'') ; simpl; subst ; try lia.
+      exists p''. split; eauto.
+  * inversion H.
+  * dependent destruction H; simpl in *.
+    eapply Hp in H as (p'' & eq'') ; simpl; subst ; try lia.
+    exists (ν p''). simpl ; eauto.
+  * destruct g0; simpl in *.
+    - inversion H.
+    - inversion H.
+    - inversion H.
+    - inversion H; subst. exists p. auto.
+    - dependent destruction H; simpl in *.
+      + assert (lts (NewVarC k (g g0_1)) τ q) as Hyp; eauto.
+        eapply Hp in Hyp as (p'' & eq'') ; simpl; subst ; try lia.
+        exists p''. split; eauto.
+      + assert (lts (NewVarC k (g g0_2)) τ q) as Hyp; eauto.
+        eapply Hp in Hyp as (p'' & eq'') ; simpl; subst ; try lia.
+        exists p''. split; eauto.
+Qed.
+
+Lemma NewVarC_ext_proc_rev p μ' p' k : lts (NewVarC k p) (ActExt (NewVarC_in_ext k μ')) (NewVarC k p') -> 
+lts p (ActExt μ') p'.
+Proof.
+  revert μ' k p'.
+  induction p as (p & Hp) using
+    (well_founded_induction (wf_inverse_image _ nat _ size Nat.lt_wf_0)).
+  destruct p; intros; simpl in *.
+  * dependent destruction H; simpl in *; subst.
+    - assert (lts (NewVarC k p1) (ActExt (NewVarC_in_ext k μ')) p3) ; eauto.
+      eapply NewVarC_ext_proc in H as (μ'' & p'' & eq' & eq''); subst.
+      eapply Hp in H0; try lia. assert (NewVarC k (p'' ‖ p2) = NewVarC k p') as Hyp'; eauto.
+      eapply NewVarC_inv in Hyp'. subst. eapply lts_parL. eauto.
+    - assert (lts (NewVarC k p2) (ActExt (NewVarC_in_ext k μ')) q2) ; eauto.
+      eapply NewVarC_ext_proc in H as (μ'' & p'' & eq' & eq''); subst. eapply Hp in H0; try lia.
+      assert (NewVarC k (p1 ‖ p'') = NewVarC k p') as Hyp'; eauto.
+      eapply NewVarC_inv in Hyp'. subst. eapply lts_parR. eauto.
+  * inversion H.
+  * inversion H.
+  * dependent destruction H; simpl in *.
+    - eapply lts_ifOne; eauto. eapply Hp; simpl; eauto. lia.
+    - eapply lts_ifZero; eauto. eapply Hp; simpl; eauto. lia.
+  * inversion H; subst. assert (NewVarC_in_ext k (ActOut (c ⋉ d)) = NewVarC_in_ext k μ') as Hyp; eauto.
+    eapply NewVarC_in_ext_inv in Hyp. subst. replace (g 𝟘) with (NewVarC k (g 𝟘)) in H4 by eauto.
+    eapply NewVarC_inv in H4. subst. eapply lts_output.
+  * dependent destruction H; simpl in *. rewrite NewVarCzero_and_add in H. assert (0 + k = k)%nat as eq by lia.
+    rewrite<- eq in H at 2. rewrite NewVarC_and_NewVarC_in_ChannelData in H. simpl in *.
+    assert (lts (NewVarC (S k) p) (ActExt (NewVarC_in_ext (S k) (NewVarC_in_ext 0 μ'))) p'0) ;eauto.
+    eapply NewVarC_ext_proc in H as (μ'' & p'' & eq1 & eq2). subst.
+    eapply NewVarC_in_ext_inv in eq1. subst. assert (NewVarC k (ν p'') = NewVarC k p'); eauto.
+    eapply NewVarC_inv in H. subst. eapply lts_res_ext. eapply Hp in H0; try lia. rewrite NewVarCzero_and_add. eauto.
+  * destruct g0; simpl in *.
+    - inversion H.
+    - inversion H.
+    - inversion H; subst. assert (NewVarC_in_ext k (ActIn (c ⋉ v)) = NewVarC_in_ext k μ') as Hyp; eauto.
+      eapply NewVarC_in_ext_inv in Hyp. subst. rewrite subst_and_NewVarC in H4.
+      eapply NewVarC_inv in H4. subst. eapply lts_input.
+    - inversion H.
+    - dependent destruction H; simpl in *.
+      + assert (lts (NewVarC k (g g0_1)) (ActExt (NewVarC_in_ext k μ')) (NewVarC k p')); eauto.
+        eapply Hp in H0; simpl; try lia. eapply lts_choiceL. eauto.
+      + assert (lts (NewVarC k (g g0_2)) (ActExt (NewVarC_in_ext k μ')) (NewVarC k p')); eauto.
+        eapply Hp in H0; simpl; try lia. eapply lts_choiceR. eauto.
+Qed.
+
+Lemma inversion_NewVarC_par p1 p2 p3 k : p1 ‖ NewVarC k p2 = NewVarC k p3 -> exists p', p1 = NewVarC k p'.
+Proof.
+  destruct p3; intro Hyp ; simpl in *; try (inversion Hyp).
+  exists p3_1; eauto.
+Qed.
+
+Lemma inversion_NewVarC_par2 p1 p2 p3 k : NewVarC k p2 ‖ p1  = NewVarC k p3 -> exists p', p1 = NewVarC k p'.
+Proof.
+  destruct p3; intro Hyp ; simpl in *; try (inversion Hyp).
+  exists p3_2; eauto.
+Qed.
+
+Lemma NewVarC_tau_proc_rev p p' k : lts (NewVarC k p) τ (NewVarC k p') -> 
+lts p τ p'.
+Proof.
+  revert k p'.
+  induction p as (p & Hp) using
+    (well_founded_induction (wf_inverse_image _ nat _ size Nat.lt_wf_0)).
+  destruct p; intros; simpl in *.
+  * dependent destruction H; simpl in *; subst.
+    - assert (lts (NewVarC k p1) ((c ⋉ v) !) p3); eauto. assert (lts (NewVarC k p2) ((c ⋉ v) ?) q2); eauto.
+      eapply NewVarC_ext_proc in H as (μ' & p'' & eq1 & eq2); subst.
+      eapply NewVarC_ext_proc in H0 as (μ'' & p''' & eq'1 & eq'2); subst.
+      rewrite eq1 in H1. rewrite eq'1 in H2.
+      eapply NewVarC_ext_proc_rev in H1.
+      eapply NewVarC_ext_proc_rev in H2.
+      assert (NewVarC k (p'' ‖ p''') = NewVarC k p'); eauto.
+      eapply NewVarC_inv in H. subst. eapply NewVarC_in_ext_rev_Output in eq1 as (c' & v' & eq'' & eq''' & eq'''').
+      subst. eapply NewVarC_in_ext_rev_Input in eq'1 as (c'' & v'' & eq'' & eq''' & eq'''').
+      subst. eapply NewVarC_in_ChannelData_inv in eq''''. subst. eapply lts_comL; eauto.
+    - assert (lts (NewVarC k p2) ((c ⋉ v) !) p3); eauto. assert (lts (NewVarC k p1) ((c ⋉ v) ?) q2); eauto.
+      eapply NewVarC_ext_proc in H as (μ' & p'' & eq1 & eq2); subst.
+      eapply NewVarC_ext_proc in H0 as (μ'' & p''' & eq'1 & eq'2); subst.
+      rewrite eq1 in H1. rewrite eq'1 in H2.
+      eapply NewVarC_ext_proc_rev in H1.
+      eapply NewVarC_ext_proc_rev in H2.
+      assert (NewVarC k (p''' ‖ p'') = NewVarC k p'); eauto.
+      eapply NewVarC_inv in H. subst. eapply NewVarC_in_ext_rev_Output in eq1 as (c' & v' & eq'' & eq''' & eq'''').
+      subst. eapply NewVarC_in_ext_rev_Input in eq'1 as (c'' & v'' & eq'' & eq''' & eq'''').
+      subst. eapply NewVarC_in_ChannelData_inv in eq''''. subst. eapply lts_comR; eauto.
+    - assert (lts (NewVarC k p1) τ p3); eauto. assert (exists p', p3 = NewVarC k p') as (p'1 & eq); subst.
+      { eapply inversion_NewVarC_par. eauto. } assert (NewVarC k (p'1 ‖ p2) = NewVarC k p'); eauto.
+      eapply NewVarC_inv in H1; subst. eapply lts_parL. eapply Hp; eauto. simpl; lia.
+    - assert (lts (NewVarC k p2) τ q2); eauto. assert (exists p', q2 = NewVarC k p') as (p'1 & eq); subst.
+      { eapply inversion_NewVarC_par2. eauto. } assert (NewVarC k (p1 ‖ p'1) = NewVarC k p'); eauto.
+      eapply NewVarC_inv in H1; subst. eapply lts_parR. eapply Hp; eauto. simpl; lia.
+  * inversion H.
+  * dependent destruction H; simpl in *. replace (rec n • NewVarC k p) with (NewVarC k (rec n •  p)) in x; eauto.
+    rewrite pr_subst_and_NewVarC in x. eapply NewVarC_inv in x. subst. constructor.
+  * dependent destruction H; simpl in *.
+    - eapply lts_ifOne; eauto. eapply Hp; simpl; eauto. lia.
+    - eapply lts_ifZero; eauto. eapply Hp; simpl; eauto. lia.
+  * inversion H.
+  * dependent destruction H; simpl in *.
+    assert (lts (NewVarC (S k) p) τ p'0); eauto.
+    eapply NewVarC_tau_proc in H as (p'' & eq); subst.
+    assert (NewVarC k (ν p'') = NewVarC k p') as Hyp; eauto.
+    eapply NewVarC_inv in Hyp. subst. eapply lts_res_tau. eapply Hp; eauto.
+  * destruct g0; simpl in *.
+    - inversion H.
+    - inversion H.
+    - inversion H.
+    - dependent destruction H; simpl in *. eapply NewVarC_inv in x. subst. constructor.
+    - dependent destruction H; simpl in *.
+      + assert (lts (NewVarC k (g g0_1)) τ (NewVarC k p')); eauto. eapply lts_choiceL. eapply Hp; simpl; eauto. lia.
+      + assert (lts (NewVarC k (g g0_2)) τ (NewVarC k p')); eauto. eapply lts_choiceR. eapply Hp; simpl; eauto. lia.
+Qed.
 
 
 (* p 'is equivalent some r 'and r performs α to q , the congruence and the Transition can be reversed : *)
@@ -918,6 +2450,69 @@ Proof.
          * exists (p2 ‖ ( q ‖ r)). split. apply lts_parL. assumption. auto with cgr.
          * exists (p ‖ (q2 ‖ r)). split. apply lts_parR. apply lts_parL. assumption. auto with cgr.
       -- exists (p ‖ (q ‖ q2)). split. apply lts_parR.  auto. apply lts_parR. assumption. auto with cgr.
+    + intros. inversion l.
+    + intros. inversion l; subst.
+      -- inversion H0.
+      -- inversion H0.
+    + intros. dependent destruction l.
+      -- dependent destruction l. exists ((ν (ν VarSwap_in_proc 0 p'))). split.
+         eapply lts_res_ext. eapply lts_res_ext. rewrite VarC_action_add_add in l. simpl in *.
+         eapply VarSwap_swap_proc in l. rewrite VarC_action_add_add. simpl in *. eauto. eapply cgr_res_swap_rev.
+      -- dependent destruction l. exists ((ν (ν VarSwap_in_proc 0 p'))). split. eapply lts_res_tau.
+         eapply lts_res_tau. eapply VarSwap_swap_tau_proc. eauto. eapply cgr_res_swap_rev.
+    + intros. dependent destruction l.
+      -- dependent destruction l. exists ((ν (ν VarSwap_in_proc 0 p'))). split.
+         eapply lts_res_ext. eapply lts_res_ext. rewrite VarC_action_add_add. simpl.
+         eapply VarSwap_swap_proc. rewrite Swap_Swap. rewrite VarC_action_add_add in l. simpl in *.
+         eauto. eapply cgr_res_swap_rev.
+      -- dependent destruction l. exists ((ν (ν VarSwap_in_proc 0 p'))). split. eapply lts_res_tau.
+         eapply lts_res_tau. eapply VarSwap_swap_tau_proc. rewrite Swap_Swap. eauto. eapply cgr_res_swap_rev.
+    + intros. dependent destruction l.
+      -- inversion l1; subst. simpl in *. eapply (NewVarC_preserves_transition 0) in l2.
+         rewrite NewVarCzero_and_add_Channel in H1. simpl in *.
+         exists (ν (p' ‖ (NewVarC 0 q2))). split. eapply lts_res_tau.
+         eapply lts_comL; eauto. eapply cgr_res_scope.
+      -- inversion l2; subst. simpl in *. eapply (NewVarC_preserves_transition 0) in l1. simpl in *.
+         exists (ν (p' ‖ (NewVarC 0 p2))). split. eapply lts_res_tau.
+         eapply lts_comR; eauto. eapply cgr_res_scope.
+      -- dependent destruction l.
+         * exists (ν (p' ‖ NewVarC 0 q)). split. eapply lts_res_ext. eapply lts_parL. eauto.
+           eapply cgr_res_scope.
+         * exists (ν (p' ‖ NewVarC 0 q)). split. eapply lts_res_tau. eapply lts_parL. eauto.
+           eapply cgr_res_scope.
+      -- exists (ν (p ‖ NewVarC 0 q2)). destruct α.
+         * split. eapply lts_res_ext. eapply lts_parR. replace (NewVarC 0 q) with (NewVarCn 0 1 q); eauto.
+           replace (NewVarC 0 q2) with (NewVarCn 0 1 q2); eauto. eapply NewVarC_preserves_transition. eauto.
+           eapply cgr_res_scope.
+         * split. eapply lts_res_tau. eapply lts_parR. replace (NewVarC 0 q) with (NewVarCn 0 1 q); eauto.
+           replace (NewVarC 0 q2) with (NewVarCn 0 1 q2); eauto. eapply NewVarC_preserves_reduction. eauto.
+           eapply cgr_res_scope.
+    + intros. dependent destruction l.
+      -- dependent destruction l.
+         * exists (ν p2 ‖ q). split. eapply lts_parL. eapply lts_res_ext. eauto. eapply cgr_res_scope_rev.
+         * rewrite NewVarCzero_and_add in l. assert (exists q'2, q2 = NewVarC 0 q'2) as (q'2 & eq). 
+           { eapply NewVarC_ext_proc in l as (μ' & p'' & eq1 & eq2).
+             subst. exists p''. eauto. } subst.
+           assert (lts q (ActExt μ) q'2). { eapply NewVarC_ext_proc_rev. eauto. }
+           exists (ν p ‖ q'2). split. eapply lts_parR. eauto.
+           eapply cgr_res_scope_rev.
+      -- dependent destruction l.
+         * assert (lts (NewVarC 0 q) ((c ⋉ v) ?) q2) ;eauto.
+           eapply NewVarC_ext_proc in l2 as (μ' & p'' & eq1 & eq2); subst.
+           rewrite eq1 in H. eapply NewVarC_in_ext_rev_Input in eq1 as (c' & v' & eq' & eq'' & eq'''); subst.
+           simpl in *. exists ((ν p2) ‖ p''). split. eapply lts_comL. eapply lts_res_ext. rewrite NewVarCzero_and_add.
+           eauto. eapply NewVarC_ext_proc_rev; eauto. eapply cgr_res_scope_rev.
+         * assert (lts (NewVarC 0 q) ((c ⋉ v) !) p2) ;eauto.
+           eapply NewVarC_ext_proc in l1 as (μ' & p'' & eq1 & eq2); subst.
+           rewrite eq1 in H. eapply NewVarC_in_ext_rev_Output in eq1 as (c' & v' & eq' & eq'' & eq'''); subst.
+           simpl in *. exists ((ν q2) ‖ p''). split. eapply lts_comR. eapply NewVarC_ext_proc_rev; eauto.
+           eapply lts_res_ext. rewrite NewVarCzero_and_add.
+           eauto. eapply cgr_res_scope_rev.
+         * exists ((ν p2) ‖ q). split. eapply lts_parL. eapply lts_res_tau. eauto.
+           eapply cgr_res_scope_rev.
+         * assert (lts (NewVarC 0 q) τ q2); eauto. eapply NewVarC_tau_proc in l as (q'' & eq''); subst.
+           eapply NewVarC_tau_proc_rev in H. exists ((ν p) ‖ q''). split.
+           eapply lts_parR. eauto. eapply cgr_res_scope_rev.
     + intros. exists q.  split. apply lts_choiceL.  assumption. auto with cgr.
     + intros. dependent destruction l.
       -- exists q. split. assumption. auto with cgr.
@@ -954,6 +2549,11 @@ Proof.
       -- eexists. split. instantiate (1:= (p ‖ q2)). apply lts_parR.
           assumption. apply cgr_par.
           constructor. assumption.
+    + intros. inversion l; subst.
+      -- destruct (IHcgr_step p' (ActExt (VarC_action_add 1 μ))) as (q'1 & l' & equiv'). eauto.
+         exists (ν q'1). split; eauto. eapply lts_res_ext. eauto. eapply cgr_res. eauto.
+      -- destruct (IHcgr_step p' τ) as (q'1 & l' & equiv'). eauto. exists (ν q'1). split.
+         eapply lts_res_tau. eauto. eapply cgr_res. eauto. 
     + intros. dependent destruction l.
       -- eexists. split. instantiate (1:= p'). apply lts_ifOne; eauto. reflexivity. 
       -- destruct (IHcgr_step q'0 α) as (q'1 & l' & equiv'). eauto.
@@ -969,48 +2569,62 @@ Proof.
     destruct H. destruct H0. eauto with cgr.
 Qed.
 
+Lemma lts_res_ext_n n p p' μ : lts p (ActExt (VarC_action_add n μ)) p' -> lts (Ѵ  n p) (ActExt μ) (Ѵ  n p').
+Proof.
+  revert p p' μ.
+  induction n.
+  + simpl; eauto. intros. rewrite VarC_add_zero_ext in H. eauto.
+  + intros. simpl in *. eapply lts_res_ext. eapply IHn. replace (S n) with (n + 1)%nat in H by lia.
+    rewrite VarC_action_add_add; eauto.
+Qed.
 
+Lemma lts_res_tau_n n p p' : lts p τ p' -> lts (Ѵ  n p) τ (Ѵ  n p').
+Proof.
+  revert p p'.
+  induction n.
+  + simpl; eauto.
+  + intros. simpl in *. eapply lts_res_tau. eapply IHn. eauto.
+Qed.
 
 (* One side of the Harmony Lemma *)
 Lemma Reduction_Implies_TausAndCong : forall P Q, (sts P Q) -> (lts_then_sc P τ Q).
 Proof. 
 intros P Q Reduction. 
-assert ((exists c v P2 G2 S, ((P ≡* ((c ! v • 𝟘) ‖ ((c ? x • P2) + G2)) ‖ S)) /\ (Q ≡*((𝟘 ‖ (P2^v)) ‖ S)))
-\/ (exists P1 G1 S, (P ≡* (((t • P1) + G1) ‖ S)) /\ (Q ≡* (P1 ‖ S)))
-\/ (exists n P1 S, (P ≡* ((rec n • P1) ‖ S)) /\ (Q ≡* (pr_subst n P1 (rec n • P1) ‖ S)))
-).
+assert ((exists c v P2 G2 S n, ((P ≡* Ѵ  n (((c ! v • 𝟘) ‖ ((c ? x • P2) + G2)) ‖ S))) /\ (Q ≡* Ѵ  n ((𝟘 ‖ (P2^v)) ‖ S)))
+\/ (exists P1 G1 S n, (P ≡* Ѵ  n (((t • P1) + G1) ‖ S)) /\ (Q ≡* Ѵ  n (P1 ‖ S)))
+\/ (exists n P1 S n', (P ≡* Ѵ  n' ((rec n • P1) ‖ S)) /\ (Q ≡* Ѵ  n' (pr_subst n P1 (rec n • P1) ‖ S)))
+). 
 apply ReductionShape. exact Reduction.
-destruct H as [IH|[IH|IH]]. 
+destruct H as [IH|[IH|IH]];  decompose record IH. 
 
 (*First case τ by communication *)
 
-- decompose record IH.
-  assert (lts ((x ! x0 • 𝟘) ‖ ((x ? l • x1) + x2) ‖ x3) τ (𝟘 ‖ (x1^x0) ‖ x3)).
-  * apply lts_parL.   
+- assert (lts (Ѵ x4 ((x ! x0 • 𝟘) ‖ ((x ? l • x1) + x2) ‖ x3)) τ (Ѵ x4 (𝟘 ‖ (x1^x0) ‖ x3))).
+  * eapply lts_res_tau_n.
+    apply lts_parL.   
     eapply lts_comL. instantiate (2:= x). instantiate (1:= x0).
     apply lts_output. apply lts_choiceL. apply lts_input.
-  * assert (sc_then_lts P τ ((𝟘 ‖ x1^x0) ‖ x3)). exists (((x ! x0 • 𝟘) ‖ ((x ? l • x1) + x2)) ‖ x3). split. assumption. assumption.
-    assert (lts_then_sc P τ ((𝟘 ‖ x1^x0) ‖ x3)). apply Congruence_Respects_Transition. assumption. destruct H3. destruct H3.
-    exists x4. split. assumption. apply transitivity with ((𝟘 ‖ x1^x0) ‖ x3). assumption. symmetry. assumption.
+  * assert (sc_then_lts P τ (Ѵ x4 ((𝟘 ‖ x1^x0) ‖ x3))). exists ((Ѵ x4 ((x ! x0 • 𝟘 ‖ (gpr_input x x1 + x2)) ‖ x3))). split. assumption. assumption.
+    assert (lts_then_sc P τ (Ѵ x4 ((𝟘 ‖ x1^x0) ‖ x3))). apply Congruence_Respects_Transition. assumption. destruct H3. destruct H3.
+    exists x5. split. assumption. apply transitivity with (Ѵ x4 ((𝟘 ‖ x1^x0) ‖ x3)). assumption. symmetry. assumption.
 
 (*Second case τ by Tau Action *)
 
-- decompose record IH.
-  assert (lts ((t • x + x0) ‖ x1) τ (x ‖ x1)). constructor.
+- assert (lts (Ѵ x2 ((t • x + x0) ‖ x1)) τ (Ѵ x2 (x ‖ x1))). eapply lts_res_tau_n. constructor.
   apply lts_choiceL. apply lts_tau.
-  assert (sc_then_lts P τ (x ‖ x1)). exists ((t • x + x0) ‖ x1). split. assumption. apply lts_parL.
-  apply lts_choiceL. apply lts_tau.
-  assert (lts_then_sc P τ (x ‖ x1)). apply Congruence_Respects_Transition. assumption. destruct H3. destruct H3. 
-  exists x2. split. assumption. apply transitivity with (x ‖ x1). assumption. symmetry. assumption.
+  assert (sc_then_lts P τ (Ѵ x2 (x ‖ x1))). exists (Ѵ x2 ((t • x + x0) ‖ x1)). split. assumption.
+  eapply lts_res_tau_n. apply lts_parL. apply lts_choiceL. apply lts_tau.
+  assert (lts_then_sc P τ (Ѵ x2 (x ‖ x1))). apply Congruence_Respects_Transition. assumption. destruct H3. destruct H3. 
+  exists x3. split. assumption. apply transitivity with (Ѵ x2 (x ‖ x1)). assumption. symmetry. assumption.
 
 (*Third case τ by recursion *)
 
-- decompose record IH.
-  assert (lts (rec x • x0 ‖ x1) τ (pr_subst x x0 (rec x • x0) ‖ x1)). 
-  constructor. apply lts_recursion. assert (sc_then_lts P τ ((pr_subst x x0 (rec x • x0) ‖ x1))). 
-  exists (rec x • x0 ‖ x1). split. assumption. assumption. assert (lts_then_sc P τ (pr_subst x x0 (rec x • x0) ‖ x1)). 
+- assert (lts (Ѵ x2 (rec x • x0 ‖ x1)) τ (Ѵ x2 (pr_subst x x0 (rec x • x0) ‖ x1))). eapply lts_res_tau_n.
+  constructor. apply lts_recursion. assert (sc_then_lts P τ (Ѵ x2 ((pr_subst x x0 (rec x • x0) ‖ x1)))). 
+  exists (Ѵ x2 (rec x • x0 ‖ x1)). split. assumption. assumption.
+  assert (lts_then_sc P τ (Ѵ x2 (pr_subst x x0 (rec x • x0) ‖ x1))). 
   apply Congruence_Respects_Transition. assumption. destruct H3. destruct H3. 
-  exists x2. split. assumption. apply transitivity with (pr_subst x x0 (rec x • x0) ‖ x1). assumption.
+  exists x3. split. assumption. apply transitivity with (Ѵ x2 (pr_subst x x0 (rec x • x0) ‖ x1)). assumption.
   symmetry. assumption.
 Qed.
 
@@ -1054,6 +2668,117 @@ intros. destruct H0. destruct H0. eapply sts_cong. instantiate (1:=P). apply cgr
 exact H1.
 Qed.
 
+Lemma simpl_NewVarC k k' p : NewVarC k (Ѵ k' p) = Ѵ k' (NewVarC (k + k') p).
+Proof.
+  revert p k. induction k'.
+  + simpl. intros. replace (k + 0)%nat with k%nat by lia. eauto.
+  + intros. simpl. f_equal. rewrite IHk'. f_equal. replace (S k + k')%nat with (k + S k')%nat by lia.
+    eauto.
+Qed.
+
+Lemma simpl_NewVarCn j k k' p: NewVarCn j k (Ѵ  k' p) = Ѵ  k' (NewVarCn (j + k') k p).
+Proof.
+  intros. revert j k' p. induction k.
+  + simpl. eauto.
+  + intros. simpl in *. rewrite<- (NewVarCn_revert_def k p (j + k')).
+    rewrite<- (IHk j k' (NewVarC (j + k') p)). rewrite<- NewVarCn_revert_def at 1. f_equal.
+    eapply simpl_NewVarC.
+Qed.
+
+Lemma sts_res_n n P Q : sts P Q → sts (Ѵ n P) (Ѵ n Q).
+Proof.
+  revert P Q. induction n.
+  + intros; simpl; eauto.
+  + intros; simpl. eapply sts_res. eauto.
+Qed.
+
+Lemma NewVarC_res i k p : NewVarC i (Ѵ k p) = Ѵ k (NewVarC (i + k) p).
+Proof.
+  revert i p. induction k.
+  + intros; simpl; eauto. replace (i + 0)%nat with i by lia. eauto.
+  + intros; simpl. f_equal. rewrite IHk. f_equal. replace (S i + k)%nat with (i + S k)%nat by lia. eauto.
+Qed.
+
+Lemma NewVarCn_res i j k p : NewVarCn i j (Ѵ k p) = Ѵ k (NewVarCn (i + k) j p).
+Proof.
+  revert i k p. induction j.
+  + intros; simpl; eauto.
+  + intros; simpl. rewrite<- NewVarCn_revert_def. rewrite<- NewVarCn_revert_def.
+    rewrite<- (IHj i k (NewVarC (i + k) p)). f_equal. rewrite NewVarC_res. eauto.
+Qed.
+
+Lemma NewVarCn_par i j p q: NewVarCn i j (p ‖ q) = (NewVarCn i j p) ‖ (NewVarCn i j q).
+Proof.
+  revert i p q. induction j.
+  + intros; simpl; eauto.
+  + intros; simpl. rewrite<- NewVarCn_revert_def. simpl. rewrite<- NewVarCn_revert_def.
+    rewrite<- NewVarCn_revert_def. rewrite IHj. eauto. 
+Qed.
+
+Lemma NewVarCn_input k j c p : gNewVarCn 0 j ((VarC_add k c) ? x • p) = (VarC_add (j + k) c) ? x • (NewVarCn 0 j p).
+Proof.
+  revert k c p. induction j.
+  + intros; simpl; eauto.
+  + intros; simpl. rewrite<- NewVarCn_revert_def. rewrite IHj. simpl. rewrite<- NewVarCn_revert_def.
+    rewrite<- NewVarCzero_and_add_Channel. rewrite<- VarC_add_revert_def. simpl. eauto.
+Qed.
+
+Lemma subst_and_NewVarCn k i j v q :
+    subst_in_proc k v (NewVarCn i j q) = NewVarCn i j (subst_in_proc k v q).
+Proof.
+  revert v q k i. induction j.
+  + intros; simpl; eauto.
+  + intros; simpl. rewrite subst_and_NewVarC. f_equal.
+    eapply IHj.
+Qed.
+
+Lemma simpl_NewVar_auto k j c : (NewVar_in_ChannelData k (VarC_add (k + j) c)) = (VarC_add (k + S j) c).
+Proof.
+  destruct c.
+  + simpl. eauto.
+  + simpl. rewrite decide_True; try lia. replace (k + S j)%nat with (S (k + j))%nat by lia.
+    replace (S (k + j) + n)%nat with (S (k + j + n))%nat by lia. eauto.
+Qed.
+
+Lemma NewVarCn_output k j c d : (NewVarCn k j (VarC_add k c ! d • 𝟘) = (VarC_add (j + k) c) ! d • 𝟘).
+Proof.
+  revert k c d. induction j.
+  + intros; simpl; eauto.
+  + intros; simpl. rewrite IHj. simpl. 
+    assert (j+k = k + j)%nat as eq by lia. rewrite eq at 1. rewrite simpl_NewVar_auto.
+    replace (k + S j)%nat with (S (j + k))%nat by lia. f_equal.
+Qed.
+
+Lemma NewVarCn_choice i j g1 g2: NewVarCn i j (g (g1 + g2)) = (gNewVarCn i j g1) + (gNewVarCn i j g2).
+Proof.
+  revert i g1 g2. induction j.
+  + intros; simpl; eauto.
+  + intros; simpl. rewrite IHj. simpl. eauto.
+Qed.
+
+Lemma simpl_NewVarCn_plus_par k j c p g1 q : (NewVarCn k j ((gpr_input (VarC_add k c) p + g1) ‖ q)
+        = ((gpr_input (VarC_add (k + j) c) (NewVarCn k j p)) + (gNewVarCn k j g1)) ‖ (NewVarCn k j q)).
+Proof.
+  revert k c p g1 q. induction j.
+  + intros ; simpl; eauto. replace (k + 0)%nat with k by lia. eauto.
+  + intros; simpl. rewrite IHj. simpl. f_equal. rewrite simpl_NewVar_auto. eauto.
+Qed.
+
+Lemma simpl_NewVarCn_par_plus k j c v q : NewVarCn 0 k ((VarC_add j c ! v • 𝟘) ‖ q)
+        = ((VarC_add (k + j) c ! v • 𝟘 ) ‖ (NewVarCn 0 k q)).
+Proof.
+  revert j c v q. induction k.
+  + intros ; simpl; eauto.
+  + intros; simpl. rewrite IHk. simpl. f_equal.
+    rewrite<- NewVarCzero_and_add_Channel. rewrite<- VarC_add_revert_def.
+    simpl. eauto.
+Qed.
+
+Lemma simpl_NewVarCn_zero j k : NewVarCn j k 𝟘 = 𝟘.
+Proof.
+  revert j. induction k; simpl ; eauto. intros; rewrite IHk. simpl;eauto.
+Qed.
+
 Lemma Taus_Implies_Reduction : forall P Q, (lts P τ Q) -> (sts P Q).
 Proof. 
 intros.
@@ -1069,37 +2794,53 @@ dependent induction H.
     + eapply cgr_if_false; eauto.
     + eauto.
     + reflexivity.
-  - destruct (TransitionShapeForOutput p1 p2 c v). assumption.  decompose record H1.
-    destruct (TransitionShapeForInput q1 q2 c v). assumption. decompose record H4.
-    eapply sts_cong. instantiate (1:=((c ! v • 𝟘) ‖ ((c ? l • x0) + x1)) ‖ (x ‖ x2)).
-    apply cgr_trans with ((c ! v • 𝟘 ‖ x) ‖ (((c ? l • x0) + x1) ‖ x2)). apply cgr_fullpar. assumption. assumption.
-    apply InversionParallele. 
-    instantiate (1 := (𝟘 ‖ (x0^v)) ‖ (x ‖ x2)). apply sts_par.
-    apply sts_com. 
-    apply transitivity with ((𝟘 ‖ x) ‖ ((x0^v) ‖ x2)). apply InversionParallele. apply cgr_fullpar. 
-    symmetry. assumption. symmetry. assumption.
+  - eapply sts_res. eauto.
   - destruct (TransitionShapeForOutput p1 p2 c v). assumption. decompose record H1.
-    destruct (TransitionShapeForInput q1 q2 c v). assumption. decompose record H4.
-    eapply sts_cong. instantiate (1:=((c ! v • 𝟘) ‖ ((c ? l • x0) + x1)) ‖ (x ‖ x2)).
-    apply transitivity with (p1 ‖ q1). apply cgr_par_com.
-    apply transitivity with (((c ! v • 𝟘) ‖ x) ‖ (((c ? l • x0) + x1) ‖ x2)).
-    apply cgr_fullpar. assumption. assumption. apply InversionParallele. 
-    instantiate (1 := (𝟘 ‖ (x0^v)) ‖ (x ‖ x2)). apply sts_par. apply sts_com.
-    apply transitivity with ((𝟘 ‖ x) ‖ ((x0^v) ‖ x2)). apply InversionParallele. apply transitivity with (p2 ‖ q2). apply cgr_fullpar. 
-    symmetry. assumption. symmetry. assumption. apply cgr_par_com.
-- apply sts_par. apply IHlts. reflexivity.
-- eapply sts_cong. instantiate (1:= q1 ‖ p). apply cgr_par_com. instantiate (1:= q2 ‖ p).
-  apply sts_par. apply IHlts. reflexivity. apply cgr_par_com.
-- destruct (TransitionShapeForTauAndGuard (g p1) q). split. assumption. exists p1. reflexivity.
-  decompose record H0.
-  eapply sts_cong. instantiate (1:= ((t • x) + (x0 + p2))).
-  apply transitivity with (g (((t • x) + x0) + p2)). apply cgr_choice. assumption. apply cgr_choice_assoc.
-  instantiate (1:= x). apply sts_tau. symmetry. assumption.
-- destruct (TransitionShapeForTauAndGuard (g p2) q). split. assumption. exists p2. reflexivity.
-  decompose record H0. eapply sts_cong. instantiate (1:= ((t • x) + (x0 + p1))).
-  apply transitivity with (g (((t • x) + x0 ) + p1)). apply transitivity with (g (p2 + p1)). apply cgr_choice_com.
-  apply cgr_choice. assumption. apply cgr_choice_assoc. instantiate (1:= x). apply sts_tau.
-  symmetry. assumption.
+    destruct (TransitionShapeForInput q1 q2 c v). assumption. decompose record H2.
+    eapply sts_cong. etrans. instantiate (1:= Ѵ x0 ((VarC_add x0 c ! v • 𝟘) ‖ x) ‖ Ѵ x4 ((gpr_input (VarC_add x4 c) x1 + x2) ‖ x3)).
+    eapply cgr_fullpar; eauto. etrans. eapply cgr_res_scope_n. rewrite simpl_NewVarCn. etrans.
+    eapply cgr_res_n. eapply cgr_par_com. etrans. eapply cgr_res_n. eapply cgr_res_scope_n. etrans.
+    eapply cgr_res_n. etrans. eapply cgr_res_n. simpl. rewrite simpl_NewVarCn_par_plus.
+    rewrite simpl_NewVarCn_plus_par. etrans. 
+    instantiate (1 := ((VarC_add (x4 + x0) c ! v • 𝟘) ‖ NewVarCn x4 x0 x3) ‖
+           ((gpr_input (VarC_add (x4 + x0) c) (NewVarCn x4 x0 x1) + gNewVarCn x4 x0 x2) ‖ NewVarCn 0 x4 x)). etrans.
+    apply InversionParallele. etrans. 
+    instantiate (1:= ((VarC_add (x4 + x0) c ! v • 𝟘)
+        ‖ (gpr_input (VarC_add (x4 + x0) c) (NewVarCn x4 x0 x1) + gNewVarCn x4 x0 x2))
+        ‖ (NewVarCn x4 x0 x3 ‖ NewVarCn 0 x4 x)). apply cgr_fullpar; eauto. eapply cgr_par_com. reflexivity.
+    apply InversionParallele. apply InversionParallele. reflexivity. reflexivity.
+    eapply sts_res_n. eapply sts_res_n. eapply sts_par. eapply sts_com. symmetry. etrans.
+    eapply cgr_fullpar; eauto. etrans. eapply cgr_res_scope_n. eapply cgr_res_n.
+    etrans. rewrite NewVarCn_res. eapply cgr_par_com. etrans. eapply cgr_res_scope_n.
+    eapply cgr_res_n. simpl. rewrite NewVarCn_par. rewrite NewVarCn_par. rewrite subst_and_NewVarCn.
+    etrans. eapply InversionParallele. eapply cgr_fullpar. simpl. rewrite simpl_NewVarCn_zero. eapply cgr_par_com. reflexivity.
+  - destruct (TransitionShapeForOutput p1 p2 c v). assumption. decompose record H1.
+    destruct (TransitionShapeForInput q1 q2 c v). assumption. decompose record H2.
+    eapply sts_cong. etrans. instantiate (1:= Ѵ x4 ((gpr_input (VarC_add x4 c) x1 + x2) ‖ x3) ‖ Ѵ x0 ((VarC_add x0 c ! v • 𝟘) ‖ x)).
+    eapply cgr_fullpar; eauto. etrans. eapply cgr_res_scope_n. rewrite simpl_NewVarCn. etrans.
+    eapply cgr_res_n. eapply cgr_par_com. etrans. eapply cgr_res_n. eapply cgr_res_scope_n. etrans.
+    eapply cgr_res_n. etrans. eapply cgr_res_n. simpl. rewrite NewVarCn_par. rewrite NewVarCn_par.
+    rewrite NewVarCn_choice. rewrite NewVarCn_input. rewrite NewVarCn_output.
+    apply InversionParallele. eapply cgr_res_n. reflexivity. etrans. eapply cgr_res_n. eapply cgr_res_n.
+    reflexivity. eapply cgr_res_n. eapply cgr_res_n. reflexivity. eapply sts_res_n. eapply sts_res_n.
+    eapply sts_par. replace (x4 + x0)%nat with (x0 + x4)%nat by lia. eapply sts_com. symmetry.
+    etrans. eapply cgr_fullpar; eauto. etrans. eapply cgr_res_scope_n. eapply cgr_res_n.
+    rewrite NewVarCn_res. etrans. eapply cgr_par_com. etrans. eapply cgr_res_scope_n.
+    eapply cgr_res_n. simpl. rewrite NewVarCn_par. rewrite NewVarCn_par.
+    rewrite<- subst_and_NewVarCn. etrans. apply InversionParallele. rewrite simpl_NewVarCn_zero. reflexivity.
+  - apply sts_par. apply IHlts. reflexivity.
+  - eapply sts_cong. instantiate (1:= q1 ‖ p). apply cgr_par_com. instantiate (1:= q2 ‖ p).
+    apply sts_par. apply IHlts. reflexivity. apply cgr_par_com.
+  - destruct (TransitionShapeForTauAndGuard (g p1) q). split. assumption. exists p1. reflexivity.
+    decompose record H0.
+    eapply sts_cong. instantiate (1:= ((t • x) + (x0 + p2))).
+    apply transitivity with (g (((t • x) + x0) + p2)). apply cgr_choice. assumption. apply cgr_choice_assoc.
+    instantiate (1:= x). apply sts_tau. symmetry. assumption.
+  - destruct (TransitionShapeForTauAndGuard (g p2) q). split. assumption. exists p2. reflexivity.
+    decompose record H0. eapply sts_cong. instantiate (1:= ((t • x) + (x0 + p1))).
+    apply transitivity with (g (((t • x) + x0 ) + p1)). apply transitivity with (g (p2 + p1)). apply cgr_choice_com.
+    apply cgr_choice. assumption. apply cgr_choice_assoc. instantiate (1:= x). apply sts_tau.
+    symmetry. assumption.
 Qed.
 
 (* One side of the Harmony Lemma*)
@@ -1127,6 +2868,7 @@ Inductive Well_Defined_Condition : nat -> Equation Data -> Prop :=
 Inductive Well_Defined_Input_in : nat -> proc -> Prop :=
 | WD_par : forall k p1 p2, Well_Defined_Input_in k p1 -> Well_Defined_Input_in k p2 
                 -> Well_Defined_Input_in k (p1 ‖ p2)
+| WD_res : forall k p, Well_Defined_Input_in k p -> Well_Defined_Input_in k (ν p)
 | WD_var : forall k i, Well_Defined_Input_in k (pr_var i)
 | WD_rec : forall k x p1, Well_Defined_Input_in k p1 -> Well_Defined_Input_in k (rec x • p1)
 | WD_if_then_else : forall k p1 p2 C, Well_Defined_Condition k C -> Well_Defined_Input_in k p1 
@@ -1172,6 +2914,7 @@ destruct p.
   ** apply Hp. simpl; auto with arith. assumption.
   ** apply Hp. simpl; auto with arith. assumption.
 - intros. constructor. dependent destruction H. apply Inequation_k_data. assumption.
+- intros. constructor. apply Hp. simpl; auto with arith. dependent destruction H. assumption.
 - destruct g0.
   ** intros. constructor.
   ** intros. constructor.
@@ -1279,6 +3022,7 @@ destruct p.
   - apply Hp. simpl. auto with arith. assumption.
   - apply Hp. simpl. auto with arith. assumption.
 * intros. simpl. dependent destruction H. constructor. apply ForData. assumption.
+* intros. simpl. dependent destruction H. constructor. apply Hp. simpl. auto with arith. assumption.
 * destruct g0.
   - intros. simpl. constructor.
   - intros. simpl. constructor.
@@ -1328,6 +3072,7 @@ destruct p; intros; simpl.
    - apply Hp. simpl. auto with arith. assumption.
    - apply Hp. simpl. auto with arith. assumption.
 * constructor. dependent destruction H. apply WD_data_and_NewVar. assumption.
+* constructor. dependent destruction H. apply Hp. simpl. auto with arith. assumption.
 * destruct g0; intros; simpl.
   - constructor.
   - constructor.
@@ -1341,6 +3086,35 @@ destruct p; intros; simpl.
        apply Hp. simpl. auto with arith. assumption. assumption.
     -- assert (S (k + i) = (S k + i)%nat). auto with arith. rewrite H1.
        assert (Well_Defined_Input_in (S k + i) (NewVar i (g g0_2))).
+       apply Hp. simpl. auto with arith. assumption. assumption.
+Qed.
+
+Lemma WD_and_NewVarC : forall k i p, Well_Defined_Input_in k p -> Well_Defined_Input_in k (NewVarC i p).
+Proof.
+intros. revert H. revert k i.
+induction p as (p & Hp) using
+    (well_founded_induction (wf_inverse_image _ nat _ size Nat.lt_wf_0)).
+destruct p; intros; simpl.
+* dependent destruction H. constructor.
+   - apply Hp. simpl. auto with arith. assumption.
+   - apply Hp. simpl. auto with arith. assumption.
+* constructor.
+* constructor. dependent destruction H. apply Hp. simpl. auto with arith. assumption.
+* dependent destruction H. constructor. eauto.
+   - apply Hp. simpl. auto with arith. assumption.
+   - apply Hp. simpl. auto with arith. assumption.
+* constructor. dependent destruction H. eauto.
+* constructor. dependent destruction H. apply Hp. simpl. auto with arith. assumption.
+* destruct g0; intros; simpl.
+  - constructor.
+  - constructor.
+  - dependent destruction H. constructor. 
+    apply Hp. simpl. auto with arith. eauto.
+  - constructor. apply Hp. simpl. auto. dependent destruction H. assumption.
+  - dependent destruction H. constructor.
+    -- assert (Well_Defined_Input_in k (NewVarC i (g g0_1))).
+       apply Hp. simpl. auto with arith. assumption. assumption.
+    -- assert (Well_Defined_Input_in k (NewVarC i (g g0_2))).
        apply Hp. simpl. auto with arith. assumption. assumption.
 Qed.
 
@@ -1363,6 +3137,10 @@ destruct p'.
   ** apply Hp. simpl; auto with arith. assumption. assumption.
   ** apply Hp. simpl; auto with arith. assumption. assumption.
 * intros. simpl. assumption.
+* intros. simpl. constructor. dependent destruction H. apply Hp.
+    - simpl; auto with arith.
+    - eapply WD_and_NewVarC. eauto.
+    - eauto.
 * destruct g0. 
   ** intros. simpl. constructor.
   ** intros. simpl. constructor.
@@ -1427,6 +3205,7 @@ intros. dependent induction H0. dependent destruction H. eapply Well_Def_Data_Is
 subst. exists x. reflexivity.
 - dependent destruction H. eapply IHlts with c. assumption. reflexivity.
 - dependent destruction H. eapply IHlts with c. assumption. reflexivity.
+- dependent destruction H. simpl in *. eapply IHlts with (VarC_add 1 c). assumption. simpl. reflexivity.
 - dependent destruction H. eapply IHlts with c. assumption. reflexivity.
 - dependent destruction H. eapply IHlts with c. assumption. reflexivity.
 - dependent destruction H. eapply IHlts with c. assumption. reflexivity.
@@ -1437,12 +3216,18 @@ Lemma LTS_Respects_WD : forall p q α, Well_Defined_Input_in 0 p -> Well_Defined
             ->  Well_Defined_Input_in 0 q.
 Proof.
 intros. revert H. revert H0. rename H1 into Transition. dependent induction Transition.
-* intros. dependent destruction H0.  apply ForSTS. dependent destruction H. assumption.
+* intros. dependent destruction H0. apply ForSTS. dependent destruction H. assumption.
 * intros. constructor.
 * intros. dependent destruction H. assumption.
 * intros. apply ForRecursionSanity. dependent destruction H. assumption. assumption.
 * intros. inversion H1; subst. eapply IHTransition; eauto.
 * intros. inversion H1; subst. eapply IHTransition; eauto.
+* intros. inversion H; subst. constructor. eapply IHTransition; eauto. destruct μ; destruct a; destruct d; simpl in *.
+  + simpl. constructor.
+  + simpl. inversion H0.
+  + simpl. constructor.
+  + simpl. inversion H0.
+* intros. inversion H; subst. constructor. eapply IHTransition; eauto.
 * intros. dependent destruction H. constructor. 
   ** apply IHTransition1. assert (exists v', v = cst v'). eapply Output_are_good. exact H.
      exact Transition1. destruct H2. subst. constructor. assumption.
@@ -1467,6 +3252,7 @@ intros. dependent destruction a. dependent induction H.
 - exists c. exists d. reflexivity.
 - destruct (IHlts c d). reflexivity. destruct H1. dependent destruction H1. exists x. exists x0. reflexivity.
 - destruct (IHlts c d). reflexivity. destruct H1. dependent destruction H1. exists x. exists x0. reflexivity.
+- exists c. exists d. eauto.
 - destruct (IHlts c d). reflexivity. destruct H0. dependent destruction H0. exists x. exists x0. reflexivity.
 - destruct (IHlts c d). reflexivity. destruct H0. dependent destruction H0. exists x. exists x0. reflexivity.
 - destruct (IHlts c d). reflexivity. destruct H0. dependent destruction H0. exists x. exists x0. reflexivity.
@@ -1479,12 +3265,23 @@ intros. dependent destruction a. dependent induction H.
 - exists c. exists d. reflexivity.
 - destruct (IHlts c d). reflexivity. destruct H1. dependent destruction H1. exists x. exists x0.  reflexivity.
 - destruct (IHlts c d). reflexivity. destruct H1. dependent destruction H1. exists x. exists x0. reflexivity.
+- exists c. exists d. eauto.
 - destruct (IHlts c d). reflexivity. destruct H0. dependent destruction H0. exists x. exists x0. reflexivity.
 - destruct (IHlts c d). reflexivity. destruct H0. dependent destruction H0. exists x. exists x0. reflexivity.
 - destruct (IHlts c d). reflexivity. destruct H0. dependent destruction H0. exists x. exists x0. reflexivity.
 - destruct (IHlts c d). reflexivity. destruct H0. dependent destruction H0. exists x. exists x0. reflexivity.
 Qed.
 
+Lemma cgr_par_nil_n n r :  Ѵ n 𝟘 ‖ r ≡* r.
+Proof.
+  revert r. induction n.
+  - simpl. intros. eauto with cgr.
+  - simpl. intros. etrans. instantiate (1 := (𝟘 ‖ (ν Ѵ n 𝟘) ‖ r)).
+    eapply cgr_par. symmetry. etrans. eapply cgr_par_com. eapply cgr_par_nil.
+    etrans. eapply cgr_par. eapply cgr_par_com. etrans. eapply cgr_par.
+    eapply cgr_res_scope_rev. simpl. etrans. eapply cgr_par. eapply cgr_res. eauto.
+    etrans. eapply cgr_par. eapply cgr_res_nil. etrans. eapply cgr_par_com. eapply cgr_par_nil.
+Qed.
 
 (* Peter Selinger Axioms (OutBuffered Agent with FeedBack) up to structural equivalence*)
 
@@ -1492,16 +3289,29 @@ Lemma OBA_with_FB_First_Axiom : forall p q r a α,
   lts p (a !) q -> lts q α r ->
   (exists r', lts p α r' /\ lts_then_sc r' (a !) r). (* output-commutativity *)
 Proof.
-intros. assert (lts p (a !) q). assumption. apply OutputWithValue in H1.
-decompose record H1. subst. eapply TransitionShapeForOutputSimplified in H.
-eapply lts_parR in H0. instantiate (1 := (x ! x0 • 𝟘)) in H0.
-edestruct (Congruence_Respects_Transition p ((x ! x0 • 𝟘) ‖ r) α).
-exists ((x ! x0 • 𝟘) ‖ q). split; assumption. destruct H2.
-assert (lts ((x ! x0 • 𝟘) ‖ r) ((x ⋉ x0) !) (𝟘 ‖ r)). constructor. constructor.
-edestruct (Congruence_Respects_Transition x1 (𝟘 ‖ r) ((x ⋉ x0) !)).
-exists ((x ! x0 • 𝟘) ‖ r). split ; assumption. destruct H5.
-assert (x2 ≡* r). eauto with cgr.
-exists x1. split. assumption. exists x2. split; assumption.
+  intros. assert (lts p (a !) q). assumption. apply OutputWithValue in H1.
+  decompose record H1. subst. eapply TransitionShapeForOutputSimplified in H as (n & eq).
+  eapply lts_parR in H0. instantiate (1 := Ѵ n (VarC_add n x ! x0 • 𝟘)) in H0.
+  edestruct (Congruence_Respects_Transition p (Ѵ n (VarC_add n x ! x0 • 𝟘) ‖ r) α).
+  exists (Ѵ n (VarC_add n x ! x0 • 𝟘) ‖ q). split; assumption. destruct H.
+  assert (lts (Ѵ n (VarC_add n x ! x0 • 𝟘) ‖ r) ((x ⋉ x0) !) (Ѵ n 𝟘 ‖ r)). constructor.
+  eapply lts_res_ext_n. simpl. constructor.
+  edestruct (Congruence_Respects_Transition x1 (Ѵ n 𝟘 ‖ r) ((x ⋉ x0) !)).
+  exists (Ѵ n (VarC_add n x ! x0 • 𝟘) ‖ r). split ; assumption. destruct H4.
+  assert (x2 ≡* r). etrans. eauto. eapply cgr_par_nil_n.
+  exists x1. split. assumption. exists x2. split; assumption.
+Qed.
+
+Lemma simpl_output_res n c v p μ : lts (Ѵ n (VarC_add n c ! v • 𝟘)) (ActExt μ) p -> μ = ActOut (c ⋉ v) /\ p = Ѵ n 𝟘.
+Proof.
+  revert c v p μ.
+  induction n.
+  + simpl in * ; intros. rewrite VarC_add_zero in H. inversion H; eauto; split ;eauto.
+  + intros. simpl in *. inversion H. subst. replace (S n)%nat with (n + 1)%nat in H2 by lia.
+    rewrite VarC_add_revert_def in H2. simpl in *. eapply IHn in H2 as (eq1 & eq2).
+    subst. rewrite NewVarCzero_and_add in eq1.
+    replace (ActOut (VarC_add 1 c ⋉ v)) with (VarC_action_add 1 (ActOut (c ⋉ v))) in eq1 by eauto.
+    rewrite NewVarCzero_and_add in eq1. eapply NewVarC_in_ext_inv in eq1. subst. split ;eauto.
 Qed.
 
 Lemma OBA_with_FB_Second_Axiom : forall p q1 q2 a μ, 
@@ -1510,93 +3320,121 @@ Lemma OBA_with_FB_Second_Axiom : forall p q1 q2 a μ,
   lts p (ActExt μ) q2 ->
   ∃ r : proc, lts q1 (ActExt μ) r ∧ lts_then_sc q2 (a !) r. (* output-confluence  *)
 Proof.
-intros. assert (lts p (a !) q1). assumption. apply OutputWithValue in H2.
-decompose record H2. subst. rename x into c. rename x0 into v.
-eapply TransitionShapeForOutputSimplified in H0.
-edestruct (Congruence_Respects_Transition ((c ! v • 𝟘) ‖ q1) q2 (ActExt μ)).
-exists p. split. symmetry. assumption. assumption.
-destruct H3. inversion H3; subst.
-inversion H9. subst. now destruct H. 
-exists q3. split. assumption.
-assert (lts ((c ! v • 𝟘) ‖ q3) ((c ⋉ v) !) (𝟘 ‖ q3)). constructor. constructor.
-edestruct (Congruence_Respects_Transition q2 (𝟘 ‖ q3) ((c ⋉ v) !)).
-exists ((c ! v • 𝟘) ‖ q3). split. eauto with cgr. assumption. destruct H6. exists x. split. assumption.
-eauto with cgr.
+  intros. assert (lts p (a !) q1). assumption. apply OutputWithValue in H2.
+  decompose record H2. subst. rename x into c. rename x0 into v.
+  eapply TransitionShapeForOutputSimplified in H0 as (n & H0).
+  edestruct (Congruence_Respects_Transition (Ѵ n (VarC_add n c ! v • 𝟘) ‖ q1) q2 (ActExt μ)).
+  exists p. split. symmetry. assumption. assumption.
+  destruct H3. inversion H3; subst.
+  - assert (lts (Ѵ n (VarC_add n c ! v • 𝟘)) (ActExt μ) p2); eauto. eapply simpl_output_res in H9 as (eq1 & eq2). subst.
+    assert (ActOut (c ⋉ v) = ActOut (c ⋉ v)). eauto. exfalso. eapply H. eauto.
+  - exists q3. split. assumption.
+    assert (lts (Ѵ n (VarC_add n c ! v • 𝟘) ‖ q3) ((c ⋉ v) !) (Ѵ n 𝟘 ‖ q3)). constructor. eapply lts_res_ext_n. constructor.
+    edestruct (Congruence_Respects_Transition q2 (Ѵ n 𝟘 ‖ q3) ((c ⋉ v) !)).
+    exists (Ѵ n (VarC_add n c ! v • 𝟘) ‖ q3). split. eauto with cgr. assumption. destruct H6. exists x. split. assumption.
+    etrans. eauto. eapply cgr_par_nil_n.
 Qed.
 
 Lemma OBA_with_FB_Third_Axiom : forall p1 p2 p3 a, 
             lts p1 (a !) p2 → lts p1 (a !) p3 -> p2 ≡* p3. (* output-determinacy *)
 Proof.
-intros. assert (lts p1 (a !) p2). assumption. apply OutputWithValue in H1.
-decompose record H1. subst. rename x into c. rename x0 into v.
-revert H0. revert p3. dependent induction H.
-- intros. inversion H0. subst. eauto with cgr.
-- intros. inversion H2; subst.
-  + eapply IHlts; eauto.
-  + rewrite H in H8. inversion H8.
-- intros. inversion H2; subst.
-  + rewrite H in H8. inversion H8.
-  + eapply IHlts; eauto.
-- intros. inversion H0;subst. 
-  * apply cgr_fullpar. eapply IHlts. eauto. eauto. assumption. eauto with cgr.
-  * apply TransitionShapeForOutputSimplified in H.
-    apply TransitionShapeForOutputSimplified in H6.
-    apply transitivity with (p2 ‖ ((c ! v • 𝟘) ‖ q2)). eauto with cgr. 
-    apply transitivity with ((p2 ‖ (c ! v • 𝟘)) ‖ q2). eauto with cgr. apply cgr_par.
-    eauto with cgr.
-- intros. inversion H0 ; subst.
-  * apply TransitionShapeForOutputSimplified in H.
-    apply TransitionShapeForOutputSimplified in H6.
-    apply transitivity with (((c ! v • 𝟘) ‖ p2) ‖ q2). eauto with cgr.
-    apply transitivity with (( p2 ‖ (c ! v • 𝟘)) ‖ q2). eauto with cgr.
-    apply transitivity with ( p2 ‖ ((c ! v • 𝟘) ‖ q2)). eauto with cgr. apply cgr_fullpar. reflexivity.
-    eauto with cgr.
-  * apply cgr_fullpar. reflexivity. eapply IHlts. eauto. eauto. assumption.
-- intros. exfalso. eapply guarded_does_no_output. eassumption.
-- intros. exfalso. eapply guarded_does_no_output. eassumption.
-Qed.
+  intros. assert (lts p1 (a !) p2). assumption. apply OutputWithValue in H1.
+  decompose record H1. subst. rename x into c. rename x0 into v.
+  revert H0. revert p3. dependent induction H.
+  - intros. inversion H0. subst. eauto with cgr.
+  - intros. inversion H2; subst.
+    + eapply IHlts; eauto.
+    + rewrite H in H8. inversion H8.
+  - intros. inversion H2; subst.
+    + rewrite H in H8. inversion H8.
+    + eapply IHlts; eauto.
+  - intros. inversion H0;subst. eapply cgr_res. eapply (IHlts v (VarC_add 1 c)); eauto.
+  - intros. inversion H0;subst. 
+    * apply cgr_fullpar. eapply IHlts. eauto. eauto. assumption. eauto with cgr.
+    * (* apply TransitionShapeForOutputSimplified in H as (n & H).
+      apply TransitionShapeForOutputSimplified in H6 as (n' & H6).
+      apply transitivity with (p2 ‖ (Ѵ n (VarC_add n c ! v • 𝟘) ‖ q2)). eapply cgr_fullpar. 
+      reflexivity. exact H6. etrans. symmetry. eapply cgr_par_assoc.
+      eapply cgr_par. etrans. eapply cgr_par_com. symmetry. eauto. *) admit.
+  - intros. inversion H0 ; subst.
+    * (*apply TransitionShapeForOutputSimplified in H.
+      apply TransitionShapeForOutputSimplified in H6.
+      apply transitivity with (((c ! v • 𝟘) ‖ p2) ‖ q2). eauto with cgr.
+      apply transitivity with (( p2 ‖ (c ! v • 𝟘)) ‖ q2). eauto with cgr.
+      apply transitivity with ( p2 ‖ ((c ! v • 𝟘) ‖ q2)). eauto with cgr. apply cgr_fullpar. reflexivity.
+      eauto with cgr. *) admit.
+    * apply cgr_fullpar. reflexivity. eapply IHlts. eauto. eauto. assumption.
+  - intros. exfalso. eapply guarded_does_no_output. eassumption.
+  - intros. exfalso. eapply guarded_does_no_output. eassumption.
+Admitted.
 
 Lemma OBA_with_FB_Fourth_Axiom : forall p1 p2 p3 a, lts p1 (a !) p2 -> lts p2 (a ?) p3 
                               -> lts_then_sc p1 τ p3. (* feedback *)
 Proof.
-intros. assert (lts p1 (a !) p2). assumption. apply OutputWithValue in H1.
-decompose record H1. subst. rename x into c. rename x0 into v.
-eapply TransitionShapeForOutputSimplified in H.
-assert (lts (c ! v • 𝟘) ((c ⋉ v) !) 𝟘). constructor.
-assert (lts ((c ! v • 𝟘) ‖ p2) τ  (𝟘 ‖ p3)). econstructor; eassumption.
-edestruct (Congruence_Respects_Transition p1 (𝟘 ‖ p3) τ). exists ((c ! v • 𝟘) ‖ p2).
-split; assumption. destruct H4. exists x. split. assumption. eauto with cgr.
+  intros. assert (lts p1 (a !) p2). assumption. apply OutputWithValue in H1.
+  decompose record H1. subst. rename x into c. rename x0 into v.
+  eapply TransitionShapeForOutputSimplified in H as (n & H).
+  assert (lts (Ѵ n (VarC_add n c ! v • 𝟘)) ((c ⋉ v) !) (Ѵ n 𝟘)). eapply lts_res_ext_n.
+  constructor.
+  assert (lts (Ѵ n (VarC_add n c ! v • 𝟘) ‖ p2) τ  (Ѵ n 𝟘 ‖ p3)). econstructor; eassumption.
+  edestruct (Congruence_Respects_Transition p1 (Ѵ n 𝟘 ‖ p3) τ). exists (Ѵ n (VarC_add n c ! v • 𝟘) ‖ p2).
+  split; assumption. destruct H4. exists x. split. assumption. etrans. eauto. eapply cgr_par_nil_n.
 Qed.
 
 Lemma OBA_with_FB_Fifth_Axiom : forall p q1 q2 a,
   lts p (a !) q1 -> lts p τ q2 ->
   (∃ q : proc, lts q1 τ q /\ lts_then_sc q2 (a !) q) \/ lts_then_sc q1 (a ?) q2. (* output-tau  *)
 Proof.
-intros. assert (lts p (a !) q1). assumption. apply OutputWithValue in H1.
-decompose record H1. subst. rename x into c. rename x0 into v.
-eapply TransitionShapeForOutputSimplified in H.
-edestruct (Congruence_Respects_Transition ((c ! v • 𝟘) ‖ q1) q2 τ). exists p. split. eauto with cgr. assumption.
-destruct H2. dependent induction H2.
-- inversion H2_; subst. right. exists q0. split. assumption. eauto with cgr. 
-- inversion H2_0.
-- inversion H2.
-- left. exists q0. split. assumption. 
-  assert (lts ((c ! v • 𝟘) ‖ q0) ((c ⋉ v) !) (𝟘 ‖ q0)). constructor. constructor.
-  edestruct (Congruence_Respects_Transition q2 (𝟘 ‖ q0) ((c ⋉ v) !)). exists ((c ! v • 𝟘) ‖ q0).
-  split. eauto with cgr. assumption. destruct H5. exists x. split. assumption. eauto with cgr.
-Qed.
+  intros. assert (lts p (a !) q1). assumption. apply OutputWithValue in H1.
+  decompose record H1. subst. rename x into c. rename x0 into v.
+  eapply TransitionShapeForOutputSimplified in H as (n & H).
+  edestruct (Congruence_Respects_Transition (Ѵ n (VarC_add n c ! v • 𝟘) ‖ q1) q2 τ). exists p. split. eauto with cgr. assumption.
+  (* destruct H2. dependent induction H2.
+  - inversion H2_; subst. right. exists q0. split. assumption. eauto with cgr. 
+  - inversion H2_0.
+  - inversion H2.
+  - left. exists q0. split. assumption. 
+    assert (lts ((c ! v • 𝟘) ‖ q0) ((c ⋉ v) !) (𝟘 ‖ q0)). constructor. constructor.
+    edestruct (Congruence_Respects_Transition q2 (𝟘 ‖ q0) ((c ⋉ v) !)). exists ((c ! v • 𝟘) ‖ q0).
+    split. eauto with cgr. assumption. destruct H5. exists x. split. assumption. eauto with cgr. *) admit.
+Admitted.
 
 
 Lemma ExtraAxiom : forall p1 p2 q1 q2 a,
       lts p1 (a !) q1 -> lts p2 (a !) q2 -> q1 ≡* q2 -> p1 ≡* p2.
 Proof.
-intros. assert (lts p1 (a !) q1). assumption. apply OutputWithValue in H2.
-decompose record H2. subst. rename x into c. rename x0 into v.
-eapply TransitionShapeForOutputSimplified in H0.
-eapply TransitionShapeForOutputSimplified in H.
-apply transitivity with ((c ! v • 𝟘) ‖ q1). assumption.
-apply transitivity with ((c ! v • 𝟘) ‖ q2). eauto with cgr. eauto with cgr.
-Qed. 
+  intros. assert (lts p1 (a !) q1). assumption. apply OutputWithValue in H2.
+  decompose record H2. subst. rename x into c. rename x0 into v.
+  eapply TransitionShapeForOutputSimplified in H0 as (n' & H0).
+  eapply TransitionShapeForOutputSimplified in H as (n & H).
+  (* apply transitivity with ((c ! v • 𝟘) ‖ q1). assumption.
+  apply transitivity with ((c ! v • 𝟘) ‖ q2). eauto with cgr. eauto with cgr. *) admit.
+Admitted.
+
+Definition encode_channeldata (C : ChannelData) : gen_tree (nat + Channel) :=
+match C with
+  | cstC c => GenLeaf (inr c)
+  | bvarC i => GenLeaf (inl i)
+end.
+
+Definition decode_channeldata (tree : gen_tree (nat + Channel)) : ChannelData :=
+match tree with
+  | GenLeaf (inr c) => cstC c
+  | GenLeaf (inl i) => bvarC i
+  | _ => bvarC 0
+end.
+
+Lemma encode_decide_channeldatas c : decode_channeldata (encode_channeldata c) = c.
+Proof. case c. 
+* intros. simpl. reflexivity.
+* intros. simpl. reflexivity.
+Qed.
+
+#[global] Instance channeldata_countable : Countable ChannelData.
+Proof.
+  refine (inj_countable' encode_channeldata decode_channeldata _).
+  apply encode_decide_channeldatas.
+Qed.
 
 Definition encode_data (D : Data) : gen_tree (nat + Value) :=
 match D with
@@ -1677,12 +3515,12 @@ Qed.
 
 #[global] Instance proc_eqdecision : EqDecision proc. by exact proc_dec. Defined.
 
-Definition encode_TypeOfActions (a : TypeOfActions) : gen_tree (nat + (Channel + Data)) :=
+Definition encode_TypeOfActions (a : TypeOfActions) : gen_tree (nat + (ChannelData + Data)) :=
 match a with
   | act c v => GenNode 0 [GenLeaf (inr (inl c)) ; GenLeaf (inr (inr v))]
 end.
 
-Definition decode_TypeOfActions (tree :gen_tree (nat + (Channel + Data))) : option TypeOfActions :=
+Definition decode_TypeOfActions (tree :gen_tree (nat + (ChannelData + Data))) : option TypeOfActions :=
 match tree with
   | GenNode 0 [GenLeaf (inr (inl c)); GenLeaf (inr (inr v))] => Some (act c v)
   | _ => None
@@ -1700,17 +3538,62 @@ Proof.
   intro. apply encode_decide_TypeOfActions.
 Qed.
 
-Fixpoint encode_proc (p: proc) : gen_tree (nat + (((Equation Data ) + TypeOfActions) + Channel)) :=
+Definition encode_ExtAct_TypeOfActions (a : ExtAct TypeOfActions) : 
+    gen_tree (nat + (ChannelData + Data)) :=
+match a with
+  | ActIn a => GenNode 0 [encode_TypeOfActions a]
+  | ActOut a => GenNode 1 [encode_TypeOfActions a]
+end.
+
+Definition decode_ExtAct_TypeOfActions_raw (tree :gen_tree (nat + (ChannelData + Data))) 
+  : option (ExtAct (option TypeOfActions)) :=
+match tree with
+  | GenNode 0 [l] => Some (ActIn (decode_TypeOfActions l))
+  | GenNode 1 [l] => Some (ActOut (decode_TypeOfActions l))
+  | _ => None
+end.
+
+Definition simpl_option (a : option (ExtAct (option TypeOfActions)))
+  : option (ExtAct TypeOfActions) :=
+match a with
+  | Some (ActIn None) => None
+  | Some (ActIn (Some b)) => Some (ActIn b)
+  | Some (ActOut None) => None
+  | Some (ActOut (Some b)) => Some (ActOut b)
+  | None => None
+end.
+
+Definition decode_ExtAct_TypeOfActions (tree :gen_tree (nat + (ChannelData + Data))) 
+  : option (ExtAct TypeOfActions) := simpl_option (decode_ExtAct_TypeOfActions_raw tree).
+
+Lemma encode_decide_ExtAct_TypeOfActions a : 
+  decode_ExtAct_TypeOfActions (encode_ExtAct_TypeOfActions  a) = Some a.
+Proof. 
+induction a. 
+* unfold decode_ExtAct_TypeOfActions. simpl.
+  rewrite encode_decide_TypeOfActions. eauto.
+* unfold decode_ExtAct_TypeOfActions. simpl.
+  rewrite encode_decide_TypeOfActions. eauto.
+Qed.
+
+#[global] Instance ExtAct_TypeOfActions_countable : Countable (ExtAct TypeOfActions).
+Proof.
+  eapply inj_countable with encode_ExtAct_TypeOfActions decode_ExtAct_TypeOfActions. 
+  intro. apply encode_decide_ExtAct_TypeOfActions.
+Qed.
+
+Fixpoint encode_proc (p: proc) : gen_tree (nat + (((Equation Data ) + TypeOfActions) + ChannelData)) :=
   match p with
   | p ‖ q  => GenNode 0 [encode_proc p; encode_proc q]
   | c ! v • 𝟘  => GenLeaf (inr $ inl $ inr $ (c ⋉ v))
   | pr_var i => GenNode 2 [GenLeaf $ inl i]
   | rec x • P => GenNode 3 [GenLeaf $ inl x; encode_proc P]
   | If C Then A Else B => GenNode 4 [GenLeaf (inr ( inl (inl C))) ; encode_proc A; encode_proc B]
+  | ν p => GenNode 5 [encode_proc p]
   | g gp => GenNode 1 [encode_gproc gp]
   end
 with
-encode_gproc (gp: gproc) : gen_tree (nat + (((Equation Data ) + TypeOfActions) + Channel)) :=
+encode_gproc (gp: gproc) : gen_tree (nat + (((Equation Data ) + TypeOfActions) + ChannelData)) :=
   match gp with
   | ① => GenNode 1 []
   | 𝟘 => GenNode 0 []
@@ -1718,29 +3601,21 @@ encode_gproc (gp: gproc) : gen_tree (nat + (((Equation Data ) + TypeOfActions) +
   | t • p => GenNode 3 [encode_proc p]
   | gp + gq => GenNode 4 [encode_gproc gp; encode_gproc gq]
   end.
-  
-Definition Channel_of (a : TypeOfActions) : Channel := 
-match a with 
-| act c d => c
-end.
 
-Definition Data_of (a : TypeOfActions) : Data := 
-match a with 
-| act c d => d
-end.
 
-Fixpoint decode_proc (t': gen_tree (nat + (((Equation Data ) + TypeOfActions) + Channel))) : proc :=
+Fixpoint decode_proc (t': gen_tree (nat + (((Equation Data ) + TypeOfActions) + ChannelData))) : proc :=
   match t' with
   | GenNode 0 [ep; eq] => (decode_proc ep) ‖ (decode_proc eq)
-  | GenLeaf (inr ( inl (inr a))) => (Channel_of a) ! (Data_of a) • 𝟘
+  | GenLeaf (inr ( inl (inr a))) => (ChannelData_of a) ! (Data_of a) • 𝟘
   | GenNode 2 [GenLeaf (inl i)] => pr_var i
   | GenNode 3 [GenLeaf (inl i); egq] => rec i • (decode_proc egq)
   | GenNode 4 [GenLeaf (inr ( inl (inl C))); A; B] => If C Then (decode_proc A) Else (decode_proc B)
+  | GenNode 5 [eq] => ν (decode_proc eq)
   | GenNode 1 [egp] => g (decode_gproc egp)
   | _ => ① 
   end
 with
-decode_gproc (t': gen_tree (nat + (((Equation Data ) + TypeOfActions) + Channel))): gproc :=
+decode_gproc (t': gen_tree (nat + (((Equation Data ) + TypeOfActions) + ChannelData))): gproc :=
   match t' with
   | GenNode 1 [] => ①
   | GenNode 0 [] => 𝟘
@@ -1758,6 +3633,7 @@ Proof. all: case p.
 * intros. simpl. rewrite (encode_decide_procs p0). reflexivity.
 * intros. simpl. rewrite (encode_decide_procs p0). rewrite (encode_decide_procs p1). reflexivity.
 * intros. simpl. reflexivity.
+* intros. simpl. rewrite (encode_decide_procs p0). eauto.
 * intros. simpl. rewrite (encode_decide_gprocs g0). reflexivity.
 * intros. simpl. reflexivity. 
 * intros. simpl. reflexivity. 
@@ -1770,62 +3646,278 @@ Qed.
 refine (inj_countable' encode_proc decode_proc _).
   apply encode_decide_procs.
 Qed.
-#[global] Instance Singletons_of_TypeOfActions : SingletonMS TypeOfActions (gmultiset TypeOfActions) 
+(* #[global] Instance Singletons_of_TypeOfActions : SingletonMS TypeOfActions (gmultiset TypeOfActions) 
 :=gmultiset_singleton.
 #[global] Instance Singletons_of_proc : Singleton proc (gset proc) := gset_singleton.
 #[global] Instance Empty_of_proc : Empty (gset proc) := gset_empty.
 #[global] Instance Union_of_proc : Union (gset proc) := gset_union.
-#[global] Instance SemiSet_of_proc : SemiSet proc (gset proc) := gset_semi_set.
+#[global] Instance SemiSet_of_proc : SemiSet proc (gset proc) := gset_semi_set. *)
 
 (* Next Obligations *)
-Fixpoint moutputs_of p : gmultiset TypeOfActions := 
+Fixpoint moutputs_of (k : nat) p : gmultiset TypeOfActions := 
 match p with
-  | P ‖ Q => (moutputs_of P) ⊎ (moutputs_of Q)
+  | P ‖ Q => (moutputs_of k P) ⊎ (moutputs_of k Q)
   | pr_var _ => ∅
   | rec _ • _ => ∅
   | If E Then P Else Q => match (Eval_Eq E) with 
-                          | Some true => moutputs_of P
-                          | Some false => moutputs_of Q
+                          | Some true => moutputs_of k P
+                          | Some false => moutputs_of k Q
                           | None => ∅
                           end
-  | c ! v • 𝟘 => {[+ c ⋉ v +]}
+  | (cstC c) ! v • 𝟘 => {[+ ((cstC c) ⋉ v) +]}
+  | (bvarC i) ! v • 𝟘 => if decide(k < (S i)) then {[+ ((bvarC (i - k)) ⋉ v) +]}
+                                            else ∅
+  | ν p => moutputs_of (S k) p
   | g _ => ∅
-end.  
-Definition outputs_of p := dom (moutputs_of p).
+end.
 
-Lemma mo_equiv_spec_step : forall {p q}, p ≡ q -> moutputs_of p = moutputs_of q.
-Proof. intros. dependent induction H ; try multiset_solver; simpl in *; try rewrite H; eauto.
-+ destruct (Eval_Eq C); eauto. destruct b; eauto.
-+ destruct (Eval_Eq C); eauto. destruct b; eauto.
-Qed.
+Definition outputs_of p := dom (moutputs_of 0 p).
 
-Lemma mo_equiv_spec : forall {p q}, p ≡* q -> moutputs_of p = moutputs_of q.
+Lemma VarSwap_and_moutputs j p k : moutputs_of (j + S (S k)) p =
+moutputs_of (j + S (S k)) (VarSwap_in_proc j p).
 Proof.
-  intros p q hcgr.
-  induction hcgr. now eapply mo_equiv_spec_step.
-  etrans; eauto.
+  revert j k.
+  induction p as (p & Hp) using
+    (well_founded_induction (wf_inverse_image _ nat _ size Nat.lt_wf_0)).
+  destruct p; intros; simpl in *; try multiset_solver.
+  + assert (moutputs_of (j + S (S k)) p1 
+      = moutputs_of (j + S (S k)) (VarSwap_in_proc j p1)) as eq1. 
+    { eapply Hp. simpl. lia. }
+    assert (moutputs_of (j + S (S k)) p2 
+      = moutputs_of (j + S (S k)) (VarSwap_in_proc j p2)) as eq2. 
+    { eapply Hp. simpl. lia. }
+    rewrite eq1, eq2. eauto. 
+  + case_eq (Eval_Eq e); intros; try multiset_solver.
+    destruct b.
+    ++ eapply Hp. simpl. lia.
+    ++ eapply Hp. simpl. lia.
+  + destruct c.
+      * simpl. eauto.
+      * simpl. destruct (decide (j + S (S k) < S n)).
+        ++ destruct (decide (n = j)); subst.
+           +++ rewrite decide_True ; try lia.
+           +++ destruct (decide (n = S j)); subst.
+               ++++ destruct (decide (j + S (S k) < S j)).
+                    +++++ lia.
+                    +++++ lia.
+               ++++ rewrite decide_True ; try lia. eauto.
+        ++ destruct (decide (n = j)); subst.
+           +++ rewrite decide_False ; try lia. eauto.
+           +++ destruct (decide (n = S j)); subst.
+               ++++ rewrite decide_False ; try lia. eauto.
+               ++++ rewrite decide_False ; try lia. eauto.
+  + replace (S (j + S (S k)))%nat with ((S j) + S (S k))%nat by lia. eauto. 
 Qed.
 
-Lemma mo_spec p a q : lts p (a !) q -> moutputs_of p = {[+ a +]} ⊎ moutputs_of q.
+Lemma NewVarC_and_moutputs p j : moutputs_of (S j) (NewVarC j p) = moutputs_of j p.
+Proof.
+  revert j.
+  induction p as (p & Hp) using
+    (well_founded_induction (wf_inverse_image _ nat _ size Nat.lt_wf_0)).
+  destruct p; intros; simpl in *; try multiset_solver.
+  + assert (moutputs_of (S j) (NewVarC j p1)
+      = moutputs_of j p1 ) as eq1. 
+    { eapply Hp. simpl. lia. }
+    assert (moutputs_of (S j) (NewVarC j p2)
+      = moutputs_of j p2) as eq2. 
+    { eapply Hp. simpl. lia. }
+    rewrite eq1, eq2. eauto. 
+  + case_eq (Eval_Eq e); intros; try multiset_solver.
+    destruct b.
+    ++ eapply Hp. simpl. lia.
+    ++ eapply Hp. simpl. lia.
+  + destruct c.
+      * simpl. eauto.
+      * simpl. destruct (decide (j < S n)).
+        ++ rewrite decide_True; try lia. eauto.
+        ++ rewrite decide_False; try lia. eauto.
+Qed.
+
+Lemma simpl_bvar_in_NewVar_ChannelData j c : NewVar_in_ChannelData j (NewVar_in_ChannelData j c) 
+        = NewVar_in_ChannelData (S j) (NewVar_in_ChannelData j c).
+Proof.
+  destruct c.
+  + simpl. eauto.
+  + simpl. destruct (decide (j < S n)).
+    ++ simpl. rewrite decide_True; try lia.
+       rewrite decide_True; try lia. eauto.
+    ++ simpl. rewrite decide_False; try lia.
+       rewrite decide_False; try lia. eauto.
+Qed.
+
+Lemma simpl_bvar_in_NewVarC j p : NewVarC j (NewVarC j p) = NewVarC (S j) (NewVarC j p).
+Proof.
+  revert j.
+  induction p as (p & Hp) using
+    (well_founded_induction (wf_inverse_image _ nat _ size Nat.lt_wf_0)).
+  destruct p; intros; simpl in *.
+  + assert ((NewVarC j (NewVarC j p1)) = (NewVarC (S j) (NewVarC j p1))) as eq1.
+    { eapply Hp. simpl. lia. }
+    assert ((NewVarC j (NewVarC j p2)) = (NewVarC (S j) (NewVarC j p2))) as eq2.
+    { eapply Hp. simpl. lia. }
+    rewrite eq1, eq2. eauto.
+  + eauto.
+  + f_equal. eapply Hp. simpl; eauto.
+  + assert ((NewVarC j (NewVarC j p1)) = (NewVarC (S j) (NewVarC j p1))) as eq1.
+    { eapply Hp. simpl. lia. }
+    assert ((NewVarC j (NewVarC j p2)) = (NewVarC (S j) (NewVarC j p2))) as eq2.
+    { eapply Hp. simpl. lia. }
+    rewrite eq1, eq2. eauto.
+  + rewrite simpl_bvar_in_NewVar_ChannelData. eauto.
+  + f_equal. eapply Hp. simpl; eauto.
+  + destruct g0; simpl in *.
+    - eauto.
+    - eauto.
+    - rewrite simpl_bvar_in_NewVar_ChannelData.
+      assert ((NewVarC j (NewVarC j p)) = (NewVarC (S j) (NewVarC j p))) as eq.
+      { eapply Hp. simpl. eauto. }
+      rewrite eq. eauto.
+    - assert ((NewVarC j (NewVarC j p)) = (NewVarC (S j) (NewVarC j p))) as eq.
+      { eapply Hp. simpl. eauto. }
+      rewrite eq. eauto.
+    - assert (NewVarC j (NewVarC j (g g0_1)) = NewVarC (S j) (NewVarC j (g g0_1))) as eq1.
+      { eapply Hp. simpl. lia. }
+      assert (NewVarC j (NewVarC j (g g0_2)) = NewVarC (S j) (NewVarC j (g g0_2))) as eq2.
+      { eapply Hp. simpl. lia. }
+      inversion eq1. inversion eq2. eauto.
+Qed.
+
+Lemma simpl_bvar_in_NewVarCn j k p :(NewVarCn j k (NewVarC j p) = NewVarCn (S j) k (NewVarC j p)).
+Proof.
+  revert p j.
+  induction k.
+  - simpl; eauto.
+  - intros; simpl. rewrite<- (NewVarCn_revert_def k _ j). rewrite IHk.
+    rewrite<- (NewVarCn_revert_def k _ (S j)). f_equal.
+    replace (NewVarC j (NewVarCn j k (NewVarC j p))) with (NewVarCn j 1 (NewVarCn j k (NewVarC j p))).
+    2 : { eauto. } rewrite simpl_bvar_in_NewVarC. eauto.
+Qed.
+
+Lemma NewVarCn_and_moutputs j p k : moutputs_of j p =
+moutputs_of (k + j) (NewVarCn j k p).
+Proof.
+  revert p j.
+  induction k.
+  + simpl; eauto.
+  + intros. simpl. rewrite<- NewVarCn_revert_def.
+    replace (S (k + j))%nat with (k + (S j))%nat by lia.
+    assert ((NewVarCn j k (NewVarC j p)) = (NewVarCn (S j) k (NewVarC j p))) as eq.
+    { rewrite simpl_bvar_in_NewVarCn. eauto. } rewrite eq. rewrite<- (IHk  (NewVarC j p)).
+    rewrite NewVarC_and_moutputs. eauto.
+Qed.
+
+Lemma moutputs_and_NewVar k p j : moutputs_of (k + j) p = moutputs_of (k + S j) (NewVarC j p).
+Proof.
+  revert j k.
+  induction p as (p & Hp) using
+    (well_founded_induction (wf_inverse_image _ nat _ size Nat.lt_wf_0)).
+  destruct p; intros; simpl in *.
+  + assert (moutputs_of (k + j) p1 = moutputs_of (k + S j) (NewVarC j p1)) as eq1.
+    { eapply Hp. lia. }
+    assert (moutputs_of (k + j) p2 = moutputs_of (k + S j) (NewVarC j p2)) as eq2.
+    { eapply Hp. lia. }
+    rewrite eq1, eq2. eauto.
+  + eauto.
+  + eauto.
+  + assert (moutputs_of (k + j) p1 = moutputs_of (k + S j) (NewVarC j p1)) as eq1.
+    { eapply Hp. lia. }
+    assert (moutputs_of (k + j) p2 = moutputs_of (k + S j) (NewVarC j p2)) as eq2.
+    { eapply Hp. lia. }
+    rewrite eq1, eq2. eauto.
+  + destruct c.
+      * simpl. eauto.
+      * destruct (decide (k + j < S n)).
+        ++ simpl. rewrite decide_True; try lia.
+           rewrite decide_True; try lia.
+           replace ((S n - (k + S j)))%nat with (n - (k + j))%nat by lia.
+           eauto.
+        ++ simpl. destruct (decide (j < S n)).
+           +++ rewrite decide_False; try lia. eauto.
+           +++ rewrite decide_False; try lia. eauto.
+  + replace ((S (k + j)))%nat with (k + S j)%nat by lia.
+    replace (S (k + S j))%nat with (k + S (S j))%nat by lia.
+    eapply Hp. simpl. eauto.
+  + eauto.
+Qed.
+
+Lemma NewVarCn_and_moutputs2 j p k : moutputs_of k p =
+moutputs_of (j + k) (NewVarCn 0 j p).
+Proof.
+  revert p k.
+  induction j.
+  + intros; simpl; eauto.
+  + intros. simpl. rewrite<- NewVarCn_revert_def.
+    replace (S (j+ k))%nat with (j + (S k))%nat by lia.
+    rewrite<- (IHj (NewVarC 0 p)).
+    assert ((NewVarCn j k (NewVarC j p)) = (NewVarCn (S j) k (NewVarC j p))) as eq.
+    { rewrite simpl_bvar_in_NewVarCn. eauto. } replace k%nat with (k + 0)%nat by lia.
+    rewrite moutputs_and_NewVar. replace (k + 1)%nat with (S k)%nat by lia.
+    replace (S (k + 0))%nat with (S k)%nat by lia. eauto.
+Qed.
+
+Lemma mo_equiv_spec_step : forall {p q k}, p ≡ q -> moutputs_of k p = moutputs_of k q.
+Proof. intros. revert k. dependent induction H ; try multiset_solver; simpl in *; try rewrite H; eauto.
++ intros. replace (S (S k))%nat with (0 + (S (S k)))%nat by lia. rewrite VarSwap_and_moutputs. eauto.
++ intros. replace (S (S k))%nat with (0 + (S (S k)))%nat by lia. symmetry. rewrite VarSwap_and_moutputs. eauto.
++ intros. f_equal. replace (NewVarC 0 q) with (NewVarCn 0 1 q); eauto.
+  replace (S k)%nat with (1 + k)%nat; eauto. rewrite<- NewVarCn_and_moutputs2. eauto.
++ intros. f_equal. replace (NewVarC 0 q) with (NewVarCn 0 1 q); eauto.
+  replace (S k)%nat with (1 + k)%nat; eauto. rewrite<- NewVarCn_and_moutputs2. eauto.
++ destruct (Eval_Eq C); eauto. destruct b; eauto.
++ destruct (Eval_Eq C); eauto. destruct b; eauto.
+Qed.
+
+Lemma mo_equiv_spec : forall {p q k}, p ≡* q -> moutputs_of k p = moutputs_of k q.
+Proof.
+  intros p q l hcgr.
+  induction hcgr.
+  - now eapply mo_equiv_spec_step.
+  - etrans; eauto.
+Qed.
+
+Lemma simpl_new_output n k c v : moutputs_of k (c ! v • 𝟘) = moutputs_of k (Ѵ n (VarC_add n c ! v • 𝟘)).
+Proof.
+  revert k c v.
+  induction n.
+  - intros; simpl; eauto. destruct c; simpl; eauto.
+  - intros; simpl. destruct c ; simpl.
+    + replace (c ! v • 𝟘) with (VarC_add n c ! v • 𝟘) by eauto.
+      rewrite<- IHn. simpl. eauto.
+    + destruct (decide (k < S n0)).
+      ++ replace (S (n + n0))%nat with (n + S n0)%nat by lia.
+         replace ((n + S n0)%nat ! v • 𝟘) with (VarC_add n (S n0) ! v • 𝟘) by (simpl; eauto). rewrite<- IHn.
+         simpl. rewrite decide_True; try lia. eauto.
+      ++ replace (S (n + n0))%nat with (n + S n0)%nat by lia.
+         replace ((n + S n0)%nat ! v • 𝟘) with (VarC_add n (S n0) ! v • 𝟘) by (simpl; eauto). rewrite<- IHn.
+         simpl. rewrite decide_False; try lia. eauto.
+Qed.
+
+Lemma mo_spec p a q : lts p (a !) q -> moutputs_of 0 p = {[+ a +]} ⊎ moutputs_of 0 q.
 Proof.
   intros l. assert (lts p (a !) q). assumption. apply OutputWithValue in H.
   decompose record H. subst. rename x into c. rename x0 into v.
-  eapply TransitionShapeForOutputSimplified, mo_equiv_spec in l. simpl in l. eauto.
+  eapply TransitionShapeForOutputSimplified in l as (n & l). eapply mo_equiv_spec in l. simpl in l.
+  rewrite l. f_equal. rewrite<- simpl_new_output. simpl. destruct c; eauto.
+  replace (n0 - 0)%nat with n0%nat; try lia. eauto.
 Qed.
 
-Lemma mo_spec_l e a :
-  a ∈ moutputs_of e -> {e' | lts e (ActExt $ ActOut a) e' /\ moutputs_of e' = moutputs_of e ∖ {[+ a +]}}.
+Lemma mo_spec_l e a k :
+  a ∈ moutputs_of k e -> {e' | lts (Ѵ  k e) (ActExt $ ActOut a) (Ѵ  k e') /\ moutputs_of k e' = moutputs_of k e ∖ {[+ a +]}}.
 Proof.
   intros mem.
   dependent induction e.
   + cbn in mem.
-    destruct (decide (a ∈ moutputs_of e1)).
-    destruct (IHe1 a e) as (e1' & lts__e1 & eq).
+    destruct (decide (a ∈ moutputs_of k e1)).
+    destruct (IHe1 a k e) as (e1' & lts__e1 & eq).
     exists (pr_par e1' e2). repeat split; eauto with ccs.
+    eapply inversion_res_ext in lts__e1. eapply lts_res_ext_n.
+    eapply lts_parL. eauto.
     multiset_solver.
-    destruct (decide (a ∈ moutputs_of e2)).
-    destruct (IHe2 a e) as (e2' & lts__e2 & eq).
+    destruct (decide (a ∈ moutputs_of k e2)).
+    destruct (IHe2 a k e) as (e2' & lts__e2 & eq).
     exists (pr_par e1 e2'). repeat split; eauto with ccs.
+    eapply inversion_res_ext in lts__e2. eapply lts_res_ext_n.
+    eapply lts_parR. eauto.
     multiset_solver.
     contradict mem. intro mem. multiset_solver.
   + exfalso. multiset_solver.
@@ -1833,37 +3925,53 @@ Proof.
   + simpl in *. case_eq (Eval_Eq e1); intros.
     ++ rewrite H in mem. destruct b.
        +++ eapply IHe1 in mem as (e' & l & eq).
-           exists e'. split ;eauto. eapply lts_ifOne; eauto.
+           exists e'. split ;eauto. eapply lts_res_ext_n. eapply lts_ifOne; eauto.
+           eapply inversion_res_ext. eauto.
        +++ eapply IHe2 in mem as (e' & l & eq).
-           exists e'. split ;eauto. eapply lts_ifZero; eauto.
+           exists e'. split ;eauto. eapply lts_res_ext_n. eapply lts_ifZero; eauto.
+           eapply inversion_res_ext. eauto.
     ++ rewrite H in mem. exfalso. inversion mem.
   + exists (g 𝟘).
-    assert (a = c ⋉ d). multiset_solver. subst.
-    repeat split; eauto with ccs. multiset_solver.
+    destruct c.
+    ++ simpl in *.
+       assert (a = c ⋉ d). multiset_solver. subst.
+       repeat split; eauto with ccs. eapply lts_res_ext_n. simpl. constructor. multiset_solver.
+    ++ simpl in *. destruct (decide (k < S n)).
+       +++ split. eapply lts_res_ext_n. simpl. destruct a. assert (c ⋉ d0 = (n - k) ⋉ d). multiset_solver.
+           inversion H; subst. simpl in *. replace (k + (n - k))%nat with n%nat by lia. constructor.
+           multiset_solver.
+       +++ inversion mem.
+  + simpl in *. eapply IHe in mem as (e' & eq1 & eq2).
+    exists (ν e'). split. rewrite BigNew_reverse_def_one. rewrite BigNew_reverse_def_one.
+    simpl in *; eauto. simpl. eauto.
   + simpl in mem. exfalso. set_solver. 
 Qed.
 
-Lemma mo_spec_r e a :
-  {e' | lts e (ActExt $ ActOut a) e' /\ moutputs_of e' = moutputs_of e ∖ {[+ a +]}} -> a ∈ moutputs_of e.
+Lemma mo_spec_r e a k:
+  {e' | lts (Ѵ  k e) (ActExt $ ActOut a) (Ѵ  k e') /\ moutputs_of k e' = moutputs_of k e ∖ {[+ a +]}} -> a ∈ moutputs_of k e.
 Proof.
   dependent induction e; intros (e' & l & mem).
-  + cbn.
+  + cbn. eapply inversion_res_ext in l.
     inversion l; subst.
     eapply gmultiset_elem_of_disj_union. left.
-    eapply IHe1. exists p2. split.
-    eassumption. cbn in mem. multiset_solver.
+    eapply IHe1. exists p2. split. eapply lts_res_ext_n; eauto. cbn in mem.
+    multiset_solver.
     eapply gmultiset_elem_of_disj_union. right.
-    eapply IHe2. exists q2. split.
-    eassumption. cbn in mem. multiset_solver.
-  + inversion l.
-  + inversion l.
-  + inversion l; subst; simpl in *; rewrite H4 in mem; rewrite H4.
-    ++ eapply IHe1 ; eauto.
-    ++ eapply IHe2 ; eauto.
-  + inversion l; subst. set_solver.
-  + destruct a. now eapply guarded_does_no_output in l.
+    eapply IHe2. exists q2. split. eapply lts_res_ext_n; eauto. cbn in mem.
+    multiset_solver.
+  + eapply inversion_res_ext in l. inversion l.
+  + eapply inversion_res_ext in l. inversion l.
+  + eapply inversion_res_ext in l. inversion l; subst; simpl in *; rewrite H4 in mem; rewrite H4.
+    ++ destruct a. eapply IHe1 ; eauto. exists e'. split. eapply lts_res_ext_n. simpl; eauto. multiset_solver.
+    ++ destruct a. eapply IHe2 ; eauto. exists e'. split. eapply lts_res_ext_n. simpl; eauto. multiset_solver.
+  + eapply inversion_res_ext in l. inversion l; subst. destruct a.
+    inversion H; subst. destruct c0.
+    ++ simpl. subst. multiset_solver.
+    ++ simpl. rewrite decide_True; try lia. replace (k + n - k)%nat with n%nat by lia. multiset_solver.
+  + eapply inversion_res_ext in l. inversion l; subst. destruct a. simpl. eapply IHe. exists p'. split.
+    eapply lts_res_ext_n. simpl in *. rewrite<- VarC_add_revert_def in H1. simpl in *. eauto. multiset_solver.
+  + destruct a. simpl in *. eapply inversion_res_ext in l. now eapply guarded_does_no_output in l.
 Qed.
-
 
 Lemma outputs_of_spec2 p a : a ∈ outputs_of p -> {q | lts p (ActExt (ActOut a)) q}.
 Proof.
@@ -1875,7 +3983,7 @@ Qed.
 
 Lemma outputs_of_spec1_zero (p : proc) (a : TypeOfActions) : {q | lts p (ActExt (ActOut a)) q} 
       -> a ∈ outputs_of p.
-Proof.    
+Proof.
   intros (p' & lts__p).
   dependent induction p.
   + eapply gmultiset_elem_of_dom.
@@ -1886,11 +3994,15 @@ Proof.
   + inversion lts__p; subst ; eapply gmultiset_elem_of_dom; simpl in *; rewrite H4.
     ++ eapply gmultiset_elem_of_dom. eapply IHp1; eauto.
     ++ eapply gmultiset_elem_of_dom. eapply IHp2; eauto.
-  + inversion lts__p; subst. unfold outputs_of. multiset_solver.
+  + inversion lts__p; subst. unfold outputs_of. eapply gmultiset_elem_of_dom. eapply mo_spec_r; exists 𝟘 ; simpl; eauto.
+    split. eauto. destruct c. multiset_solver. replace (n - 0)%nat with n%nat by lia. multiset_solver.
+  + inversion lts__p; subst. eapply gmultiset_elem_of_dom. simpl. eapply mo_spec_r. exists p'0.
+    split; eauto. replace (VarC_action_add 1 (ActOut a)) with (ActOut (VarC_TypeOfActions_add 1 a)) in H1. eapply mo_spec in H1.
+    admit. simpl. destruct a. simpl. eauto.
   + assert (lts g0 (a !) p'). assumption. apply OutputWithValue in H.
     decompose record H. subst. rename x into c. rename x0 into v.
     now eapply guarded_does_no_output in lts__p.
-Qed.
+Admitted.
 
 Lemma outputs_of_spec1 (p : proc) (a : TypeOfActions) (q : proc) : lts p (ActExt (ActOut a)) q
       -> a ∈ outputs_of p.
@@ -1913,18 +4025,19 @@ match p with
                           | None => ∅
                           end
   | c ! v • 𝟘 => if decide(a = (c ⋉ v)) then {[ (g 𝟘) ]} else ∅
+  | ν p => list_to_set (map (fun q => ν q) (elements $ lts_set_output p (VarC_TypeOfActions_add 1 a))) 
   | g _  => ∅
 end.
 
 Fixpoint lts_set_input_g (g : gproc) (a : TypeOfActions) : gset proc :=
   match g with
-  | c ? x • p => if decide(Channel_of a = c) then {[ p^(Data_of a) ]} else ∅
+  | c ? x • p => if decide(ChannelData_of a = c) then {[ p^(Data_of a) ]} else ∅
   | g1 + g2 => lts_set_input_g g1 a ∪ lts_set_input_g g2 a
   | ① => ∅
   | 𝟘 => ∅
   | t • p => ∅
   end.
-  
+
 Fixpoint lts_set_input (p : proc) (a : TypeOfActions) : gset proc :=
 match p with
   | p1 ‖ p2 =>
@@ -1939,9 +4052,10 @@ match p with
                           | Some false => lts_set_input B a
                           | None => ∅
                           end
+  | ν p => list_to_set (map (fun q => ν q) (elements $ lts_set_input p (VarC_TypeOfActions_add 1 a))) 
   | g gp => lts_set_input_g gp a  
   end.
-  
+
 Fixpoint lts_set_tau_g (gp : gproc) : gset proc :=
 match gp with
   | c ? x • p => ∅
@@ -1950,7 +4064,6 @@ match gp with
   | t • p => {[ p ]}
   | gp1 + gp2 => lts_set_tau_g gp1 ∪ lts_set_tau_g gp2
 end.
-
 
 
 Fixpoint lts_set_tau (p : proc) : gset proc :=
@@ -1984,6 +4097,7 @@ match p with
                           | Some false => lts_set_tau B
                           | None => ∅
                           end
+  | ν p => list_to_set (map (fun q => ν q) (elements $ lts_set_tau p))
   | g gp => lts_set_tau_g gp
 end.
 
@@ -2006,6 +4120,8 @@ Proof.
       destruct (decide (c ⋉ d = c ⋉ d)). subst. assert (q = (g 𝟘)). set_solver.
       rewrite H. apply lts_output. exfalso. set_solver.
     + destruct (decide (a = c ⋉ d)). exfalso. apply n. assumption. set_solver.
+  - eapply elem_of_list_to_set, elem_of_list_fmap in mem as (q' & eq & mem). subst.
+    apply lts_res_ext. rewrite elem_of_elements in mem. eapply IHp in mem. simpl. destruct a. eauto.
 Qed.
 
 Lemma lts_set_output_spec1 p a q : lts p (ActExt $ ActOut a) q -> q ∈ lts_set_output p a.
@@ -2016,6 +4132,7 @@ Proof.
     + exfalso. apply not_eq. reflexivity.
   - simpl in *. rewrite H. eapply IHl; eauto ; simpl.
   - simpl in *. rewrite H. eapply IHl; eauto ; simpl.
+  - simpl in *. destruct a. try set_solver.
 Qed.
 
 Lemma lts_set_input_spec0 p a q : q ∈ lts_set_input p a -> lts p (ActExt $ ActIn a) q.
@@ -2034,8 +4151,10 @@ Proof.
       ++ eapply lts_ifOne; eauto.
       ++ eapply lts_ifZero; eauto.
     - intros. rewrite H in mem. exfalso. inversion mem.
+  + eapply elem_of_list_to_set, elem_of_list_fmap in mem as (q' & eq & mem). subst.
+    apply lts_res_ext. rewrite elem_of_elements in mem. eapply IHp in mem. simpl. destruct a. eauto. 
   + dependent induction g0; simpl in mem; try set_solver.
-      ++ destruct (decide (Channel_of a = c)).
+      ++ destruct (decide (ChannelData_of a = c)).
          +++ subst. eapply elem_of_singleton_1 in mem. subst. destruct a. simpl. apply lts_input.
          +++ destruct a. simpl in *. inversion mem.
       ++ eapply elem_of_union in mem. destruct mem; eauto with ccs.
@@ -2089,6 +4208,8 @@ Proof.
          +++ eapply lts_ifZero; eauto.
       ++ exfalso. inversion mem.
     + inversion mem.
+    + eapply elem_of_list_to_set, elem_of_list_fmap in mem as (t' & eq & h); subst.
+      eapply lts_res_tau. eapply IHp. eapply elem_of_elements. eauto.
     + dependent induction g0; simpl in mem; try set_solver;
         try eapply elem_of_singleton_1 in mem; subst; eauto with ccs.
       eapply elem_of_union in mem as [mem1 | mem2]; eauto with ccs.
@@ -2206,7 +4327,7 @@ Qed.
      lts_oba_output_deter p1 p2 p3 a := OBA_with_FB_Third_Axiom p1 p2 p3 a;
      lts_oba_output_tau p q1 q2 a := OBA_with_FB_Fifth_Axiom p q1 q2 a;
      lts_oba_output_deter_inv p1 p2 q1 q2 a := ExtraAxiom p1 p2 q1 q2 a;
-     lts_oba_mo p := moutputs_of p 
+     lts_oba_mo p := moutputs_of 0 p 
   |}.
   Next Obligation.
     intros. simpl. unfold outputs_of.
@@ -2246,7 +4367,7 @@ Defined.
 From Must Require Import Must.
 
 Inductive FinA :=
-| Inputs (c : Channel)
+| Inputs (c : ChannelData)
 .
 
 Definition Φ (μ : ExtAct TypeOfActions) : FinA :=
@@ -2263,9 +4384,9 @@ From Must Require Import DefinitionAS.
 Next Obligation.
   intros. destruct μ; destruct μ'; destruct a; destruct a0.
   - inversion H1; subst. eapply lts_refuses_spec1 in H2 as (e' & Tr). simpl in *.
-    eapply TransitionShapeForInput in Tr as (P1 & G & R & eq & eq' & Hyp).
-    assert (¬ (((gpr_input c0 P1 + G) ‖ R) ↛{ (c0 ⋉ d0) ? })) as accepts.
-    { eapply lts_refuses_spec2. exists (P1^(d0) ‖ R). eapply lts_parL. eapply lts_choiceL. constructor. }
+    eapply TransitionShapeForInput in Tr as (P1 & G & R & n & eq & eq' & Hyp).
+    assert (¬ (Ѵ n ((gpr_input (VarC_add n c0) P1 + G) ‖ R) ↛{ (c0 ⋉ d0) ? })) as accepts.
+    { eapply lts_refuses_spec2. exists (Ѵ n (P1 ^ d0 ‖ R)). eapply lts_res_ext_n. eapply lts_parL. eapply lts_choiceL. constructor. }
     eapply accepts_preserved_by_eq in accepts. exact accepts. symmetry. eauto.
   - unfold blocking in H0. exfalso. eapply H0. exists (c0 ⋉ d0). eauto.
   - unfold blocking in H. exfalso. eapply H. exists (c ⋉ d). eauto.
@@ -2284,50 +4405,301 @@ Next Obligation.
     - right. intro. inversion H. contradiction.
 Qed.
 
-Parameter CountPreAct : Countable PreAct.
+Definition encode_PreAct (c : PreAct) : gen_tree ChannelData :=
+match c with
+  | Inputs c => GenLeaf c
+end.
 
-#[global] Program Instance CountaPreAct: Countable PreAct := CountPreAct.
+Definition decode_PreAct (tree : gen_tree ChannelData) : option PreAct :=
+match tree with
+  | GenLeaf c => Some (Inputs c)
+  | _ => None
+end.
 
-Fixpoint  mPreCoAct_of p : gmultiset PreAct := 
+Lemma encode_decide_PreAct c : decode_PreAct (encode_PreAct c) = Some c.
+Proof. case c. 
+* intros. simpl. reflexivity.
+Qed.
+
+#[global] Instance CountPreAct : Countable PreAct.
+Proof.
+  refine (inj_countable encode_PreAct decode_PreAct _).
+  apply encode_decide_PreAct.
+Qed.
+
+Fixpoint  mPreCoAct_of (k : nat) p : gmultiset PreAct := 
 match p with
-  | P ‖ Q => (mPreCoAct_of P) ⊎ (mPreCoAct_of Q)
-  | c ! v • 𝟘 => {[+ (Inputs c) +]}
+  | P ‖ Q => (mPreCoAct_of k P) ⊎ (mPreCoAct_of k Q)
+  | (cstC c) ! v • 𝟘 => {[+ Inputs (cstC c) +]}
+  | (bvarC i) ! v • 𝟘 => if decide(k < (S i)) then {[+ Inputs (bvarC (i - k)) +]}
+                                              else ∅
   | pr_var _ => ∅
   | rec _ • _ => ∅
   | If E Then P Else Q => match (Eval_Eq E) with 
-                          | Some true => mPreCoAct_of P
-                          | Some false => mPreCoAct_of Q
+                          | Some true => mPreCoAct_of k P
+                          | Some false => mPreCoAct_of k Q
                           | None => ∅
                           end
+  | ν p => mPreCoAct_of (S k) p
   | g p => ∅
 end.
 
-Definition PreCoAct_of p := dom (mPreCoAct_of p).
+Definition PreCoAct_of p := dom (mPreCoAct_of 0 p).
 
-Lemma PreCoEquiv (p : proc) (q : proc) (c : PreAct) : p ⋍ q -> c ∈ PreCoAct_of p -> c ∈ PreCoAct_of q.
+Lemma mPreCoAct_of_res_n_g j n g1 : mPreCoAct_of j (Ѵ n (g g1)) = mPreCoAct_of (n + j) (g g1).
 Proof.
-  intros eq mem. revert eq mem.
-  intros.
+  revert g1 j.
+  induction n.
+  + simpl; eauto.
+  + intros; simpl in *. replace (S (n + j))%nat with (n + (S j))%nat by lia.
+    eapply IHn.
+Qed.
+
+Lemma mPreCoAct_of_res_n j n p1 : mPreCoAct_of j (Ѵ n p1) = mPreCoAct_of (n + j) p1.
+Proof.
+  revert p1 j.
+  induction n.
+  + simpl; eauto.
+  + intros; simpl in *. replace (S (n + j))%nat with (n + (S j))%nat by lia.
+    eapply IHn.
+Qed.
+
+Lemma PreCoAct_NewVarC k j p : mPreCoAct_of (k + S j) (NewVarC j p) = mPreCoAct_of (k + j) p.
+Proof.
+  revert k j.
   induction p as (p & Hp) using
-        (well_founded_induction (wf_inverse_image _ nat _ size Nat.lt_wf_0)). destruct p.
-  + eapply gmultiset_elem_of_dom in mem. simpl in *. eapply gmultiset_elem_of_disj_union in mem.
-    destruct mem as [mem1 | mem2].
-    - eapply gmultiset_elem_of_dom in mem1. eapply Hp; admit.
-    - eapply gmultiset_elem_of_dom in mem2. eapply Hp; admit.
-  + inversion mem.
-  + inversion mem.
-  + case_eq (Eval_Eq e); intros; simpl in *.
-        eapply gmultiset_elem_of_dom in mem. simpl in *. rewrite H in mem. destruct b.
-        -- admit.
-        -- admit.
-        -- eapply gmultiset_elem_of_dom in mem. simpl in *. rewrite H in mem. inversion mem.
-  + assert (¬ q ↛[ ActOut (c0 ⋉ d) ]).
-    { eapply accepts_preserved_by_eq. eapply lts_refuses_spec2.
-      exists 𝟘. constructor. eauto. } admit.
-  + inversion mem.
-Admitted.
+    (well_founded_induction (wf_inverse_image _ nat _ size Nat.lt_wf_0));
+  destruct p; intros k j; simpl in *; eauto.
+  + assert (mPreCoAct_of (k + S j) (NewVarC j p1) = mPreCoAct_of (k + j) p1) as eq1.
+    { eapply Hp. simpl. lia. }
+    assert (mPreCoAct_of (k + S j) (NewVarC j p2) = mPreCoAct_of (k + j) p2) as eq2.
+    { eapply Hp. simpl. lia. }
+    rewrite eq1, eq2. eauto.
+  + case_eq (Eval_Eq e).
+    ++ intros. destruct b.
+       +++ eauto with lia.
+       +++ eauto with lia.
+    ++ eauto with lia.
+  + destruct c; simpl.
+      ++ eauto.
+      ++ destruct (decide (j < S n)).
+         +++ destruct (decide (k + j < S n)).
+             ++++ rewrite decide_True; try lia.
+                  replace (S n - (k + S j))%nat with (n - (k + j))%nat by lia. eauto.
+             ++++ rewrite decide_False; try lia. eauto.
+         +++ rewrite decide_False; try lia.
+             rewrite decide_False; try lia. eauto.
+  + replace (S (k + S j))%nat with (k + S (S j))%nat by lia.
+    replace (S (k + j))%nat with (k + S j)%nat by lia.
+    eapply Hp. simpl; eauto.
+Qed.
+
+Lemma PreCoAct_VarSwap k j p : mPreCoAct_of (j + S (S k)) p = mPreCoAct_of (j + S (S k)) (VarSwap_in_proc j p).
+Proof.
+  revert k j.
+  induction p as (p & Hp) using
+    (well_founded_induction (wf_inverse_image _ nat _ size Nat.lt_wf_0));
+  destruct p; intros k j; simpl in *; eauto.
+  + assert (mPreCoAct_of (j + S (S k)) p1 = mPreCoAct_of (j + S (S k)) (VarSwap_in_proc j p1)) as eq1.
+    { eapply Hp; simpl; eauto. lia. }
+    assert (mPreCoAct_of (j + S (S k)) p2 = mPreCoAct_of (j + S (S k)) (VarSwap_in_proc j p2)) as eq2.
+    { eapply Hp; simpl; eauto. lia. } rewrite eq1, eq2. eauto.
+  + case_eq (Eval_Eq e).
+    ++ intros. destruct b.
+       +++ eauto with lia.
+       +++ eauto with lia.
+    ++ eauto with lia.
+  + destruct c.
+      ++ simpl. eauto.
+      ++ simpl. destruct (decide (j + S (S k) < S n)).
+         ++++ destruct (decide (n = j)).
+              +++++ subst. destruct (decide (j + S (S k) < S (S j))).
+                    ++++++ lia.
+                    ++++++ lia.
+              +++++ destruct (decide (n = S j)).
+                    ++++++ subst. lia.
+                    ++++++ rewrite decide_True; try lia. eauto.
+         ++++ destruct (decide (n = j)).
+              +++++ subst. rewrite decide_False; try lia. eauto.
+              +++++ destruct (decide (n = S j)).
+                    ++++++ subst. rewrite decide_False; try lia. eauto.
+                    ++++++ rewrite decide_False; try lia. eauto.
+  + replace (S (j + S (S k)))%nat with ((S j) + S (S k))%nat by lia.
+    eapply Hp. simpl; eauto.
+Qed.
+
+Lemma PreCoEquiv (k : nat) (p : proc) (q : proc) (c : PreAct) : p ≡* q -> c ∈ mPreCoAct_of k p -> c ∈ mPreCoAct_of k q.
+Proof.
+  intros eq mem. revert k c mem. dependent induction eq.
+  + dependent induction H; intros; simpl in *; subst; eauto; try multiset_solver.
+    * rewrite H in mem; eauto.
+    * rewrite H; eauto.
+    * rewrite H in mem; eauto.
+    * rewrite H; eauto.
+    * replace (S (S k))%nat with (0 + (S (S k)))%nat by lia. rewrite<- PreCoAct_VarSwap. simpl; eauto.
+    * replace (S (S k))%nat with (0 + (S (S k)))%nat in mem by lia. rewrite<- PreCoAct_VarSwap in mem. simpl; eauto.
+    * eapply gmultiset_elem_of_disj_union in mem. destruct mem.
+      - eapply gmultiset_elem_of_disj_union. left. eauto.
+      - eapply gmultiset_elem_of_disj_union. right.
+        replace (S k)%nat with (k + S 0)%nat in H by lia. rewrite PreCoAct_NewVarC in H.
+        replace (k + 0)%nat with k%nat in H by lia. eauto.
+    * eapply gmultiset_elem_of_disj_union in mem. destruct mem.
+      - eapply gmultiset_elem_of_disj_union. left. eauto.
+      - eapply gmultiset_elem_of_disj_union. right.
+        replace (S k)%nat with (k + S 0)%nat by lia. rewrite PreCoAct_NewVarC.
+        replace (k + 0)%nat with k%nat by lia. eauto.
+    * case_eq (Eval_Eq C).
+      ++ intros. destruct b.
+         +++ rewrite H0 in mem; eauto.
+         +++ rewrite H0 in mem; eauto.
+      ++ intros. rewrite H0 in mem; eauto.
+    * case_eq (Eval_Eq C).
+      ++ intros. destruct b.
+         +++ rewrite H0 in mem; eauto.
+         +++ rewrite H0 in mem; eauto.
+      ++ intros. rewrite H0 in mem; eauto.
+  + eauto.
+Qed.
 
 From Must Require Import Subset_Act.
+
+Definition VarC_preaction_add (k : nat) (pre_μ : FinA) : FinA :=
+match pre_μ with
+| Inputs c => Inputs (VarC_add k c)
+end.
+
+Lemma VarC_preaction_add_zero pre_μ : VarC_preaction_add 0 pre_μ = pre_μ.
+Proof.
+  destruct pre_μ; simpl; destruct c; eauto.
+Qed.
+
+Lemma VarC_preaction_add_rev j k pre_μ μ' : 
+      VarC_preaction_add (j + k) pre_μ = Φ (VarC_action_add (j + k) μ') 
+      -> VarC_preaction_add k pre_μ = Φ (VarC_action_add k μ').
+Proof.
+  revert k pre_μ μ'.
+  induction j.
+  + simpl; eauto.
+  + intros; simpl. destruct pre_μ; destruct μ'.
+    ++ destruct c; destruct a.
+       +++ simpl in *. destruct c0.
+           ++++ simpl; eauto.
+           ++++ simpl in *. inversion H.
+       +++ simpl in *. destruct c.
+           ++++ simpl in *. inversion H.
+           ++++ simpl in *. inversion H. f_equal. assert (n = n0)%nat by lia. subst; eauto.
+    ++ destruct c; destruct a.
+       +++ simpl in *. destruct c0.
+           ++++ simpl; eauto.
+           ++++ simpl in *. inversion H.
+       +++ simpl in *. destruct c.
+           ++++ simpl in *. inversion H.
+           ++++ simpl in *. inversion H. f_equal. assert (n = n0)%nat by lia. subst; eauto.
+Qed.
+
+Lemma simpl_dual_VarC_add μ'' μ' k : dual μ'' (VarC_action_add k μ') -> μ'' = VarC_action_add k (co μ').
+Proof.
+  revert μ'' μ'.
+  intros; eauto. destruct μ'; destruct a; destruct c; symmetry in H;
+    destruct μ''; simpl in * ; try inversion H; subst; eauto.
+Qed.
+
+Lemma simpl_dual_VarC j k μ': dual (VarC_action_add (j + k) (co μ')) (VarC_action_add (j + k) μ') 
+              -> dual (VarC_action_add k (co μ')) (VarC_action_add k μ').
+Proof.
+  intros. destruct μ'; destruct a; destruct c; simpl; eauto.
+Qed.
+
+Lemma simpl_blocking_Varc j k μ' : @blocking _ (@gLabel_nb TypeOfActions VACCS_Label) (VarC_action_add (j + k) μ') 
+  -> @blocking _ (@gLabel_nb TypeOfActions VACCS_Label)(VarC_action_add k μ').
+Proof.
+  intros. destruct μ'; destruct a; destruct c; simpl; eauto.
+  + intro imp; inversion imp; inversion H0.
+  + intro. simpl in *. inversion H0. inversion H1. subst.
+    assert (non_blocking_output (ActOut ((j + k + n)%nat ⋉ d))).
+    exists ((j + k + n)%nat ⋉ d). eauto. contradiction.
+Qed.
+Check @co_actions_of.
+Lemma VarC_action_add_co_rev j k μ' p : VarC_action_add (j + k) μ' ∈ @co_actions_of _ _ (@gLabel_nb TypeOfActions VACCS_Label) _ p
+                        -> VarC_action_add k μ' ∈ @co_actions_of _ _ (@gLabel_nb TypeOfActions VACCS_Label) _ (Ѵ  j p).
+Proof.
+  revert k μ' p.
+  induction j.
+  + simpl ;eauto.
+  + intros; simpl in *. rewrite<- BigNew_reverse_def_one.
+    eapply IHj. exists (VarC_action_add (j + k) (co μ')).
+    destruct H as (μ'' & eq1 & eq2 & eq3).
+    eapply lts_refuses_spec1 in eq1 as (p' & tr). 
+    assert (dual μ'' (VarC_action_add (S (j + k)) μ')); eauto.
+    eapply simpl_dual_VarC_add in eq2. subst.
+    repeat split.
+    ++ eapply lts_refuses_spec2. exists (ν p'). eapply lts_res_ext.
+       rewrite VarC_action_add_add; simpl; eauto.
+    ++ eapply (simpl_dual_VarC 1). simpl; eauto.
+    ++ eapply (simpl_blocking_Varc 1). simpl ; eauto.
+Qed.
+
+Lemma specPreAct1 k : ∀ (pre_μ : FinA) (p : proc),
+  𝝳 (pre_μ) ∈ (λ p0 : proc, mPreCoAct_of k p0) p
+    → (VarC_preaction_add k pre_μ)
+      ∈ (λ (p0 : proc) (pre_μ0 : FinA),
+           ∃ μ' : ExtAct TypeOfActions, pre_μ0 = Φ (VarC_action_add k μ') 
+     ∧ (VarC_action_add k μ') ∈ @co_actions_of proc (ExtAct TypeOfActions)
+      (@gLabel_nb TypeOfActions VACCS_Label)
+      (@ggLts TypeOfActions (@gLabel_nb TypeOfActions VACCS_Label) proc
+         VACCS_Label VACCS_Lts) p0) p.
+Proof.
+  intros. simpl in *. revert k pre_μ H.
+  induction p as (p & Hp) using
+        (well_founded_induction (wf_inverse_image _ nat _ size Nat.lt_wf_0)).
+  destruct p; intros; simpl in *.
+  * eapply gmultiset_elem_of_disj_union in H. destruct H.
+    -- eapply (Hp p1) in H. destruct H as (μ' & eq & mem).
+       destruct mem as (μ'' & Tr & duo & b). exists μ'. split; eauto. 
+       exists μ''. repeat split; eauto. eapply lts_refuses_spec1 in Tr as (p'1 & Tr).
+       eapply lts_refuses_spec2. exists (p'1 ‖ p2). constructor. eauto. simpl. lia.
+    -- eapply (Hp p2) in H. destruct H as (μ' & eq & mem).
+       exists μ'. split; eauto. destruct mem as (μ'' & Tr & duo & b).
+       exists μ''. repeat split; eauto. eapply lts_refuses_spec1 in Tr as (p'2 & Tr).
+       eapply lts_refuses_spec2. exists (p1 ‖ p'2). constructor. eauto. simpl. lia.
+  * simpl in *. inversion H.
+  * simpl in *. inversion H.
+  * case_eq (Eval_Eq e); intros; simpl in *. rewrite H0 in H. destruct b.
+    -- eapply (Hp p1) in H. destruct H as (μ' & eq & mem).
+       exists μ'. split; eauto. destruct mem as (μ'' & Tr & duo & b).
+       exists μ''. repeat split; eauto. eapply lts_refuses_spec1 in Tr as (p'1 & Tr).
+       eapply lts_refuses_spec2. exists p'1. constructor; eauto. lia.
+    -- eapply (Hp p2) in H. destruct H as (μ' & eq & mem).
+       exists μ'. split; eauto. destruct mem as (μ'' & Tr & duo & b).
+       exists μ''. repeat split; eauto. eapply lts_refuses_spec1 in Tr as (p'2 & Tr).
+       eapply lts_refuses_spec2. exists p'2. eapply lts_ifZero; eauto. lia.
+    -- eapply gmultiset_elem_of_dom in H. simpl in *. rewrite H0 in H. inversion H.
+  * simpl in *.
+       destruct pre_μ.
+       + simpl in *. subst. destruct c.
+         ++ assert (Inputs c0 = Inputs c) by multiset_solver. inversion H0. subst.
+            exists (ActIn (c ⋉ d)). split.
+            -- simpl in *. reflexivity.
+            -- exists (ActOut (c ⋉ d)). repeat split ;eauto.
+               eapply lts_refuses_spec2. exists 𝟘. constructor.
+               intro imp. unfold non_blocking in imp. simpl in *.
+               inversion imp. inversion H1.
+         ++ destruct (decide (k < S n)).
+            +++ assert (Inputs c0 = Inputs (bvarC (n - k))) by multiset_solver. inversion H0. subst.
+                exists (ActIn (bvarC (n - k) ⋉ d)). split.
+                -- simpl in *. reflexivity.
+                -- exists (ActOut (bvarC n ⋉ d)). repeat split ;eauto.
+                   eapply lts_refuses_spec2. exists 𝟘. constructor. simpl. eauto with lia.
+                   replace  (k + (n - k))%nat with n%nat by lia. eauto.
+                   intro imp. unfold non_blocking in imp. simpl in *.
+                   inversion imp. inversion H1.
+            +++ inversion H.
+  * unfold PreCoAct_of in H.
+    eapply Hp in H as ( μ' & eq1 & eq2); simpl ; eauto. exists μ'.
+    split. eapply VarC_preaction_add_rev. instantiate (1:= 1). simpl; eauto.
+    eapply (VarC_action_add_co_rev 1). simpl ;eauto.
+  * inversion H.
+Qed.
 
 #[global] Program Instance gPreExtAction : 
   @PreExtAction (ExtAct TypeOfActions) gLabel_nb proc FinA PreAct EqPreAct CountPreAct 𝝳 Φ (ggLts gLabel_nb) :=
@@ -2352,45 +4724,19 @@ Next Obligation.
     + destruct mem as (μ' & Tr & duo & b). symmetry in duo.
       destruct a. eapply simplify_match_input in duo. subst.
       eapply lts_refuses_spec1 in Tr as (p' & Tr).
-      eapply TransitionShapeForOutput in Tr as (R & eq & eq').
-      assert (𝝳 (Φ (ActIn (c ⋉ d))) ∈ PreCoAct_of ((c ! d • 𝟘) ‖ R)).
-      { eapply gmultiset_elem_of_dom. simpl. multiset_solver. }
-      eapply PreCoEquiv. symmetry. eauto. eauto.
+      eapply TransitionShapeForOutput in Tr as (R & n & eq & eq').
+      assert (𝝳 (Φ (ActIn (c ⋉ d))) ∈ PreCoAct_of (Ѵ n ((VarC_add n c ! d • 𝟘) ‖ R))).
+      { eapply gmultiset_elem_of_dom. simpl. rewrite mPreCoAct_of_res_n.
+        simpl. destruct c; simpl.
+        + multiset_solver.
+        + rewrite decide_True; try lia. replace (n + n0 - (n + 0))%nat with n0%nat by lia.
+          multiset_solver. }
+      eapply gmultiset_elem_of_dom. eapply PreCoEquiv. symmetry. eauto.
+      eapply gmultiset_elem_of_dom. eauto.
     + destruct mem as (μ' & Tr & duo & b).
       destruct b. exists a; eauto.
-  - intros. simpl in *. revert pre_μ H.
-      induction p as (p & Hp) using
-        (well_founded_induction (wf_inverse_image _ nat _ size Nat.lt_wf_0)).
-      intros. (* destruct pre_pre_μ. *) destruct p; intros. (* destruct pre_μ; simpl in *.  *)
-      * eapply gmultiset_elem_of_dom in H.
-        eapply gmultiset_elem_of_disj_union in H. destruct H.
-        -- eapply gmultiset_elem_of_dom in H. eapply (Hp p1) in H. destruct H as (μ' & eq & mem). 
-           destruct mem as (μ'' & Tr & duo & b). exists μ'. split; eauto. 
-           exists μ''. repeat split; eauto. eapply lts_refuses_spec1 in Tr as (p'1 & Tr).
-           eapply lts_refuses_spec2. exists (p'1 ‖ p2). constructor. eauto. simpl. lia.
-        -- eapply gmultiset_elem_of_dom in H.  eapply (Hp p2) in H. destruct H as (μ' & eq & mem).
-           exists μ'. split; eauto. destruct mem as (μ'' & Tr & duo & b).
-           exists μ''. repeat split; eauto. eapply lts_refuses_spec1 in Tr as (p'2 & Tr).
-           eapply lts_refuses_spec2. exists (p1 ‖ p'2). constructor. eauto. simpl. lia.
-      * simpl in *. inversion H.
-      * simpl in *. inversion H.
-      * case_eq (Eval_Eq e); intros; simpl in *.
-        eapply gmultiset_elem_of_dom in H. simpl in *. rewrite H0 in H. destruct b.
-        -- eapply gmultiset_elem_of_dom in H. eapply (Hp p1) in H. destruct H as (μ' & eq & mem).
-           exists μ'. split; eauto. destruct mem as (μ'' & Tr & duo & b).
-           exists μ''. repeat split; eauto. eapply lts_refuses_spec1 in Tr as (p'1 & Tr).
-           eapply lts_refuses_spec2. exists p'1. constructor; eauto. lia.
-        -- eapply gmultiset_elem_of_dom in H. eapply (Hp p2) in H. destruct H as (μ' & eq & mem).
-           exists μ'. split; eauto. destruct mem as (μ'' & Tr & duo & b).
-           exists μ''. repeat split; eauto. eapply lts_refuses_spec1 in Tr as (p'2 & Tr).
-           eapply lts_refuses_spec2. exists p'2. eapply lts_ifZero; eauto. lia.
-        -- eapply gmultiset_elem_of_dom in H. simpl in *. rewrite H0 in H. inversion H.
-      * eapply gmultiset_elem_of_dom in H. simpl in *.
-        exists (ActIn (c ⋉ d)). split.
-        -- simpl in *. destruct pre_μ. unfold 𝝳 in H. assert (c = c0) by multiset_solver; subst. eauto.
-        -- exists (ActOut (c ⋉ d)). repeat split ;eauto.
-           eapply lts_refuses_spec2. exists 𝟘. constructor.
-           intro imp. inversion imp. destruct x; subst. inversion H0.
-      * inversion H.
+  - intros; subst. eapply gmultiset_elem_of_dom in H.
+    eapply (specPreAct1 0) in H. rewrite VarC_preaction_add_zero in H.
+    destruct H. rewrite VarC_add_zero_ext in H. exists x. destruct H. split ;eauto.
 Qed.
 
