theories/Testing_Pre_orders/Testing_Predicate/Exemples_of_Testing_Predicate/VACCS_Good.v
@@ -26,14 +26,15 @@
 From Coq.Program Require Import Equality.
 From stdpp Require Import countable decidable.
 From Must Require Import gLts InputOutputActions GeneralizeLtsOutputs Must VACCS_Instance Testing_Predicate.
-
+From Coq.Wellfounded Require Import Inverse_Image.
 
 Inductive good_VACCS : proc -> Prop :=
 | good_success : good_VACCS ①
 | good_par : forall p q, good_VACCS p \/ good_VACCS q -> good_VACCS (p ‖ q)
 | good_choice : forall p q, good_VACCS (g p) \/ good_VACCS (g q) -> good_VACCS (p + q)
 | good_if_true : forall E p q, good_VACCS p -> Eval_Eq E = Some true -> good_VACCS (If E Then p Else q)
-| good_if_false : forall E p q, good_VACCS q -> Eval_Eq E = Some false -> good_VACCS (If E Then p Else q).
+| good_if_false : forall E p q, good_VACCS q -> Eval_Eq E = Some false -> good_VACCS (If E Then p Else q)
+| good_res : forall p, good_VACCS p -> good_VACCS (ν p).
 
 #[global] Hint Constructors good_VACCS:ccs.
 
@@ -51,9 +52,98 @@ Proof.
         right. inversion 1; naive_solver.
         right. inversion 1; naive_solver.
     + right. inversion 1; naive_solver.
+  - destruct IHe. 
+    + left. eapply good_res. eauto.
+    + right. intro imp. inversion imp; eauto.
   - dependent induction g; try (now right; inversion 1); try (now left; eauto with ccs).
     destruct IHg1; destruct IHg2; try (now left; eauto with ccs).
     right. inversion 1; naive_solver.
+Qed.
+
+Lemma VarSwap_respects_good k p : good_VACCS p <-> good_VACCS (VarSwap_in_proc k p).
+Proof.
+  split.
+  + revert k. induction p as (p & Hp) using
+    (well_founded_induction (wf_inverse_image _ nat _ size Nat.lt_wf_0)).
+    destruct p; intros; simpl in *; eauto.
+    ++ dependent destruction H. destruct H.
+       +++ eapply good_par. left. eapply Hp. simpl; lia. eauto.
+       +++ eapply good_par. right. eapply Hp. simpl; lia. eauto.
+    ++ inversion H.
+    ++ inversion H; subst.
+       +++ eapply good_if_true; eauto. eapply Hp. simpl; lia. eauto.
+       +++ eapply good_if_false; eauto. eapply Hp. simpl; lia. eauto.
+    ++ inversion H.
+    ++ dependent destruction H. eapply good_res. eapply Hp. simpl; lia. eauto.
+    ++ destruct g; intros; simpl in *; eauto; try now inversion H.
+       dependent destruction H. destruct H.
+       +++ eapply good_choice. left.
+           assert (good_VACCS (VarSwap_in_proc k (g g1))) as eq1.
+           { eapply Hp. simpl; lia. eauto. }
+           simpl in *; eauto.
+       +++ eapply good_choice. right.
+           assert (good_VACCS (VarSwap_in_proc k (g g2))) as eq2.
+           { eapply Hp. simpl; lia. eauto. }
+           simpl in *; eauto.
+  + revert k. induction p as (p & Hp) using
+    (well_founded_induction (wf_inverse_image _ nat _ size Nat.lt_wf_0)).
+    destruct p; intros; simpl in *; eauto.
+    ++ dependent destruction H. destruct H.
+       +++ eapply good_par. left. eapply Hp. simpl; lia. eauto.
+       +++ eapply good_par. right. eapply Hp. simpl; lia. eauto.
+    ++ inversion H.
+    ++ inversion H; subst.
+       +++ eapply good_if_true; eauto. eapply Hp. simpl; lia. eauto.
+       +++ eapply good_if_false; eauto. eapply Hp. simpl; lia. eauto.
+    ++ simpl in *. inversion H.
+    ++ dependent destruction H. eapply good_res. eapply Hp. simpl; lia. eauto.
+    ++ destruct g; intros; simpl in *; eauto; try now inversion H.
+       dependent destruction H. destruct H.
+       +++ eapply good_choice. left. eapply Hp. simpl; lia. eauto.
+       +++ eapply good_choice. right. eapply Hp. simpl; lia. eauto.
+Qed.
+
+Lemma NewVarC_respects_good k p : good_VACCS p <-> good_VACCS (NewVarC k p).
+Proof.
+  split.
+  + revert k. induction p as (p & Hp) using
+    (well_founded_induction (wf_inverse_image _ nat _ size Nat.lt_wf_0)).
+    destruct p; intros; simpl in *; eauto.
+    ++ dependent destruction H. destruct H.
+       +++ eapply good_par. left. eapply Hp. simpl; lia. eauto.
+       +++ eapply good_par. right. eapply Hp. simpl; lia. eauto.
+    ++ inversion H.
+    ++ inversion H; subst.
+       +++ eapply good_if_true; eauto. eapply Hp. simpl; lia. eauto.
+       +++ eapply good_if_false; eauto. eapply Hp. simpl; lia. eauto.
+    ++ inversion H.
+    ++ dependent destruction H. eapply good_res. eapply Hp. simpl; lia. eauto.
+    ++ destruct g; intros; simpl in *; eauto; try now inversion H.
+       dependent destruction H. destruct H.
+       +++ eapply good_choice. left.
+           assert (good_VACCS (NewVarC k (g g1))) as eq1.
+           { eapply Hp. simpl; lia. eauto. }
+           simpl in *; eauto.
+       +++ eapply good_choice. right.
+           assert (good_VACCS (NewVarC k (g g2))) as eq2.
+           { eapply Hp. simpl; lia. eauto. }
+           simpl in *; eauto.
+  + revert k. induction p as (p & Hp) using
+    (well_founded_induction (wf_inverse_image _ nat _ size Nat.lt_wf_0)).
+    destruct p; intros; simpl in *; eauto.
+    ++ dependent destruction H. destruct H.
+       +++ eapply good_par. left. eapply Hp. simpl; lia. eauto.
+       +++ eapply good_par. right. eapply Hp. simpl; lia. eauto.
+    ++ inversion H.
+    ++ inversion H; subst.
+       +++ eapply good_if_true; eauto. eapply Hp. simpl; lia. eauto.
+       +++ eapply good_if_false; eauto. eapply Hp. simpl; lia. eauto.
+    ++ inversion H.
+    ++ dependent destruction H. eapply good_res. eapply Hp. simpl; lia. eauto.
+    ++ destruct g; intros; simpl in *; eauto; try now inversion H.
+       dependent destruction H. destruct H.
+       +++ eapply good_choice. left. eapply Hp. simpl; lia. eauto.
+       +++ eapply good_choice. right. eapply Hp. simpl; lia. eauto.
 Qed.
 
 Lemma good_preserved_by_cgr_step p q : good_VACCS p -> p ≡ q -> good_VACCS q.
@@ -73,6 +163,16 @@ Proof.
   + dependent destruction happy. dependent destruction H.
     eapply good_par; eauto. left. eapply good_par; eauto.
     dependent destruction H. eapply good_par. destruct H; eauto. left. eapply good_par; eauto.
+  + eapply good_res. eapply good_res. inversion happy; subst.
+    inversion H0. subst. eapply VarSwap_respects_good in H1. eauto.
+  + eapply good_res. eapply good_res. inversion happy; subst.
+    inversion H0. subst. eapply VarSwap_respects_good in H1. eauto.
+  + inversion happy; subst. inversion H0;subst. destruct H1.
+    ++ eapply good_par. left. eapply good_res. eauto.
+    ++ eapply good_par. right. eapply NewVarC_respects_good. eauto.
+  + eapply good_res. eapply good_par. inversion happy; eauto; subst. destruct H0.
+    ++ left. inversion H; subst; eauto.
+    ++ right. eapply NewVarC_respects_good in H. eauto.
   + dependent destruction happy ;eauto. destruct H; eauto. inversion H.
   + eapply good_choice. left; eauto.
   + dependent destruction happy ;eauto. eapply good_choice. destruct H; eauto.
@@ -85,6 +185,7 @@ Proof.
     left. eapply good_choice; eauto.
   + dependent destruction happy. destruct H. eapply good_par. left. eauto.
     eapply good_par. right. eauto.
+  + eapply good_res; eauto. inversion happy ; subst; eauto.
   + dependent destruction happy. eapply good_if_true; eauto.
     eapply good_if_false; eauto.
   + dependent destruction happy. eapply good_if_true; eauto.
@@ -99,18 +200,29 @@ Proof.
   dependent induction hcgr; [eapply good_preserved_by_cgr_step|]; eauto.
 Qed.
 
+Lemma good_VACCS_res_n n p : good_VACCS p <-> good_VACCS (Ѵ n p).
+Proof.
+  split.
+  + revert p. induction n.
+    -- simpl; eauto.
+    -- intros. simpl in *. eapply good_res. eauto.
+  + revert p. induction n.
+    -- simpl; eauto.
+    -- intros. simpl in *. inversion H; subst. eauto.
+Qed.
+
 Lemma good_preserved_by_non_bloking_actions p q a : good_VACCS p -> lts p (a !) q -> good_VACCS q.
 Proof.
   intros hhp hl. destruct a.
-  eapply TransitionShapeForOutputSimplified in hl.
-  eapply (good_preserved_by_cgr p ((c ! d • 𝟘) ‖ q)) in hhp; eauto with ccs.
-  inversion hhp; subst. destruct H0; eauto with ccs. inversion H.
+  eapply TransitionShapeForOutputSimplified in hl as (n & hl).
+  eapply (good_preserved_by_cgr p (Ѵ n (VarC_add n c ! d • 𝟘) ‖ q)) in hhp; eauto with ccs.
+  inversion hhp; subst. destruct H0; eauto with ccs. eapply good_VACCS_res_n in H. inversion H.
 Qed.
 
 Lemma good_preserved_by_non_bloking_actions_converse p q a : lts p (a !) q -> good_VACCS q -> good_VACCS p.
 Proof.
   intros hl hhq. destruct a.
-  eapply TransitionShapeForOutputSimplified in hl.
+  eapply TransitionShapeForOutputSimplified in hl as (n & hl).
   eapply good_preserved_by_cgr.
   eapply good_par. right.
   eauto with ccs. symmetry. eauto with ccs.
