theories/Labelled_Transition_System/Examples_of_LTS/VACCS/Testing/VACCS_tc.v
@@ -108,6 +108,7 @@ destruct p; intros.
   { apply Hp. simpl. auto with arith. }
   rewrite eq1, eq2. auto.
 * simpl. rewrite All_According_To_Data. reflexivity.
+* simpl. f_equal. eauto.
 * destruct g.
   - simpl. auto.
   - simpl. auto.
@@ -198,6 +199,7 @@ destruct p; simpl; intros.
   { apply Hp. simpl. auto with arith. }
   rewrite eq2, eq3. auto.
 * rewrite New_Var_And_NewVar_in_Data. eauto.
+* f_equal. eauto.
 * destruct g; simpl.
   - simpl. reflexivity.
   - simpl. reflexivity.
